@prefix clarify: <http://research.tib.eu/clarify2020/vocab/> .
@prefix owl: <http://www.w3.org/2002/07/owl#> .
@prefix rdf: <http://www.w3.org/1999/02/22-rdf-syntax-ns#> .
@prefix rdfs: <http://www.w3.org/2000/01/rdf-schema#> .
@prefix xsd: <http://www.w3.org/2001/XMLSchema#> .
@prefix dcterms: <http://purl.org/dc/terms/> .
@prefix dc: <http://purl.org/dc/elements/1.1/> .
@prefix prov: <http://www.w3.org/ns/prov#> .

#################################################################################################################################################
#################################################################################################################################################

<https://github.com/tibonto/clarify> rdf:type owl:Ontology ;
                                   owl:versionIRI <https://github.com/tibonto/clarify/tree/v8.0> ;
                                   dc:contributor "Samaneh Jozashoori" ,
                                                  "Maria-Esther Vidal" ;
                                   dc:creator "CLARIFY project" ;
                                   dc:title "CLARIFY Unified Schema" ;
                                   owl:versionInfo "v8.0" .

#################################################################################################################################################
#################################################################################################################################################
#################################################################################################################################################
###############################################################   Classes   #####################################################################
#################################################################################################################################################
#################################################################################################################################################
#################################################################################################################################################


######################################################################################################################################
#################################################    annotation   ##############################################################
######################################################################################################################################

<http://research.tib.eu/clarify2020/vocab/Source>	rdf:type	owl:Class;
				rdfs:label	"Source";
				rdfs:subClassOf	<http://research.tib.eu/clarify2020/vocab/Concept>;
				rdfs:comment "Represents the provenance of an extracted concept.";
				dcterms:modified "2021-12-29"^^xsd:date;
				dcterms:creator <https://www.tib.eu/en/research-development/scientific-data-management/staff/samaneh-jozashoori/>.

<http://research.tib.eu/clarify2020/vocab/SemanticType>	rdf:type	owl:Class;
						rdfs:label	"SemanticType";
						rdfs:subClassOf	<http://research.tib.eu/clarify2020/vocab/Concept>;
						rdfs:comment "Represents the Semantic Type provided by UMLS.";
						dcterms:modified "2021-07-21"^^xsd:date;
						dcterms:creator <https://www.tib.eu/en/research-development/scientific-data-management/staff/samaneh-jozashoori/>.

<http://research.tib.eu/clarify2020/vocab/SemanticTypeGroup>	rdf:type	owl:Class;
							rdfs:label	"SemanticTypeGroup";
							rdfs:subClassOf	<http://research.tib.eu/clarify2020/vocab/Concept>;
							rdfs:comment "Represents the Semantic Type Group provided by UMLS.";
							dcterms:modified "2021-07-21"^^xsd:date;
							dcterms:creator <https://www.tib.eu/en/research-development/scientific-data-management/staff/samaneh-jozashoori/>.

<http://research.tib.eu/clarify2020/vocab/AnnotationDefinition>	rdf:type	owl:Class;
								rdfs:label	"AnnotationDefinition";
								rdfs:subClassOf	<http://research.tib.eu/clarify2020/vocab/Concept>;
								rdfs:comment "Represents the definition of the UMLS CUI.";
								dcterms:modified "2021-12-16"^^xsd:date;
								dcterms:creator <https://www.tib.eu/en/research-development/scientific-data-management/staff/samaneh-jozashoori/>.

<http://research.tib.eu/clarify2020/vocab/AnnotationType>	rdf:type	owl:Class;
						rdfs:label	"AnnotationType";
						rdfs:subClassOf	<http://research.tib.eu/clarify2020/vocab/Concept>;
						rdfs:comment "Represents the type of the UMLS CUI.";
						dcterms:modified "2021-12-16"^^xsd:date;
						dcterms:creator <https://www.tib.eu/en/research-development/scientific-data-management/staff/samaneh-jozashoori/>.


######################################################################################################################################
#########################################################    Clinical    #############################################################
######################################################################################################################################



<http://research.tib.eu/clarify2020/vocab/Concept>	rdf:type	owl:Class;
				rdfs:label	"Concept";
				rdfs:comment "Constituents of thoughts or real world entities.";
				dcterms:modified "2020-10-19"^^xsd:date;
				dcterms:creator <https://www.tib.eu/en/research-development/scientific-data-management/staff/samaneh-jozashoori/>.

<http://research.tib.eu/clarify2020/vocab/Annotation>	rdf:type	owl:Class;
					rdfs:label	"Annotation";
					rdfs:comment "Annotation of a concept including label, id and source of concept.";
					dcterms:modified "2020-10-19"^^xsd:date;
					dcterms:creator <https://www.tib.eu/en/research-development/scientific-data-management/staff/samaneh-jozashoori/>.

<http://research.tib.eu/clarify2020/vocab/CPatient>	rdf:type	owl:Class;
					rdfs:label	"CancerPatient";
					rdfs:comment "Cancer Patient independent of type of their cancer.";
					dcterms:modified "2020-10-19"^^xsd:date;
					dcterms:creator <https://www.tib.eu/en/research-development/scientific-data-management/staff/samaneh-jozashoori/>.

<http://research.tib.eu/clarify2020/vocab/LCPatient>	rdf:type	owl:Class;
				rdfs:label	"LungCancerPatient";
				rdfs:subClassOf	<http://research.tib.eu/clarify2020/vocab/CPatient>;
				rdfs:comment "A patient who is diagnosed with Lung Cancer.";
				dcterms:modified "2020-10-19"^^xsd:date;			
				dcterms:creator <https://www.tib.eu/en/research-development/scientific-data-management/staff/samaneh-jozashoori/>.

<http://research.tib.eu/clarify2020/vocab/BCPatient>	rdf:type	owl:Class;
					rdfs:label	"BCPatient";
					rdfs:subClassOf	<http://research.tib.eu/clarify2020/vocab/CPatient>;
					rdfs:comment "A patient who is diagnosed with Breast Cancer.";
					dcterms:modified "2022-09-12"^^xsd:date;			
					dcterms:creator <https://www.tib.eu/en/research-development/scientific-data-management/staff/samaneh-jozashoori/>.

<http://research.tib.eu/clarify2020/vocab/Observation>	rdf:type	owl:Class;
				rdfs:label	"Observation";
				rdfs:subClassOf	<http://research.tib.eu/clarify2020/vocab/Concept>;
				rdfs:comment "Any record that relates to monitoring a process.";
				dcterms:modified "2021-01-25"^^xsd:date;			
				dcterms:creator <https://www.tib.eu/en/research-development/scientific-data-management/staff/samaneh-jozashoori/>.

<http://research.tib.eu/clarify2020/vocab/Diagnosis>  	rdf:type owl:Class;
					rdfs:label	"Diagnosis";
					rdfs:subClassOf	<http://research.tib.eu/clarify2020/vocab/Observation>;
					rdfs:comment "The identification of the nature of an illness or other problem by examination of the symptoms.";
					dcterms:modified "2020-09-15"^^xsd:date;
					dcterms:creator <https://www.tib.eu/en/research-development/scientific-data-management/staff/samaneh-jozashoori/>.	

<http://research.tib.eu/clarify2020/vocab/Sex>	rdf:type	owl:Class;
			rdfs:label	"Sex";
			rdfs:subClassOf	<http://research.tib.eu/clarify2020/vocab/Concept>;
			rdfs:comment "One of the main biological categories of female or male (independent of the gender identity).";
			dcterms:modified "2020-10-19"^^xsd:date;
			dcterms:creator <https://www.tib.eu/en/research-development/scientific-data-management/staff/samaneh-jozashoori/>.

<http://research.tib.eu/clarify2020/vocab/Race>	rdf:type	owl:Class;
				rdfs:label	"Race";
				rdfs:subClassOf	<http://research.tib.eu/clarify2020/vocab/Concept>;
				rdfs:comment "Categories of humankind that shares certain distinctive physical traits.";
				dcterms:modified "2020-10-19"^^xsd:date;
				dcterms:creator <https://www.tib.eu/en/research-development/scientific-data-management/staff/samaneh-jozashoori/>.						

<http://research.tib.eu/clarify2020/vocab/Biomarker>	 rdf:type	owl:Class;
					rdfs:label	"Biomarker";
					rdfs:subClassOf	<http://research.tib.eu/clarify2020/vocab/Concept>;
					rdfs:comment "A biomarker, or biological marker is a measurable indicator of some biological state or condition.";
					dcterms:modified "2020-10-19"^^xsd:date;
					dcterms:creator <https://www.tib.eu/en/research-development/scientific-data-management/staff/samaneh-jozashoori/>.

<http://research.tib.eu/clarify2020/vocab/ProgressionRelapse>	rdf:type	owl:Class;
							rdfs:label	"ProgressionRelapse";
							rdfs:subClassOf	<http://research.tib.eu/clarify2020/vocab/Concept>;
							rdfs:comment "Indicates the existance of progression OR relapse in the patient.";
							dcterms:modified "2021-02-25"^^xsd:date;
							dcterms:creator <https://www.tib.eu/en/research-development/scientific-data-management/staff/samaneh-jozashoori/>.	

<http://research.tib.eu/clarify2020/vocab/FamilyHistory>	rdf:type	owl:Class;
						rdfs:label	"FamilyHistory";
						rdfs:subClassOf	<http://research.tib.eu/clarify2020/vocab/Concept>;
						rdfs:comment "Represents the cancers from which the direct blood relatives of the patient have suffered.";
						dcterms:modified "2020-10-20"^^xsd:date;
						dcterms:creator <https://www.tib.eu/en/research-development/scientific-data-management/staff/samaneh-jozashoori/>.	

<http://research.tib.eu/clarify2020/vocab/ClinicalTrial>	rdf:type	owl:Class;
						rdfs:label	"ClinicalTrial";
						rdfs:subClassOf	<http://research.tib.eu/clarify2020/vocab/Observation>;
						rdfs:comment "Represents the clinical trial that the patient is involved in.";
						dcterms:modified "2020-10-20"^^xsd:date;
						dcterms:creator <https://www.tib.eu/en/research-development/scientific-data-management/staff/samaneh-jozashoori/>.

<http://research.tib.eu/clarify2020/vocab/Carcinogen>	rdf:type	owl:Class;
						rdfs:label	"Carcinogen";
						rdfs:subClassOf	<http://research.tib.eu/clarify2020/vocab/Concept>;
						rdfs:comment "A carcinogen is a substance, organism or agent capable of causing lung cancer.";
						dcterms:modified "2023-04-25"^^xsd:date;
						dcterms:creator <https://www.tib.eu/en/research-development/scientific-data-management/staff/emetis-niazmand/>.

<http://research.tib.eu/clarify2020/vocab/PTNMdiagnosis>	rdf:type	owl:Class;
						rdfs:label	"PTNMdiagnosis";
						rdfs:subClassOf	<http://research.tib.eu/clarify2020/vocab/Concept>;
						rdfs:comment "Pathological tumor-node-metastasis (pTNM) staging for papillary and follicular thyroid carcinomas.";
						dcterms:modified "2023-04-25"^^xsd:date;
						dcterms:creator <https://www.tib.eu/en/research-development/scientific-data-management/staff/emetis-niazmand/>.

<http://research.tib.eu/clarify2020/vocab/OccurrenceLocation>	rdf:type	owl:Class;
							rdfs:label	"OccurrenceLocation";
							rdfs:subClassOf	<http://research.tib.eu/clarify2020/vocab/Concept>;
							rdfs:comment "Superclass of metastasis location proportion and radiotherapy location.";
							dcterms:modified "2021-02-25"^^xsd:date;
							dcterms:creator <https://www.tib.eu/en/research-development/scientific-data-management/staff/samaneh-jozashoori/>.

<http://research.tib.eu/clarify2020/vocab/MetastasisLocation>	rdf:type	owl:Class;
							rdfs:label	"MetastasisLocation";
							rdfs:subClassOf	<http://research.tib.eu/clarify2020/vocab/OccurrenceLocation>;
							rdfs:comment "Determines the area to which the cancer is metastasized.";
							dcterms:modified "2020-10-20"^^xsd:date;
							dcterms:creator <https://www.tib.eu/en/research-development/scientific-data-management/staff/samaneh-jozashoori/>.

<http://research.tib.eu/clarify2020/vocab/ClinicalTrialTreatmentLine>	rdf:type	owl:Class;
									rdfs:label	"ClinicalTrialTreatmentLine";
									rdfs:subClassOf <http://research.tib.eu/clarify2020/vocab/OncologicalTreatmentLine>;
									rdfs:comment "Records of patients in clinical notes that are related to clinical trial treatment lines";
									dcterms:modified "2021-04-07"^^xsd:date;
									dcterms:creator <https://www.tib.eu/en/research-development/scientific-data-management/staff/samaneh-jozashoori/>.	

<http://research.tib.eu/clarify2020/vocab/OncologicalSurgery>	rdf:type	owl:Class;
							rdfs:label	"OncologicalSurgery";
							rdfs:subClassOf <http://research.tib.eu/clarify2020/vocab/TreatmentEpisode>;
							rdfs:comment "Is the branch of surgery applied to oncology; it focuses on the surgical management of tumors, especially cancerous tumors.";
							dcterms:modified "2022-09-12"^^xsd:date;
							dcterms:creator <https://www.tib.eu/en/research-development/scientific-data-management/staff/samaneh-jozashoori/>.																																	

<http://research.tib.eu/clarify2020/vocab/Drug>	rdf:type	owl:Class;
				rdfs:label	"Drug";
				rdfs:subClassOf	<http://research.tib.eu/clarify2020/vocab/Concept>;
				rdfs:comment "A substance used as a medication or in the preparation of medication.";
				dcterms:modified "2020-10-20"^^xsd:date;
				dcterms:creator <https://www.tib.eu/en/research-development/scientific-data-management/staff/samaneh-jozashoori/>.

<http://research.tib.eu/clarify2020/vocab/StageClassification>	rdf:type	owl:Class;
									rdfs:label	"StageClassification";
									rdfs:subClassOf	<http://research.tib.eu/clarify2020/vocab/Concept>;
									rdfs:comment "Techniques that are applied to indicate the TNM stage.";
									dcterms:modified "2020-10-21"^^xsd:date;
									dcterms:creator <https://www.tib.eu/en/research-development/scientific-data-management/staff/samaneh-jozashoori/>.

<http://research.tib.eu/clarify2020/vocab/Disorder>	rdf:type	owl:Class;
					rdfs:label	"Disorder";
					rdfs:subClassOf	<http://research.tib.eu/clarify2020/vocab/Concept>;
					rdfs:comment "A particular abnormal condition that negatively affects the structure or function of all or part of an organism, and that is not due to any immediate external injury.";
					dcterms:modified "2020-10-21"^^xsd:date;
					dcterms:creator <https://www.tib.eu/en/research-development/scientific-data-management/staff/samaneh-jozashoori/>.

<http://research.tib.eu/clarify2020/vocab/ComorbidityStatus>	rdf:type	owl:Class;
							rdfs:label	"ComorbidityStatus";
							rdfs:subClassOf	<http://research.tib.eu/clarify2020/vocab/Concept>;
							rdfs:comment "Represents the existence of comorbidity in patients.";
							dcterms:modified "2021-04-07"^^xsd:date;
							dcterms:creator <https://www.tib.eu/en/research-development/scientific-data-management/staff/samaneh-jozashoori/>.

<http://research.tib.eu/clarify2020/vocab/ComorbidityTreatmentLine>	rdf:type	owl:Class;
									rdfs:label	"ComorbidityTreatmentLine";
									rdfs:subClassOf	<http://research.tib.eu/clarify2020/vocab/Concept>;
									rdfs:comment "Represents the observation of comorbidities and symptoms in patients in each treatment line.";
									dcterms:modified "2021-06-22"^^xsd:date;
									dcterms:creator <https://www.tib.eu/en/research-development/scientific-data-management/staff/samaneh-jozashoori/>.

<http://research.tib.eu/clarify2020/vocab/StatusEvolution>	rdf:type	owl:Class;
							rdfs:label	"StatusEvolution";
							rdfs:subClassOf	<http://research.tib.eu/clarify2020/vocab/Observation>;
							rdfs:comment "Patient survival status through monitoring.";
							dcterms:modified "2020-10-21"^^xsd:date;
							dcterms:creator <https://www.tib.eu/en/research-development/scientific-data-management/staff/samaneh-jozashoori/>.

<http://research.tib.eu/clarify2020/vocab/TumorType>	rdf:type	owl:Class;
						rdfs:subClassOf <http://research.tib.eu/clarify2020/vocab/Concept>;
						rdfs:label	"TumorType";
						rdfs:comment "The histology kind of the lung cancer. The type of tumor.";
						dcterms:modified "2020-09-15"^^xsd:date;
						dcterms:creator <https://www.tib.eu/en/research-development/scientific-data-management/staff/samaneh-jozashoori/>.	

<http://research.tib.eu/clarify2020/vocab/PerformanceStatus>	rdf:type	owl:Class;
						rdfs:subClassOf <http://research.tib.eu/clarify2020/vocab/Observation>;
						rdfs:label	"PerformanceStatus";
						rdfs:comment "Represents the Performance Status of the patient.";
						dcterms:modified "2020-10-21"^^xsd:date;
						dcterms:creator <https://www.tib.eu/en/research-development/scientific-data-management/staff/samaneh-jozashoori/>.	

<http://research.tib.eu/clarify2020/vocab/NonOncologicalConsultation>  	rdf:type owl:Class;
										rdfs:label	"NonOncologicalConsultation";
										rdfs:subClassOf	<http://research.tib.eu/clarify2020/vocab/Observation>;
										rdfs:comment "Represents the first consultation with a non-oncology specialist prior to be diagnosed with cancer.";
										dcterms:modified "2020-10-23"^^xsd:date;
										dcterms:creator <https://www.tib.eu/en/research-development/scientific-data-management/staff/samaneh-jozashoori/>.	

<http://research.tib.eu/clarify2020/vocab/TreatmentLineType>  	rdf:type owl:Class;
							rdfs:label	"TreatmentLineType";
							rdfs:subClassOf	<http://research.tib.eu/clarify2020/vocab/Concept>;
							rdfs:comment "Specification of the treatment line type.";
							dcterms:modified "2021-02-25"^^xsd:date;
							dcterms:creator <https://www.tib.eu/en/research-development/scientific-data-management/staff/samaneh-jozashoori/>.	

<http://research.tib.eu/clarify2020/vocab/TreatementLineBestResponse>  	rdf:type owl:Class;
										rdfs:label	"TreatementLineBestResponse";
										rdfs:subClassOf	<http://research.tib.eu/clarify2020/vocab/Concept>;
										dcterms:modified "2021-02-18"^^xsd:date;
										rdfs:comment "Indicates the best response that a patient has in a treatment line.";
										dcterms:creator <https://www.tib.eu/en/research-development/scientific-data-management/staff/samaneh-jozashoori/>.	

<http://research.tib.eu/clarify2020/vocab/CancerType>  rdf:type owl:Class;
					rdfs:label	"CancerType";
					rdfs:subClassOf	<http://research.tib.eu/clarify2020/vocab/Concept>;
					rdfs:comment "Indicates the type of the cancer.";
					dcterms:modified "2021-02-18"^^xsd:date;
					dcterms:creator <https://www.tib.eu/en/research-development/scientific-data-management/staff/samaneh-jozashoori/>.	

<http://research.tib.eu/clarify2020/vocab/BiomarkerTestResult> rdf:type owl:Class;
						rdfs:label	"BiomarkerTestResult";
						rdfs:subClassOf	<http://research.tib.eu/clarify2020/vocab/Concept>;
						rdfs:comment "Represents the results of a Biomarket test.";
						dcterms:modified "2021-03-02"^^xsd:date;
						dcterms:creator <https://www.tib.eu/en/research-development/scientific-data-management/staff/samaneh-jozashoori/>.	

<http://research.tib.eu/clarify2020/vocab/TreatmentLineNumber> rdf:type owl:Class;
							rdfs:label	"TreatmentLineNumber";
							rdfs:subClassOf	<http://research.tib.eu/clarify2020/vocab/Episode>;
							rdfs:comment "The number representing the oncological line of treatment.";
							dcterms:modified "2021-02-25"^^xsd:date;
							dcterms:creator <https://www.tib.eu/en/research-development/scientific-data-management/staff/samaneh-jozashoori/>.	

<http://research.tib.eu/clarify2020/vocab/Assessment> 	rdf:type owl:Class;
					rdfs:label	"Assessment";
					rdfs:subClassOf	<http://research.tib.eu/clarify2020/vocab/Concept>;
					rdfs:comment "Represents any procedure or technique that is applied in the process of evaluation.";
					dcterms:modified "2021-02-25"^^xsd:date;
					dcterms:creator <https://www.tib.eu/en/research-development/scientific-data-management/staff/samaneh-jozashoori/>.	

<http://research.tib.eu/clarify2020/vocab/TrialType> 	rdf:type owl:Class;
					rdfs:label	"TrialType";
					rdfs:subClassOf	<http://research.tib.eu/clarify2020/vocab/Concept>;
					rdfs:comment "Represents the different trials, that can be directed, drug trial or observational trial."; 
					dcterms:modified "2021-02-25"^^xsd:date;
					dcterms:creator <https://www.tib.eu/en/research-development/scientific-data-management/staff/samaneh-jozashoori/>.	

<http://research.tib.eu/clarify2020/vocab/TrialPhase> 	rdf:type owl:Class;
					rdfs:label	"TrialPhase";
					rdfs:subClassOf	<http://research.tib.eu/clarify2020/vocab/Concept>;
					rdfs:comment "Indicates the phase of the clinical trial.";
					dcterms:modified "2021-02-25"^^xsd:date;
					dcterms:creator <https://www.tib.eu/en/research-development/scientific-data-management/staff/samaneh-jozashoori/>.	

<http://research.tib.eu/clarify2020/vocab/TumorSize> 	rdf:type owl:Class;
					rdfs:label	"TumorSize";
					rdfs:subClassOf	<http://research.tib.eu/clarify2020/vocab/Concept>;
					rdfs:comment "Indicates the size of the patient's tumor (T).";
					dcterms:modified "2021-02-25"^^xsd:date;
					dcterms:creator <https://www.tib.eu/en/research-development/scientific-data-management/staff/samaneh-jozashoori/>.	

<http://research.tib.eu/clarify2020/vocab/FamilyWithCancer> 	rdf:type owl:Class;
							rdfs:label	"FamilyWithCancer";
							rdfs:subClassOf	<http://research.tib.eu/clarify2020/vocab/Concept>;
							rdfs:comment "Represents if the patient has a relative with cancer.";
							dcterms:modified "2021-02-25"^^xsd:date;
							dcterms:creator <https://www.tib.eu/en/research-development/scientific-data-management/staff/samaneh-jozashoori/>.	

<http://research.tib.eu/clarify2020/vocab/FamilyType> 	rdf:type owl:Class;
					rdfs:label	"FamilyType";
					rdfs:subClassOf	<http://research.tib.eu/clarify2020/vocab/Concept>;
					rdfs:comment "Represents the type of family kinship with the patient.";
					dcterms:modified "2021-02-25"^^xsd:date;
					dcterms:creator <https://www.tib.eu/en/research-development/scientific-data-management/staff/samaneh-jozashoori/>.	

<http://research.tib.eu/clarify2020/vocab/FamilyRelationDegree> 	rdf:type owl:Class;
								rdfs:label	"FamilyRelationDegree";
								rdfs:subClassOf	<http://research.tib.eu/clarify2020/vocab/Concept>;
								rdfs:comment "Represents the relative degree of the family member with the patient.";
								dcterms:modified "2021-07-26"^^xsd:date;
								dcterms:creator <https://www.tib.eu/en/research-development/scientific-data-management/staff/samaneh-jozashoori/>.	

<http://research.tib.eu/clarify2020/vocab/CauseOfDeath> 	rdf:type owl:Class;
						rdfs:label	"CauseOfDeath";
						rdfs:subClassOf	<http://research.tib.eu/clarify2020/vocab/Concept>;
						rdfs:comment "Indicates the lung cancer patient's cause of death.";
						dcterms:modified "2021-02-25"^^xsd:date;
						dcterms:creator <https://www.tib.eu/en/research-development/scientific-data-management/staff/samaneh-jozashoori/>.	

<http://research.tib.eu/clarify2020/vocab/ReasonOfDeath> 	rdf:type owl:Class;
						rdfs:label	"ReasonOfDeath";
						rdfs:subClassOf	<http://research.tib.eu/clarify2020/vocab/Concept>;
						rdfs:comment "Indicates the lung cancer patient's reason of death.";
						dcterms:modified "2021-02-25"^^xsd:date;
						dcterms:creator <https://www.tib.eu/en/research-development/scientific-data-management/staff/samaneh-jozashoori/>.	

<http://research.tib.eu/clarify2020/vocab/CurrentStatus> 	rdf:type owl:Class;
						rdfs:label	"CurrentStatus";
						rdfs:subClassOf	<http://research.tib.eu/clarify2020/vocab/Concept>;
						rdfs:comment "Current status of Lung Cancer patient.";
						dcterms:modified "2021-02-25"^^xsd:date;
						dcterms:creator <https://www.tib.eu/en/research-development/scientific-data-management/staff/samaneh-jozashoori/>.	

<http://research.tib.eu/clarify2020/vocab/PatientCancerHistory> 	rdf:type owl:Class;
								rdfs:label	"PatientCancerHistory";
								rdfs:subClassOf	<http://research.tib.eu/clarify2020/vocab/Concept>;
								rdfs:comment "Connection between patient and her/his family history.";
								dcterms:modified "2021-02-25"^^xsd:date;
								dcterms:creator <https://www.tib.eu/en/research-development/scientific-data-management/staff/samaneh-jozashoori/>.	

<http://research.tib.eu/clarify2020/vocab/Hospital> 	rdf:type owl:Class;
					rdfs:label	"Hospital";
					rdfs:subClassOf	<http://research.tib.eu/clarify2020/vocab/Concept>;
					rdfs:comment "Represents in which hospital the patient is hospitalized.";
					dcterms:modified "2021-02-25"^^xsd:date;
					dcterms:creator <https://www.tib.eu/en/research-development/scientific-data-management/staff/samaneh-jozashoori/>.	

<http://research.tib.eu/clarify2020/vocab/City> 	rdf:type owl:Class;
				rdfs:label	"City";
				rdfs:subClassOf	<http://research.tib.eu/clarify2020/vocab/Concept>;
				rdfs:comment  "Represents the city of residence of the patient (structured information provided by HUPHM).";
				dcterms:modified "2021-02-25"^^xsd:date;
				dcterms:creator <https://www.tib.eu/en/research-development/scientific-data-management/staff/samaneh-jozashoori/>.	

<http://research.tib.eu/clarify2020/vocab/Scale> 	rdf:type owl:Class;
				rdfs:label	"Scale";
				rdfs:subClassOf	<http://research.tib.eu/clarify2020/vocab/Assessment>;
				rdfs:comment "Represents the scale that is applied in the evaluation of the patient's performance status.";
				dcterms:modified "2021-02-25"^^xsd:date;
				dcterms:creator <https://www.tib.eu/en/research-development/scientific-data-management/staff/samaneh-jozashoori/>.	

<http://research.tib.eu/clarify2020/vocab/PerformanceStatusObservation> 	rdf:type owl:Class;
										rdfs:label	"PerformanceStatusObservation";
										rdfs:subClassOf	<http://research.tib.eu/clarify2020/vocab/Observation>;
										rdfs:comment "Indicates if the person has previous cancer.";
										dcterms:modified "2021-02-25"^^xsd:date;
										dcterms:creator <https://www.tib.eu/en/research-development/scientific-data-management/staff/samaneh-jozashoori/>.	

<http://research.tib.eu/clarify2020/vocab/PerformedStudyStatus> 	rdf:type owl:Class;
								rdfs:label	"PerformedStudyStatus";
								rdfs:subClassOf	<http://research.tib.eu/clarify2020/vocab/Observation>;
								rdfs:comment "Indicates if a study is performed on the biomarker.";
								dcterms:modified "2021-04-07"^^xsd:date;
								dcterms:creator <https://www.tib.eu/en/research-development/scientific-data-management/staff/samaneh-jozashoori/>.	

<http://research.tib.eu/clarify2020/vocab/RadiotherapyIntention>	rdf:type	owl:Class;
								rdfs:label	"RadiotherapyIntention";
								rdfs:subClassOf	<http://research.tib.eu/clarify2020/vocab/Concept>;
								rdfs:comment "Represents the purpose(!) of performing radiotherapy.";
								dcterms:modified "2021-02-25"^^xsd:date;
								dcterms:creator <https://www.tib.eu/en/research-development/scientific-data-management/staff/samaneh-jozashoori/>.

<http://research.tib.eu/clarify2020/vocab/RadiotherapyLocation>	rdf:type	owl:Class;
								rdfs:label	"RadiotherapyLocation";
								rdfs:subClassOf	<http://research.tib.eu/clarify2020/vocab/OccurrenceLocation>;
								rdfs:comment "Indicates the location of the radiotherapy: bone, holocraneal bone, lung and others.";
								dcterms:modified "2021-02-25"^^xsd:date;
								dcterms:creator <https://www.tib.eu/en/research-development/scientific-data-management/staff/samaneh-jozashoori/>.

<http://research.tib.eu/clarify2020/vocab/ProgressionType>	rdf:type	owl:Class;
						rdfs:label	"ProgressionType";
						rdfs:subClassOf	<http://research.tib.eu/clarify2020/vocab/Concept>;
						rdfs:comment "Represents type of progression that patient has experienced.";
						dcterms:modified "2021-02-25"^^xsd:date;
						dcterms:creator <https://www.tib.eu/en/research-development/scientific-data-management/staff/samaneh-jozashoori/>.

<http://research.tib.eu/clarify2020/vocab/TherapyType>	rdf:type	owl:Class;
					rdfs:label	"TherapyType";
					rdfs:subClassOf	<http://research.tib.eu/clarify2020/vocab/Concept>;
					rdfs:comment "Represents the type of therapy that is prescribed to the patient (active or palliative care -pain relieving-).";
					dcterms:modified "2021-02-25"^^xsd:date;
					dcterms:creator <https://www.tib.eu/en/research-development/scientific-data-management/staff/samaneh-jozashoori/>.

<http://research.tib.eu/clarify2020/vocab/SmokingHabit>	rdf:type	owl:Class;
						rdfs:label	"SmokingHabit";
						rdfs:subClassOf	<http://research.tib.eu/clarify2020/vocab/Concept>;
						rdfs:comment "Represents the smoking habit of the patient and people with whom the patient lives/ lived.";
						dcterms:modified "2021-06-04"^^xsd:date;
						dcterms:creator <https://www.tib.eu/en/research-development/scientific-data-management/staff/samaneh-jozashoori/>.

<http://research.tib.eu/clarify2020/vocab/SmokeEnvironment>	rdf:type	owl:Class;
							rdfs:label	"SmokeEnvironment";
							rdfs:subClassOf	<http://research.tib.eu/clarify2020/vocab/Concept>;
							rdfs:comment "Represents the information about the exposure of the patient to the smoke due to living with smokers.";
							dcterms:modified "2021-02-16"^^xsd:date;
							dcterms:creator <https://www.tib.eu/en/research-development/scientific-data-management/staff/samaneh-jozashoori/>.

<http://research.tib.eu/clarify2020/vocab/LymphNodesInvolvement>	rdf:type	owl:Class;
								rdfs:label	"LymphNodesInvolvement";
								rdfs:subClassOf	<http://research.tib.eu/clarify2020/vocab/Concept>;
								rdfs:comment "Indicates if the lymph nodes are involved (N).";
								dcterms:modified "2021-02-25"^^xsd:date;
								dcterms:creator <https://www.tib.eu/en/research-development/scientific-data-management/staff/samaneh-jozashoori/>.

<http://research.tib.eu/clarify2020/vocab/PerioperativeDeath>	rdf:type	owl:Class;
							rdfs:label	"PerioperativeDeath";
							rdfs:subClassOf	<http://research.tib.eu/clarify2020/vocab/CauseOfDeath>;
							rdfs:comment "Represents if the perioperative death was the cause of death (30 days after surgery)."; 
							dcterms:modified "2021-02-25"^^xsd:date;
							dcterms:creator <https://www.tib.eu/en/research-development/scientific-data-management/staff/samaneh-jozashoori/>.

<http://research.tib.eu/clarify2020/vocab/SurgeryResectionDegree>	rdf:type	owl:Class;
								rdfs:label	"SurgeryResectionDegree";
								rdfs:subClassOf	<http://research.tib.eu/clarify2020/vocab/Concept>;
								rdfs:comment "Indicates the degree of the resection that is applied during the surgery.";							dcterms:modified "2021-02-25"^^xsd:date;
								dcterms:creator <https://www.tib.eu/en/research-development/scientific-data-management/staff/samaneh-jozashoori/>.

<http://research.tib.eu/clarify2020/vocab/SurgeryClass>	rdf:type	owl:Class;
						rdfs:label	"SurgeryClass";
						rdfs:subClassOf	<http://research.tib.eu/clarify2020/vocab/Concept>;
						rdfs:comment "Represents the type of the surgery.";
						dcterms:modified "2021-02-25"^^xsd:date;
						dcterms:creator <https://www.tib.eu/en/research-development/scientific-data-management/staff/samaneh-jozashoori/>.

<http://research.tib.eu/clarify2020/vocab/SurgerySubType>	rdf:type	owl:Class;
						rdfs:label	"SurgerySubType";
						rdfs:subClassOf	<http://research.tib.eu/clarify2020/vocab/Concept>;
						rdfs:comment "Represents the subtype of the surgery.";
						dcterms:modified "2021-02-25"^^xsd:date;
						dcterms:creator <https://www.tib.eu/en/research-development/scientific-data-management/staff/samaneh-jozashoori/>.

<http://research.tib.eu/clarify2020/vocab/MetastatisStage>	rdf:type	owl:Class;
						rdfs:label	"MetastatisStage";
						rdfs:subClassOf	<http://research.tib.eu/clarify2020/vocab/Concept>;
						rdfs:comment "Indicates that to what extend the cancer is metastasized (M).";
						dcterms:modified "2021-02-25"^^xsd:date;
						dcterms:creator <https://www.tib.eu/en/research-development/scientific-data-management/staff/samaneh-jozashoori/>.

<http://research.tib.eu/clarify2020/vocab/SurgeryPathologicalResponse>	rdf:type	owl:Class;
									rdfs:label	"SurgeryPathologicalResponse";
									rdfs:subClassOf	<http://research.tib.eu/clarify2020/vocab/Concept>;
									rdfs:comment "Represents the type of pathological response to the surgery that the patient experienced.";
									dcterms:modified "2021-02-25"^^xsd:date;
									dcterms:creator <https://www.tib.eu/en/research-development/scientific-data-management/staff/samaneh-jozashoori/>.

<http://research.tib.eu/clarify2020/vocab/SynchronousTumor>	rdf:type	owl:Class;
							rdfs:label	"SynchronousTumor";
							rdfs:subClassOf	<http://research.tib.eu/clarify2020/vocab/Concept>;
							rdfs:comment "Represents if a synchronous tumor (a second primary cancer diagnosed within 6 months of the primary cancer) is also discovered.";
							dcterms:modified "2021-02-25"^^xsd:date;
							dcterms:creator <https://www.tib.eu/en/research-development/scientific-data-management/staff/samaneh-jozashoori/>.

<http://research.tib.eu/clarify2020/vocab/HistologyDegree>	rdf:type	owl:Class;
						rdfs:label	"HistologyDegree";
						rdfs:subClassOf	<http://research.tib.eu/clarify2020/vocab/Concept>;
						rdfs:comment "Represents the histology degree.";
						dcterms:modified "2021-02-25"^^xsd:date;
						dcterms:creator <https://www.tib.eu/en/research-development/scientific-data-management/staff/samaneh-jozashoori/>.

<http://research.tib.eu/clarify2020/vocab/AdenocarcinomaHistology>	rdf:type	owl:Class;
								rdfs:label	"AdenocarcinomaHistology";
								rdfs:subClassOf	<http://research.tib.eu/clarify2020/vocab/Concept>;
								rdfs:comment "Represents type of adenocarcinoma (originally developement of the cancer in an organ or gland) experienced by the patient (if any).";
								dcterms:modified "2021-02-25"^^xsd:date;
								dcterms:creator <https://www.tib.eu/en/research-development/scientific-data-management/staff/samaneh-jozashoori/>.

<http://research.tib.eu/clarify2020/vocab/MesotheliomaType>	rdf:type	owl:Class;
							rdfs:label	"MesotheliomaType";
							rdfs:subClassOf	<http://research.tib.eu/clarify2020/vocab/Concept>;
							rdfs:comment "Represents the type of small cell mesothelioma (a malignant tumor that is caused by inhaled asbestos fibers and forms in the lining of the lungs, abdomen or heart) that patient is experienced (if any).";
							dcterms:modified "2021-02-25"^^xsd:date;
							dcterms:creator <https://www.tib.eu/en/research-development/scientific-data-management/staff/samaneh-jozashoori/>.

<http://research.tib.eu/clarify2020/vocab/CarcinomaType>	rdf:type	owl:Class;
						rdfs:label	"CarcinomaType";
						rdfs:subClassOf	<http://research.tib.eu/clarify2020/vocab/Concept>;
						rdfs:comment "Represents the type of carcinoma that the patient is experienced.";
						dcterms:modified "2021-02-25"^^xsd:date;
						dcterms:creator <https://www.tib.eu/en/research-development/scientific-data-management/staff/samaneh-jozashoori/>.

<http://research.tib.eu/clarify2020/vocab/SmallCellCarcinomaType>	rdf:type	owl:Class;
								rdfs:label	"SmallCellCarcinomaType";
								rdfs:subClassOf	<http://research.tib.eu/clarify2020/vocab/Concept>;
								rdfs:comment "Represents the type of small cell carcinoma that patient is experienced (if any).";
								dcterms:modified "2021-02-25"^^xsd:date;
								dcterms:creator <https://www.tib.eu/en/research-development/scientific-data-management/staff/samaneh-jozashoori/>.

<http://research.tib.eu/clarify2020/vocab/SecondNeoplasm>	rdf:type        owl:Class;	
						rdfs:label	"SecondNeoplasm";
						rdfs:subClassOf	<http://research.tib.eu/clarify2020/vocab/Concept>;
						rdfs:comment "Secondary malignant neoplasm is a malignant tumor whose cause is the treatment (usually radiation or chemotherapy) which was used for a prior tumor.";
						dcterms:modified "2021-03-18"^^xsd:date;
						dcterms:creator <https://www.tib.eu/en/research-development/scientific-data-management/staff/samaneh-jozashoori/>.

<http://research.tib.eu/clarify2020/vocab/Version>	rdf:type        owl:Class;	
				rdfs:label	"Version";
				rdfs:subClassOf	<http://research.tib.eu/clarify2020/vocab/Concept>;
				rdfs:comment "Indicates the versioning of a concept.";
				dcterms:modified "2021-04-26"^^xsd:date;
				dcterms:creator <https://www.tib.eu/en/research-development/scientific-data-management/staff/samaneh-jozashoori/>.

<http://research.tib.eu/clarify2020/vocab/PerformedMonitoring>	rdf:type        owl:Class;	
							rdfs:label	"PerformedMonitoring";
							rdfs:subClassOf	<http://research.tib.eu/clarify2020/vocab/Concept>;
							rdfs:comment "Indicates performed monitoring.";
							dcterms:modified "2021-04-29"^^xsd:date;
							dcterms:creator <https://www.tib.eu/en/research-development/scientific-data-management/staff/samaneh-jozashoori/>.

<http://research.tib.eu/clarify2020/vocab/SurgeryIteration>	rdf:type        owl:Class;	
							rdfs:label	"SurgeryIteration";
							rdfs:subClassOf	<http://research.tib.eu/clarify2020/vocab/Concept>;
							rdfs:comment "Indicates surgery iteration.";
							dcterms:modified "2021-05-17"^^xsd:date;
							dcterms:creator <https://www.tib.eu/en/research-development/scientific-data-management/staff/samaneh-jozashoori/>.

<http://research.tib.eu/clarify2020/vocab/PatientIdentifier>	rdf:type        owl:Class;	
							rdfs:label	"PatientIdentifier";
							rdfs:subClassOf	<http://research.tib.eu/clarify2020/vocab/Concept>;
							rdfs:comment "A unique identifier of patients.";
							dcterms:modified "2021-11-17"^^xsd:date;
							dcterms:creator <https://www.tib.eu/en/research-development/scientific-data-management/staff/samaneh-jozashoori/>.

<http://research.tib.eu/clarify2020/vocab/PatientCategory>	rdf:type        owl:Class;	
							rdfs:label	"PatientCategory";
							rdfs:subClassOf	<http://research.tib.eu/clarify2020/vocab/Concept>;
							rdfs:comment "The patient categories provided by the physicians at HUPHM.";
							dcterms:modified "2021-11-17"^^xsd:date;
							dcterms:creator <https://www.tib.eu/en/research-development/scientific-data-management/staff/samaneh-jozashoori/>.

<http://research.tib.eu/clarify2020/vocab/ParentWithCancer>	rdf:type        owl:Class;	
							rdfs:label	"ParentWithCancer";
							rdfs:subClassOf	<http://research.tib.eu/clarify2020/vocab/Concept>;
							rdfs:comment "Represents the cancer history of the parents of the patients.";
							dcterms:modified "2021-11-17"^^xsd:date;
							dcterms:creator <https://www.tib.eu/en/research-development/scientific-data-management/staff/samaneh-jozashoori/>.

<http://research.tib.eu/clarify2020/vocab/Gravidity>	rdf:type        owl:Class;	
					rdfs:label	"Gravidity";
					rdfs:subClassOf	<http://research.tib.eu/clarify2020/vocab/Concept>;
					rdfs:comment "Represents the total number of all pregnancies that patient had experienced.";
					dcterms:modified "2021-11-17"^^xsd:date;
					dcterms:creator <https://www.tib.eu/en/research-development/scientific-data-management/staff/samaneh-jozashoori/>.

<http://research.tib.eu/clarify2020/vocab/Parity>	rdf:type        owl:Class;	
				rdfs:label	"Parity";
				rdfs:subClassOf	<http://research.tib.eu/clarify2020/vocab/Concept>;
				rdfs:comment "Represents the number of times that the patient had given birth to a fetus with a gestational age of 24 weeks or more.";
				dcterms:modified "2021-11-17"^^xsd:date;
				dcterms:creator <https://www.tib.eu/en/research-development/scientific-data-management/staff/samaneh-jozashoori/>.

<http://research.tib.eu/clarify2020/vocab/MenopauseAge>	rdf:type        owl:Class;	
						rdfs:label	"MenopauseAge";
						rdfs:subClassOf	<http://research.tib.eu/clarify2020/vocab/Concept>;
						rdfs:comment "Represents the age at which the patient had experienced her menopause (defined as the final menstrual period and is confirmed when the woman has not had her period for 12 consecutive months).";
						dcterms:modified "2021-11-17"^^xsd:date;
						dcterms:creator <https://www.tib.eu/en/research-development/scientific-data-management/staff/samaneh-jozashoori/>.

<http://research.tib.eu/clarify2020/vocab/MenarcheAge>	rdf:type        owl:Class;	
					rdfs:label	"MenarcheAge";
					rdfs:subClassOf	<http://research.tib.eu/clarify2020/vocab/Concept>;
					rdfs:comment "Represents the age at which the patient had experienced her menarche (defined as the first menstrual period).";
					dcterms:modified "2021-11-17"^^xsd:date;
					dcterms:creator <https://www.tib.eu/en/research-development/scientific-data-management/staff/samaneh-jozashoori/>.

<http://research.tib.eu/clarify2020/vocab/MenopauseStage>	rdf:type        owl:Class;	
						rdfs:label	"MenopauseStage";
						rdfs:subClassOf	<http://research.tib.eu/clarify2020/vocab/Concept>;
						rdfs:comment "Represents the stage of the patient in terms of menopause.";
						dcterms:modified "2021-11-17"^^xsd:date;
						dcterms:creator <https://www.tib.eu/en/research-development/scientific-data-management/staff/samaneh-jozashoori/>.

<http://research.tib.eu/clarify2020/vocab/Contraceptive>	rdf:type        owl:Class;	
						rdfs:label	"Contraceptive";
						rdfs:subClassOf	<http://research.tib.eu/clarify2020/vocab/Concept>;
						rdfs:comment "Represents the method of contraception.";
						dcterms:modified "2021-11-17"^^xsd:date;
						dcterms:creator <https://www.tib.eu/en/research-development/scientific-data-management/staff/samaneh-jozashoori/>.

<http://research.tib.eu/clarify2020/vocab/TumorTypeCategory>	rdf:type	owl:Class;
							rdfs:subClassOf <http://research.tib.eu/clarify2020/vocab/Concept>;
							rdfs:label	"TumorTypeCategory";
							rdfs:comment "Represents the category of the tumor type.";
							dcterms:modified "2021-11-17"^^xsd:date;
							dcterms:creator <https://www.tib.eu/en/research-development/scientific-data-management/staff/samaneh-jozashoori/>.	

<http://research.tib.eu/clarify2020/vocab/BiomarkerObservation>	rdf:type	owl:Class;
								rdfs:subClassOf <http://research.tib.eu/clarify2020/vocab/Concept>;
								rdfs:label	"BiomarkerObservation";
								rdfs:comment "Represents all the tests and results related to each biomarker study on the patient.";
								dcterms:modified "2021-11-24"^^xsd:date;
								dcterms:creator <https://www.tib.eu/en/research-development/scientific-data-management/staff/samaneh-jozashoori/>.	

<http://research.tib.eu/clarify2020/vocab/Event>	rdf:type	owl:Class;
				rdfs:subClassOf <http://research.tib.eu/clarify2020/vocab/Concept>;
				rdfs:label	"Event";
				rdfs:comment "The fundamental entity of observed physical reality represented by a point designated by three coordinates of place and one of time.";
				dcterms:modified "2022-09-12"^^xsd:date;
				dcterms:creator <https://www.tib.eu/en/research-development/scientific-data-management/staff/samaneh-jozashoori/>.	

<http://research.tib.eu/clarify2020/vocab/OncologicalProcedure>	rdf:type	owl:Class;
								rdfs:subClassOf <http://research.tib.eu/clarify2020/vocab/Event>;
								rdfs:label	"OncologicalProcedure";
								rdfs:comment "Any oncological event impacting on the status of the patient.";
								dcterms:modified "2022-09-12"^^xsd:date;
								dcterms:creator <https://www.tib.eu/en/research-development/scientific-data-management/staff/samaneh-jozashoori/>.	

<http://research.tib.eu/clarify2020/vocab/OncologicalAssessment>	rdf:type	owl:Class;
								rdfs:subClassOf <http://research.tib.eu/clarify2020/vocab/Event>;
								rdfs:label	"OncologicalAssessment";
								rdfs:comment "Any oncological event involving an assessment examination or observation.";
								dcterms:modified "2022-09-12"^^xsd:date;
								dcterms:creator <https://www.tib.eu/en/research-development/scientific-data-management/staff/samaneh-jozashoori/>.	

<http://research.tib.eu/clarify2020/vocab/Episode>	rdf:type	owl:Class;
				rdfs:subClassOf <http://research.tib.eu/clarify2020/vocab/Concept>;
				rdfs:label	"Episode";
				rdfs:comment "Indicates the episode of an oncological procedure..";
				dcterms:modified "2022-09-12"^^xsd:date;
				dcterms:creator <https://www.tib.eu/en/research-development/scientific-data-management/staff/samaneh-jozashoori/>.	

<http://research.tib.eu/clarify2020/vocab/TreatmentEpisode>	rdf:type	owl:Class;
							rdfs:subClassOf <http://research.tib.eu/clarify2020/vocab/OncologicalProcedure>;
							rdfs:label	"TreatmentEpisode";
							rdfs:comment "Any oncological event impacting on the status of the patient.";
							dcterms:modified "2022-09-12"^^xsd:date;
							dcterms:creator <https://www.tib.eu/en/research-development/scientific-data-management/staff/samaneh-jozashoori/>.	

<http://research.tib.eu/clarify2020/vocab/Treatment>	rdf:type	owl:Class;
						rdfs:subClassOf <http://research.tib.eu/clarify2020/vocab/Concept>;
						rdfs:label	"Treatment";
						rdfs:comment "Represents the general category of the treatments exist for cancers.";
						dcterms:modified "2022-09-12"^^xsd:date;
						dcterms:creator <https://www.tib.eu/en/research-development/scientific-data-management/staff/samaneh-jozashoori/>.	

<http://research.tib.eu/clarify2020/vocab/Chemotherapy>	rdf:type	owl:Class;
						rdfs:subClassOf <http://research.tib.eu/clarify2020/vocab/Treatment>;
						rdfs:label	"Chemotherapy";
						rdfs:comment "Represents the chemotherapy treatment for cancer patients.";
						dcterms:modified "2022-09-12"^^xsd:date;
						dcterms:creator <https://www.tib.eu/en/research-development/scientific-data-management/staff/samaneh-jozashoori/>.	

<http://research.tib.eu/clarify2020/vocab/Radiotherapy>	rdf:type	owl:Class;
						rdfs:subClassOf <http://research.tib.eu/clarify2020/vocab/Treatment>;
						rdfs:label	"Radiotherapy";
						rdfs:comment "Represents the radiotherapy treatment for cancer patients.";
						dcterms:modified "2022-09-12"^^xsd:date;
						dcterms:creator <https://www.tib.eu/en/research-development/scientific-data-management/staff/samaneh-jozashoori/>.	

<http://research.tib.eu/clarify2020/vocab/HormonalTherapy>	rdf:type	owl:Class;
						rdfs:subClassOf <http://research.tib.eu/clarify2020/vocab/Treatment>;
						rdfs:label	"HormonalTherapy";
						rdfs:comment "Represents the hormonal therapy for cancer patients.";
						dcterms:modified "2022-09-12"^^xsd:date;
						dcterms:creator <https://www.tib.eu/en/research-development/scientific-data-management/staff/samaneh-jozashoori/>.	

<http://research.tib.eu/clarify2020/vocab/Immunotherapy>	rdf:type	owl:Class;
						rdfs:subClassOf <http://research.tib.eu/clarify2020/vocab/Treatment>;
						rdfs:label	"Immunotherapy";
						rdfs:comment "Represents the immunotherapy treatment for cancer patients.";
						dcterms:modified "2022-09-12"^^xsd:date;
						dcterms:creator <https://www.tib.eu/en/research-development/scientific-data-management/staff/samaneh-jozashoori/>.	

<http://research.tib.eu/clarify2020/vocab/RadiotherapyRound>	rdf:type	owl:Class;
							rdfs:subClassOf <http://research.tib.eu/clarify2020/vocab/Episode>;
							rdfs:label	"RadiotherapyRound";
							rdfs:comment "Indicates the occurrence number of the radiotherapy.";
							dcterms:modified "2022-09-12"^^xsd:date;
							dcterms:creator <https://www.tib.eu/en/research-development/scientific-data-management/staff/samaneh-jozashoori/>.	

<http://research.tib.eu/clarify2020/vocab/ProgressionRelapseAssessment>	rdf:type	owl:Class;
										rdfs:subClassOf <http://research.tib.eu/clarify2020/vocab/OncologicalAssessment>;
										rdfs:label	"ProgressionRelapseAssessment";
										rdfs:comment "The assessment of the progression and relapse.";
										dcterms:modified "2022-09-12"^^xsd:date;
										dcterms:creator <https://www.tib.eu/en/research-development/scientific-data-management/staff/samaneh-jozashoori/>.	

<http://research.tib.eu/clarify2020/vocab/TNMstageAssessment>	rdf:type	owl:Class;
							rdfs:subClassOf <http://research.tib.eu/clarify2020/vocab/OncologicalAssessment>;
							rdfs:label	"TNMstageAssessment";
							rdfs:comment "The assessment of the cancer stage based on TNM staging system.";
							dcterms:modified "2022-09-12"^^xsd:date;
							dcterms:creator <https://www.tib.eu/en/research-development/scientific-data-management/staff/samaneh-jozashoori/>.	

<http://research.tib.eu/clarify2020/vocab/TumorHistologyAssessment>	rdf:type	owl:Class;
									rdfs:subClassOf <http://research.tib.eu/clarify2020/vocab/OncologicalAssessment>;
									rdfs:label	"TumorHistologyAssessment";
									rdfs:comment "The assessment of the histology of the tumor.";
									dcterms:modified "2022-09-12"^^xsd:date;
									dcterms:creator <https://www.tib.eu/en/research-development/scientific-data-management/staff/samaneh-jozashoori/>.	

<http://research.tib.eu/clarify2020/vocab/TNMstage>	rdf:type	owl:Class;
					rdfs:subClassOf <http://research.tib.eu/clarify2020/vocab/Concept>;
					rdfs:label	"TNMstage";
					rdfs:comment "A measurement system assessing the stage of the cancer based on the tumor size (T), Lymph nodes involvement (N), and the metastasis (M).";
					dcterms:modified "2022-09-12"^^xsd:date;
					dcterms:creator <https://www.tib.eu/en/research-development/scientific-data-management/staff/samaneh-jozashoori/>.	

<http://research.tib.eu/clarify2020/vocab/OncologicalSurgeryIteration>	rdf:type	owl:Class;
									rdfs:subClassOf <http://research.tib.eu/clarify2020/vocab/Concept>;
									rdfs:label	"OncologicalSurgeryIteration";
									rdfs:comment "Represents the iteration of a specific oncological surgery.";
									dcterms:modified "2022-09-12"^^xsd:date;
									dcterms:creator <https://www.tib.eu/en/research-development/scientific-data-management/staff/samaneh-jozashoori/>.	

<http://research.tib.eu/clarify2020/vocab/TreatmentLineCycle>	rdf:type	owl:Class;
							rdfs:subClassOf <http://research.tib.eu/clarify2020/vocab/Episode>;
							rdfs:label	"TreatmentLineCycle";
							rdfs:comment "Represents the iteration of a specific treatment.";
							dcterms:modified "2022-09-12"^^xsd:date;
							dcterms:creator <https://www.tib.eu/en/research-development/scientific-data-management/staff/samaneh-jozashoori/>.	

<http://research.tib.eu/clarify2020/vocab/OncologicalTreatmentLine>	rdf:type	owl:Class;
									rdfs:subClassOf <http://research.tib.eu/clarify2020/vocab/Episode>;
									rdfs:label	"OncologicalTreatmentLine";
									rdfs:comment "Represents the line of a specific treatment.";
									dcterms:modified "2023-01-11"^^xsd:date;
									dcterms:creator <https://www.tib.eu/en/research-development/scientific-data-management/staff/samaneh-jozashoori/>.	

######################################################################################################################################
#####################################################    Publication    ##############################################################
######################################################################################################################################

<http://research.tib.eu/clarify2020/vocab/Publication>	rdf:type	owl:Class;
					rdfs:label	"Publication";
					rdfs:subClassOf	<http://research.tib.eu/clarify2020/vocab/Concept>;
					rdfs:comment "Scientific publications.";
					dcterms:modified "2020-12-15"^^xsd:date;
					dcterms:creator <https://www.tib.eu/en/research-development/scientific-data-management/staff/samaneh-jozashoori/>.

<http://research.tib.eu/clarify2020/vocab/Author>	rdf:type	owl:Class;
				rdfs:label	"Author";
				rdfs:subClassOf	<http://research.tib.eu/clarify2020/vocab/Concept>;
				rdfs:comment "Author of Scientific publications.";
				dcterms:modified "2021-05-17"^^xsd:date;
				dcterms:creator <https://www.tib.eu/en/research-development/scientific-data-management/staff/samaneh-jozashoori/>.

<http://research.tib.eu/clarify2020/vocab/Relation>	rdf:type	owl:Class;
					rdfs:label	"Relation";
					rdfs:subClassOf	<http://research.tib.eu/clarify2020/vocab/Concept>;
					rdfs:comment "Defines relationship between UMLS concepts.";
					dcterms:modified "2021-01-26"^^xsd:date;
					dcterms:creator <https://www.tib.eu/en/research-development/scientific-data-management/staff/samaneh-jozashoori/>.

<http://research.tib.eu/clarify2020/vocab/PublicationType>	rdf:type	owl:Class;
						rdfs:label	"PublicationType";
						rdfs:subClassOf	<http://research.tib.eu/clarify2020/vocab/Concept>;
						rdfs:comment "Defines the type of publication.";
						dcterms:modified "2021-06-08"^^xsd:date;
						dcterms:creator <https://www.tib.eu/en/research-development/scientific-data-management/staff/samaneh-jozashoori/>.

<http://research.tib.eu/clarify2020/vocab/AFFECTS>	rdf:type	owl:Class;
					rdfs:label	"AFFECTS";
					rdfs:subClassOf	<http://research.tib.eu/clarify2020/vocab/Relation>;
					rdfs:comment "Relation between two UMLS CUIs to represent pharmacogenomics; it implies a direct effect on.";
					dcterms:modified "2021-01-26"^^xsd:date;
					dcterms:creator <https://www.tib.eu/en/research-development/scientific-data-management/staff/samaneh-jozashoori/>.

<http://research.tib.eu/clarify2020/vocab/ASSOCIATED_WITH>	rdf:type	owl:Class;
					rdfs:label	"ASSOCIATED_WITH";
					rdfs:subClassOf	<http://research.tib.eu/clarify2020/vocab/Relation>;
					rdfs:comment "Relation between UMLS CUIs to represent the genetic etiology of disease; the relation is of type association between two terms.";
					dcterms:modified "2021-01-26"^^xsd:date;
					dcterms:creator <https://www.tib.eu/en/research-development/scientific-data-management/staff/samaneh-jozashoori/>.

<http://research.tib.eu/clarify2020/vocab/AUGMENTS>	rdf:type	owl:Class;
					rdfs:label	"AUGMENTS";
					rdfs:subClassOf	<http://research.tib.eu/clarify2020/vocab/Relation>;
					rdfs:comment "Relation between two UMLS CUIs to represent pharmacogenomics. It implies expanding or stimulating a process.";
					dcterms:modified "2021-01-26"^^xsd:date;
					dcterms:creator <https://www.tib.eu/en/research-development/scientific-data-management/staff/samaneh-jozashoori/>.

<http://research.tib.eu/clarify2020/vocab/CAUSES>	rdf:type	owl:Class;
					rdfs:label	"CAUSES";
					rdfs:subClassOf	<http://research.tib.eu/clarify2020/vocab/Relation>;
					rdfs:comment "Relation between two UMLS CUIs to represent the genetic etiology of disease; it implies bringing about a condition or an effect.";
					dcterms:modified "2021-01-26"^^xsd:date;
					dcterms:creator <https://www.tib.eu/en/research-development/scientific-data-management/staff/samaneh-jozashoori/>.

<http://research.tib.eu/clarify2020/vocab/COEXISTS_WITH>	rdf:type	owl:Class;
					rdfs:label	"COEXISTS_WITH";
					rdfs:subClassOf	<http://research.tib.eu/clarify2020/vocab/Relation>;
					rdfs:comment "Relation between two UMLS CUIs to represent the genetic etiology of disease; it implies occurring together with, or jointly.";
					dcterms:modified "2021-01-26"^^xsd:date;
					dcterms:creator <https://www.tib.eu/en/research-development/scientific-data-management/staff/samaneh-jozashoori/>.

<http://research.tib.eu/clarify2020/vocab/COMPLICATES>	rdf:type	owl:Class;
					rdfs:label	"COMPLICATES";
					rdfs:subClassOf	<http://research.tib.eu/clarify2020/vocab/Relation>;
					rdfs:comment "Relation between two UMLS CUIs to represent the genetic etiology of disease; it represents causes to become more severe or complex, or results in adverse effects.";
					dcterms:modified "2021-01-26"^^xsd:date;
					dcterms:creator <https://www.tib.eu/en/research-development/scientific-data-management/staff/samaneh-jozashoori/>.

<http://research.tib.eu/clarify2020/vocab/CONVERTS_TO>	rdf:type	owl:Class;
					rdfs:label	"CONVERTS_TO";
					rdfs:subClassOf	<http://research.tib.eu/clarify2020/vocab/Relation>;
					rdfs:comment "Relation between two UMLS CUIs to represent the genetic etiology of disease; it implies changing from one form to another.";
					dcterms:modified "2021-01-26"^^xsd:date;
					dcterms:creator <https://www.tib.eu/en/research-development/scientific-data-management/staff/samaneh-jozashoori/>.

<http://research.tib.eu/clarify2020/vocab/DIAGNOSES>	rdf:type	owl:Class;
					rdfs:label	"DIAGNOSES";
					rdfs:subClassOf	<http://research.tib.eu/clarify2020/vocab/Relation>;
					rdfs:comment "Relation between two UMLS CUIs that represents the relation of type distinguishing or identifying the nature or characteristics of two clinical medicine terms.";
					dcterms:modified "2021-01-26"^^xsd:date;
					dcterms:creator <https://www.tib.eu/en/research-development/scientific-data-management/staff/samaneh-jozashoori/>.

<http://research.tib.eu/clarify2020/vocab/DISRUPTS>	rdf:type	owl:Class;
					rdfs:label	"DISRUPTS";
					rdfs:subClassOf	<http://research.tib.eu/clarify2020/vocab/Relation>;
					rdfs:comment "Relation between UMLS CUIs to represent pharmacogenomics; the relation is of type altering or influencing an already existing condition, state, or situation and producing a negative effect on between two terms.";
					dcterms:modified "2021-01-26"^^xsd:date;
					dcterms:creator <https://www.tib.eu/en/research-development/scientific-data-management/staff/samaneh-jozashoori/>.

<http://research.tib.eu/clarify2020/vocab/INHIBITS>	rdf:type	owl:Class;
					rdfs:label	"INHIBITS";
					rdfs:subClassOf	<http://research.tib.eu/clarify2020/vocab/Relation>;
					rdfs:comment "Relation between two UMLS CUIs that describes substance interactions in terms of decreasing, limiting, or blocks the action or function.";
					dcterms:modified "2021-01-26"^^xsd:date;
					dcterms:creator <https://www.tib.eu/en/research-development/scientific-data-management/staff/samaneh-jozashoori/>.

<http://research.tib.eu/clarify2020/vocab/INTERACTS_WITH>	rdf:type	owl:Class;
					rdfs:label	"INTERACTS_WITH";
					rdfs:subClassOf	<http://research.tib.eu/clarify2020/vocab/Relation>;
					rdfs:comment "Relation between UMLS CUIs that describes interactions between two terms representing substances.";
					dcterms:modified "2021-01-26"^^xsd:date;
					dcterms:creator <https://www.tib.eu/en/research-development/scientific-data-management/staff/samaneh-jozashoori/>.

<http://research.tib.eu/clarify2020/vocab/ISA>	rdf:type	owl:Class;
					rdfs:label	"ISA";
					rdfs:subClassOf	<http://research.tib.eu/clarify2020/vocab/Relation>;
					rdfs:comment "Relation between two UMLS CUIs that represents that if one item has this relation to another item then the first item is more specific in meaning than the second item.";
					dcterms:modified "2021-01-26"^^xsd:date;
					dcterms:creator <https://www.tib.eu/en/research-development/scientific-data-management/staff/samaneh-jozashoori/>.

<http://research.tib.eu/clarify2020/vocab/LOCATION_OF>	rdf:type	owl:Class;
					rdfs:label	"LOCATION_OF";
					rdfs:subClassOf	<http://research.tib.eu/clarify2020/vocab/Relation>;
					rdfs:comment "The position, site, or region of an entity or the site of a process.";
					dcterms:modified "2021-01-26"^^xsd:date;
					dcterms:creator <https://www.tib.eu/en/research-development/scientific-data-management/staff/samaneh-jozashoori/>.

<http://research.tib.eu/clarify2020/vocab/MANIFESTATION_OF>	rdf:type	owl:Class;
					rdfs:label	"MANIFESTATION_OF";
					rdfs:subClassOf	<http://research.tib.eu/clarify2020/vocab/Relation>;
					rdfs:comment "Relation between two UMLS CUIs that represents that part of a phenomenon which is directly observable or concretely or visibly expressed, or which gives evidence to the underlying process.";
					dcterms:modified "2021-01-26"^^xsd:date;
					dcterms:creator <https://www.tib.eu/en/research-development/scientific-data-management/staff/samaneh-jozashoori/>.

<http://research.tib.eu/clarify2020/vocab/MEASUREMENT_OF>	rdf:type	owl:Class;
					rdfs:label	"MEASUREMENT_OF";
					rdfs:subClassOf	<http://research.tib.eu/clarify2020/vocab/Relation>;
					rdfs:comment "Relation between UMLS CUIs that represents the relation of type measurement between two terms.";
					dcterms:modified "2021-01-26"^^xsd:date;
					dcterms:creator <https://www.tib.eu/en/research-development/scientific-data-management/staff/samaneh-jozashoori/>.										

<http://research.tib.eu/clarify2020/vocab/MEASURES>	rdf:type	owl:Class;
					rdfs:label	"MEASURES";
					rdfs:subClassOf	<http://research.tib.eu/clarify2020/vocab/Relation>;
					rdfs:comment "Relation between UMLS CUIs that represents the relation of type measurement  between two terms.";
					dcterms:modified "2021-01-26"^^xsd:date;
					dcterms:creator <https://www.tib.eu/en/research-development/scientific-data-management/staff/samaneh-jozashoori/>.

<http://research.tib.eu/clarify2020/vocab/METHOD_OF>	rdf:type	owl:Class;
					rdfs:label	"METHOD_OF";
					rdfs:subClassOf	<http://research.tib.eu/clarify2020/vocab/Relation>;
					rdfs:comment "Relation between two UMLS CUIs that represents the manner and sequence of events in performing an act or procedure.";
					dcterms:modified "2021-01-26"^^xsd:date;
					dcterms:creator <https://www.tib.eu/en/research-development/scientific-data-management/staff/samaneh-jozashoori/>.					

<http://research.tib.eu/clarify2020/vocab/NEG_ADMINISTERED_TO>	rdf:type	owl:Class;
					rdfs:label	"NEG_ADMINISTERED_TO";
					rdfs:subClassOf	<http://research.tib.eu/clarify2020/vocab/Relation>;
					rdfs:comment "Relation between two UMLS CUIs that represents the negation of ADMINISTERED_TO relation.";
					dcterms:modified "2021-01-26"^^xsd:date;
					dcterms:creator <https://www.tib.eu/en/research-development/scientific-data-management/staff/samaneh-jozashoori/>.

<http://research.tib.eu/clarify2020/vocab/NEG_AFFECTS>	rdf:type	owl:Class;
					rdfs:label	"NEG_AFFECTS";
					rdfs:subClassOf	<http://research.tib.eu/clarify2020/vocab/Relation>;
					rdfs:comment "Relation between two UMLS CUIs to represent pharmacogenomics; it implies a direct effect on.";
					dcterms:modified "2021-01-26"^^xsd:date;
					dcterms:creator <https://www.tib.eu/en/research-development/scientific-data-management/staff/samaneh-jozashoori/>.

<http://research.tib.eu/clarify2020/vocab/NEG_ASSOCIATED_WITH>	rdf:type	owl:Class;
					rdfs:label	"NEG_ASSOCIATED_WITH";
					rdfs:subClassOf	<http://research.tib.eu/clarify2020/vocab/Relation>;
					rdfs:comment "Relation between UMLS CUIs to represent the genetic etiology of disease; the relation is of type association between two terms.";
					dcterms:modified "2021-01-26"^^xsd:date;
					dcterms:creator <https://www.tib.eu/en/research-development/scientific-data-management/staff/samaneh-jozashoori/>.

<http://research.tib.eu/clarify2020/vocab/NEG_AUGMENTS>	rdf:type	owl:Class;
					rdfs:label	"NEG_AUGMENTS";
					rdfs:subClassOf	<http://research.tib.eu/clarify2020/vocab/Relation>;
					rdfs:comment "Relation between two UMLS CUIs that represents the negation of AUGMENTS relation.";
					dcterms:modified "2021-01-26"^^xsd:date;
					dcterms:creator <https://www.tib.eu/en/research-development/scientific-data-management/staff/samaneh-jozashoori/>.

<http://research.tib.eu/clarify2020/vocab/NEG_CAUSES>	rdf:type	owl:Class;
					rdfs:label	"NEG_CAUSES";
					rdfs:subClassOf	<http://research.tib.eu/clarify2020/vocab/Relation>;
					rdfs:comment "Relation between two UMLS CUIs that represents the negation of CAUSES relation.";
					dcterms:modified "2021-01-26"^^xsd:date;
					dcterms:creator <https://www.tib.eu/en/research-development/scientific-data-management/staff/samaneh-jozashoori/>.

<http://research.tib.eu/clarify2020/vocab/NEG_COEXISTS_WITH>	rdf:type	owl:Class;
					rdfs:label	"NEG_COEXISTS_WITH";
					rdfs:subClassOf	<http://research.tib.eu/clarify2020/vocab/Relation>;
					rdfs:comment "Relation between two UMLS CUIs that represents the negation of COEXISTS_WITH relation.";
					dcterms:modified "2021-01-26"^^xsd:date;
					dcterms:creator <https://www.tib.eu/en/research-development/scientific-data-management/staff/samaneh-jozashoori/>.

<http://research.tib.eu/clarify2020/vocab/NEG_COMPLICATES>	rdf:type	owl:Class;
					rdfs:label	"NEG_COMPLICATES";
					rdfs:subClassOf	<http://research.tib.eu/clarify2020/vocab/Relation>;
					rdfs:comment "Relation between two UMLS CUIs that represents the negation of COMPLICATES relation.";
					dcterms:modified "2021-01-26"^^xsd:date;
					dcterms:creator <https://www.tib.eu/en/research-development/scientific-data-management/staff/samaneh-jozashoori/>.

<http://research.tib.eu/clarify2020/vocab/NEG_CONVERTS_TO>	rdf:type	owl:Class;
					rdfs:label	"NEG_CONVERTS_TO";
					rdfs:subClassOf	<http://research.tib.eu/clarify2020/vocab/Relation>;
					rdfs:comment "Relation between two UMLS CUIs that represents the negation of CONVERTS_TO relation.";
					dcterms:modified "2021-01-26"^^xsd:date;
					dcterms:creator <https://www.tib.eu/en/research-development/scientific-data-management/staff/samaneh-jozashoori/>.

<http://research.tib.eu/clarify2020/vocab/NEG_DIAGNOSES>	rdf:type	owl:Class;
					rdfs:label	"NEG_DIAGNOSES";
					rdfs:subClassOf	<http://research.tib.eu/clarify2020/vocab/Relation>;
					rdfs:comment "Relation between two UMLS CUIs that represents the negation of DIAGNOSES relation.";
					dcterms:modified "2021-01-26"^^xsd:date;
					dcterms:creator <https://www.tib.eu/en/research-development/scientific-data-management/staff/samaneh-jozashoori/>.

<http://research.tib.eu/clarify2020/vocab/NEG_DISRUPTS>	rdf:type	owl:Class;
					rdfs:label	"NEG_DISRUPTS";
					rdfs:subClassOf	<http://research.tib.eu/clarify2020/vocab/Relation>;
					rdfs:comment "Relation between two UMLS CUIs that represents the negation of DISRUPTS relation.";
					dcterms:modified "2021-01-26"^^xsd:date;
					dcterms:creator <https://www.tib.eu/en/research-development/scientific-data-management/staff/samaneh-jozashoori/>.

<http://research.tib.eu/clarify2020/vocab/NEG_INHIBITS>	rdf:type	owl:Class;
					rdfs:label	"NEG_INHIBITS";
					rdfs:subClassOf	<http://research.tib.eu/clarify2020/vocab/Relation>;
					rdfs:comment "Relation between two UMLS CUIs that represents the negation of INHIBITS relation.";
					dcterms:modified "2021-01-26"^^xsd:date;
					dcterms:creator <https://www.tib.eu/en/research-development/scientific-data-management/staff/samaneh-jozashoori/>.

<http://research.tib.eu/clarify2020/vocab/NEG_INTERACTS_WITH>	rdf:type	owl:Class;
					rdfs:label	"NEG_INTERACTS_WITH";
					rdfs:subClassOf	<http://research.tib.eu/clarify2020/vocab/Relation>;
					rdfs:comment "Relation between two UMLS CUIs that represents the negation of INTERACTS_WITH relation.";
					dcterms:modified "2021-01-26"^^xsd:date;
					dcterms:creator <https://www.tib.eu/en/research-development/scientific-data-management/staff/samaneh-jozashoori/>.

<http://research.tib.eu/clarify2020/vocab/NEG_ISA>	rdf:type	owl:Class;
					rdfs:label	"NEG_ISA";
					rdfs:subClassOf	<http://research.tib.eu/clarify2020/vocab/Relation>;
					rdfs:comment "Relation between two UMLS CUIs that represents the negation of ISA relation.";
					dcterms:modified "2021-01-26"^^xsd:date;
					dcterms:creator <https://www.tib.eu/en/research-development/scientific-data-management/staff/samaneh-jozashoori/>.

<http://research.tib.eu/clarify2020/vocab/NEG_LOCATION_OF>	rdf:type	owl:Class;
					rdfs:label	"NEG_LOCATION_OF";
					rdfs:subClassOf	<http://research.tib.eu/clarify2020/vocab/Relation>;
					rdfs:comment "Relation between two UMLS CUIs that represents the negation of LOCATION_OF relation.";
					dcterms:modified "2021-01-26"^^xsd:date;
					dcterms:creator <https://www.tib.eu/en/research-development/scientific-data-management/staff/samaneh-jozashoori/>.

<http://research.tib.eu/clarify2020/vocab/NEG_MANIFESTATION_OF>	rdf:type	owl:Class;
					rdfs:label	"NEG_MANIFESTATION_OF";
					rdfs:subClassOf	<http://research.tib.eu/clarify2020/vocab/Relation>;
					rdfs:comment "Relation between two UMLS CUIs that represents the negation of MANIFESTATION_OF relation.";
					dcterms:modified "2021-01-26"^^xsd:date;
					dcterms:creator <https://www.tib.eu/en/research-development/scientific-data-management/staff/samaneh-jozashoori/>.

<http://research.tib.eu/clarify2020/vocab/NEG_MEASURES>	rdf:type	owl:Class;
					rdfs:label	"NEG_MEASURES";
					rdfs:subClassOf	<http://research.tib.eu/clarify2020/vocab/Relation>;
					rdfs:comment "Relation between two UMLS CUIs that represents the negation of MEASURES relation.";
					dcterms:modified "2021-01-26"^^xsd:date;
					dcterms:creator <https://www.tib.eu/en/research-development/scientific-data-management/staff/samaneh-jozashoori/>.

<http://research.tib.eu/clarify2020/vocab/NEG_METHOD_OF>	rdf:type	owl:Class;
					rdfs:label	"NEG_METHOD_OF";
					rdfs:subClassOf	<http://research.tib.eu/clarify2020/vocab/Relation>;
					rdfs:comment "Relation between two UMLS CUIs that represents the negation of METHOD_OF relation.";
					dcterms:modified "2021-01-26"^^xsd:date;
					dcterms:creator <https://www.tib.eu/en/research-development/scientific-data-management/staff/samaneh-jozashoori/>.

<http://research.tib.eu/clarify2020/vocab/NEG_OCCURS_IN>	rdf:type	owl:Class;
					rdfs:label	"NEG_OCCURS_IN";
					rdfs:subClassOf	<http://research.tib.eu/clarify2020/vocab/Relation>;
					rdfs:comment "Relation between two UMLS CUIs that represents the negation of OCCURS_IN relation.";
					dcterms:modified "2021-01-26"^^xsd:date;
					dcterms:creator <https://www.tib.eu/en/research-development/scientific-data-management/staff/samaneh-jozashoori/>.

<http://research.tib.eu/clarify2020/vocab/NEG_PART_OF>	rdf:type	owl:Class;
					rdfs:label	"NEG_PART_OF";
					rdfs:subClassOf	<http://research.tib.eu/clarify2020/vocab/Relation>;
					rdfs:comment "Relation between two UMLS CUIs that represents the negation of PART_OF relation.";
					dcterms:modified "2021-01-26"^^xsd:date;
					dcterms:creator <https://www.tib.eu/en/research-development/scientific-data-management/staff/samaneh-jozashoori/>.

<http://research.tib.eu/clarify2020/vocab/NEG_PRECEDES>	rdf:type	owl:Class;
					rdfs:label	"NEG_PRECEDES";
					rdfs:subClassOf	<http://research.tib.eu/clarify2020/vocab/Relation>;
					rdfs:comment "Relation between two UMLS CUIs that represents the negation of PRECEDES relation.";
					dcterms:modified "2021-01-26"^^xsd:date;
					dcterms:creator <https://www.tib.eu/en/research-development/scientific-data-management/staff/samaneh-jozashoori/>.

<http://research.tib.eu/clarify2020/vocab/NEG_PREDISPOSES>	rdf:type	owl:Class;
					rdfs:label	"NEG_PREDISPOSES";
					rdfs:subClassOf	<http://research.tib.eu/clarify2020/vocab/Relation>;
					rdfs:comment "Relation between two UMLS CUIs that represents the negation of PREDISPOSES relation.";
					dcterms:modified "2021-01-26"^^xsd:date;
					dcterms:creator <https://www.tib.eu/en/research-development/scientific-data-management/staff/samaneh-jozashoori/>.

<http://research.tib.eu/clarify2020/vocab/NEG_PREVENTS>	rdf:type	owl:Class;
					rdfs:label	"NEG_PREVENTS";
					rdfs:subClassOf	<http://research.tib.eu/clarify2020/vocab/Relation>;
					rdfs:comment "Relation between two UMLS CUIs that represents the negation of PREVENTS relation.";
					dcterms:modified "2021-01-26"^^xsd:date;
					dcterms:creator <https://www.tib.eu/en/research-development/scientific-data-management/staff/samaneh-jozashoori/>.

<http://research.tib.eu/clarify2020/vocab/NEG_PROCESS_OF>	rdf:type	owl:Class;
					rdfs:label	"NEG_PROCESS_OF";
					rdfs:subClassOf	<http://research.tib.eu/clarify2020/vocab/Relation>;
					rdfs:comment "Relation between two UMLS CUIs that represents the negation of PROCESS_OF relation.";
					dcterms:modified "2021-01-26"^^xsd:date;
					dcterms:creator <https://www.tib.eu/en/research-development/scientific-data-management/staff/samaneh-jozashoori/>.

<http://research.tib.eu/clarify2020/vocab/NEG_PRODUCES>	rdf:type	owl:Class;
					rdfs:label	"NEG_PRODUCES";
					rdfs:subClassOf	<http://research.tib.eu/clarify2020/vocab/Relation>;
					rdfs:comment "Relation between two UMLS CUIs that represents the negation of PRODUCES relation.";
					dcterms:modified "2021-01-26"^^xsd:date;
					dcterms:creator <https://www.tib.eu/en/research-development/scientific-data-management/staff/samaneh-jozashoori/>.

<http://research.tib.eu/clarify2020/vocab/NEG_STIMULATES>	rdf:type	owl:Class;
					rdfs:label	"NEG_STIMULATES";
					rdfs:subClassOf	<http://research.tib.eu/clarify2020/vocab/Relation>;
					rdfs:comment "Relation between two UMLS CUIs that represents the negation of STIMULATES relation.";
					dcterms:modified "2021-01-26"^^xsd:date;
					dcterms:creator <https://www.tib.eu/en/research-development/scientific-data-management/staff/samaneh-jozashoori/>.

<http://research.tib.eu/clarify2020/vocab/NEG_TREATS>	rdf:type	owl:Class;
					rdfs:label	"NEG_TREATS";
					rdfs:subClassOf	<http://research.tib.eu/clarify2020/vocab/Relation>;
					rdfs:comment "Relation between two UMLS CUIs that represents the negation of TREATS relation.";
					dcterms:modified "2021-01-26"^^xsd:date;
					dcterms:creator <https://www.tib.eu/en/research-development/scientific-data-management/staff/samaneh-jozashoori/>.

<http://research.tib.eu/clarify2020/vocab/NEG_USES>	rdf:type	owl:Class;
					rdfs:label	"NEG_USES";
					rdfs:subClassOf	<http://research.tib.eu/clarify2020/vocab/Relation>;
					rdfs:comment "Relation between two UMLS CUIs that represents the negation of USES relation.";
					dcterms:modified "2021-01-26"^^xsd:date;
					dcterms:creator <https://www.tib.eu/en/research-development/scientific-data-management/staff/samaneh-jozashoori/>.

<http://research.tib.eu/clarify2020/vocab/NEG_higher_than>	rdf:type	owl:Class;
					rdfs:label	"NEG_higher_than";
					rdfs:subClassOf	<http://research.tib.eu/clarify2020/vocab/Relation>;
					rdfs:comment "Relation between two UMLS CUIs that represents the negation of higher_than relation.";
					dcterms:modified "2021-01-26"^^xsd:date;
					dcterms:creator <https://www.tib.eu/en/research-development/scientific-data-management/staff/samaneh-jozashoori/>.

<http://research.tib.eu/clarify2020/vocab/NEG_lower_than>	rdf:type	owl:Class;
					rdfs:label	"NEG_lower_than";
					rdfs:subClassOf	<http://research.tib.eu/clarify2020/vocab/Relation>;
					rdfs:comment "Relation between two UMLS CUIs that represents the negation of lower_than relation.";
					dcterms:modified "2021-01-26"^^xsd:date;
					dcterms:creator <https://www.tib.eu/en/research-development/scientific-data-management/staff/samaneh-jozashoori/>.

<http://research.tib.eu/clarify2020/vocab/NEG_same_as>	rdf:type	owl:Class;
					rdfs:label	"NEG_same_as";
					rdfs:subClassOf	<http://research.tib.eu/clarify2020/vocab/Relation>;
					rdfs:comment "Relation between two UMLS CUIs that represents the negation of same_as relation.";
					dcterms:modified "2021-01-26"^^xsd:date;
					dcterms:creator <https://www.tib.eu/en/research-development/scientific-data-management/staff/samaneh-jozashoori/>.

<http://research.tib.eu/clarify2020/vocab/OCCURS_IN>	rdf:type	owl:Class;
					rdfs:label	"OCCURS_IN";
					rdfs:subClassOf	<http://research.tib.eu/clarify2020/vocab/Relation>;
					rdfs:comment "Relation between two UMLS CUIs that represents having incidence in a group or population.";
					dcterms:modified "2021-01-26"^^xsd:date;
					dcterms:creator <https://www.tib.eu/en/research-development/scientific-data-management/staff/samaneh-jozashoori/>.

<http://research.tib.eu/clarify2020/vocab/PART_OF>	rdf:type	owl:Class;
					rdfs:label	"PART_OF";
					rdfs:subClassOf	<http://research.tib.eu/clarify2020/vocab/Relation>;
					rdfs:comment "Relation between two UMLS CUIs that represents composing, with one or more other physical units, some larger whole.";
					dcterms:modified "2021-01-26"^^xsd:date;
					dcterms:creator <https://www.tib.eu/en/research-development/scientific-data-management/staff/samaneh-jozashoori/>.

<http://research.tib.eu/clarify2020/vocab/PRECEDES>	rdf:type	owl:Class;
					rdfs:label	"PRECEDES";
					rdfs:subClassOf	<http://research.tib.eu/clarify2020/vocab/Relation>;
					rdfs:comment "Relation between two UMLS CUIs that represents occurring earlier in time.";
					dcterms:modified "2021-01-26"^^xsd:date;
					dcterms:creator <https://www.tib.eu/en/research-development/scientific-data-management/staff/samaneh-jozashoori/>.

<http://research.tib.eu/clarify2020/vocab/PREDISPOSES>	rdf:type	owl:Class;
					rdfs:label	"PREDISPOSES";
					rdfs:subClassOf	<http://research.tib.eu/clarify2020/vocab/Relation>;
					rdfs:comment "Relation between UMLS CUIs to represent the genetic etiology of disease; the relation is of type predisposal between two terms.";
					dcterms:modified "2021-01-26"^^xsd:date;
					dcterms:creator <https://www.tib.eu/en/research-development/scientific-data-management/staff/samaneh-jozashoori/>.

<http://research.tib.eu/clarify2020/vocab/PREVENTS>	rdf:type	owl:Class;
					rdfs:label	"PREVENTS";
					rdfs:subClassOf	<http://research.tib.eu/clarify2020/vocab/Relation>;
					rdfs:comment "Relation between UMLS CUIs to represent stopping, hindering or eliminating an action or condition.";
					dcterms:modified "2021-01-26"^^xsd:date;
					dcterms:creator <https://www.tib.eu/en/research-development/scientific-data-management/staff/samaneh-jozashoori/>.

<http://research.tib.eu/clarify2020/vocab/PROCESS_OF>	rdf:type	owl:Class;
					rdfs:label	"PROCESS_OF";
					rdfs:subClassOf	<http://research.tib.eu/clarify2020/vocab/Relation>;
					rdfs:comment "Relation between two UMLS CUIs that represents the disorder occurs in (higher) organisms.";
					dcterms:modified "2021-01-26"^^xsd:date;
					dcterms:creator <https://www.tib.eu/en/research-development/scientific-data-management/staff/samaneh-jozashoori/>.

<http://research.tib.eu/clarify2020/vocab/PRODUCES>	rdf:type	owl:Class;
					rdfs:label	"PRODUCES";
					rdfs:subClassOf	<http://research.tib.eu/clarify2020/vocab/Relation>;
					rdfs:comment "Relation between UMLS CUIs that represents bringing forth, generating or creating.";
					dcterms:modified "2021-01-26"^^xsd:date;
					dcterms:creator <https://www.tib.eu/en/research-development/scientific-data-management/staff/samaneh-jozashoori/>.

<http://research.tib.eu/clarify2020/vocab/STIMULATES>	rdf:type	owl:Class;
					rdfs:label	"STIMULATES";
					rdfs:subClassOf	<http://research.tib.eu/clarify2020/vocab/Relation>;
					rdfs:comment "Relation between UMLS CUIs that describes substance interactions in terms of increasing or facilitating the action or function.";
					dcterms:modified "2021-01-26"^^xsd:date;
					dcterms:creator <https://www.tib.eu/en/research-development/scientific-data-management/staff/samaneh-jozashoori/>.

<http://research.tib.eu/clarify2020/vocab/TREATS>	rdf:type	owl:Class;
					rdfs:label	"TREATS";
					rdfs:subClassOf	<http://research.tib.eu/clarify2020/vocab/Relation>;
					rdfs:comment "Relation between UMLS CUIs that represents the relation of type treating between two clinical medicine terms.";
					dcterms:modified "2021-01-26"^^xsd:date;
					dcterms:creator <https://www.tib.eu/en/research-development/scientific-data-management/staff/samaneh-jozashoori/>.

<http://research.tib.eu/clarify2020/vocab/USES>	rdf:type	owl:Class;
					rdfs:label	"USES";
					rdfs:subClassOf	<http://research.tib.eu/clarify2020/vocab/Relation>;
					rdfs:comment "Relation between two UMLS CUIs that represents employing in the carrying out of some activity.";
					dcterms:modified "2021-01-26"^^xsd:date;
					dcterms:creator <https://www.tib.eu/en/research-development/scientific-data-management/staff/samaneh-jozashoori/>.

<http://research.tib.eu/clarify2020/vocab/compared_with>	rdf:type	owl:Class;
					rdfs:label	"compared_with";
					rdfs:subClassOf	<http://research.tib.eu/clarify2020/vocab/Relation>;
					rdfs:comment "Relation between UMLS CUIs that represents the relation of type comparative between two terms.";
					dcterms:modified "2021-01-26"^^xsd:date;
					dcterms:creator <https://www.tib.eu/en/research-development/scientific-data-management/staff/samaneh-jozashoori/>.

<http://research.tib.eu/clarify2020/vocab/higher_than>	rdf:type	owl:Class;
					rdfs:label	"higher_than";
					rdfs:subClassOf	<http://research.tib.eu/clarify2020/vocab/Relation>;
					rdfs:comment "Relation between UMLS CUIs that represents the relation of type comparative between two terms";
					dcterms:modified "2021-01-26"^^xsd:date;
					dcterms:creator <https://www.tib.eu/en/research-development/scientific-data-management/staff/samaneh-jozashoori/>.

<http://research.tib.eu/clarify2020/vocab/lower_than>	rdf:type	owl:Class;
					rdfs:label	"lower_than";
					rdfs:subClassOf	<http://research.tib.eu/clarify2020/vocab/Relation>;
					rdfs:comment "Relation between UMLS CUIs that represents the relation of type comparative between two terms.";
					dcterms:modified "2021-01-26"^^xsd:date;
					dcterms:creator <https://www.tib.eu/en/research-development/scientific-data-management/staff/samaneh-jozashoori/>.

<http://research.tib.eu/clarify2020/vocab/same_as>	rdf:type	owl:Class;
					rdfs:label	"same_as";
					rdfs:subClassOf	<http://research.tib.eu/clarify2020/vocab/Relation>;
					rdfs:comment "Relation between UMLS CUIs that represents the relation of type comparative between two terms.";
					dcterms:modified "2021-01-26"^^xsd:date;
					dcterms:creator <https://www.tib.eu/en/research-development/scientific-data-management/staff/samaneh-jozashoori/>.



######################################################################################################################################
#########################################################    Drug    #################################################################
######################################################################################################################################


<http://research.tib.eu/clarify2020/vocab/Drug>	rdf:type	owl:Class;
			rdfs:label	"Drug";
			rdfs:subClassOf	<http://research.tib.eu/clarify2020/vocab/Concept>;
			rdfs:comment "A substance used as a medication or in the preparation of medication.";
			dcterms:modified "2020-09-14"^^xsd:date;
			dcterms:creator <https://www.tib.eu/en/research-development/scientific-data-management/staff/samaneh-jozashoori/>.

<http://research.tib.eu/clarify2020/vocab/DrugSchema>	rdf:type	owl:Class;
					rdfs:label	"DrugSchema";
					rdfs:subClassOf	<http://research.tib.eu/clarify2020/vocab/Concept>;
					rdfs:comment "A combination of different substances used as a medication or in the preparation of medication.";
					dcterms:modified "2022-09-12"^^xsd:date;
					dcterms:creator <https://www.tib.eu/en/research-development/scientific-data-management/staff/samaneh-jozashoori/>.


<http://research.tib.eu/clarify2020/vocab/NonOncologicalDrug>	rdf:type	owl:Class;
							rdfs:label	"NonOncologicalDrug";
							rdfs:subClassOf	<http://research.tib.eu/clarify2020/vocab/Drug>;
							rdfs:comment "A Drug which is prescribed to treat disorders other than cancer.";
							dcterms:modified "2021-06-29"^^xsd:date;
							dcterms:creator <https://www.tib.eu/en/research-development/scientific-data-management/staff/samaneh-jozashoori/>.

<http://research.tib.eu/clarify2020/vocab/OncologicalDrug>	rdf:type	owl:Class;
							rdfs:label	"OncologicalDrug";
							rdfs:subClassOf	<http://research.tib.eu/clarify2020/vocab/Drug>;
							rdfs:comment "A Drug category which is prescribed to treat cancer.";
							dcterms:modified "2021-06-29"^^xsd:date;
							dcterms:creator <https://www.tib.eu/en/research-development/scientific-data-management/staff/samaneh-jozashoori/>.

<http://research.tib.eu/clarify2020/vocab/Biomarker>	 rdf:type	owl:Class;
					rdfs:label	"Biomarker";
					rdfs:subClassOf	<http://research.tib.eu/clarify2020/vocab/Concept>;
					rdfs:comment "A biomarker, or biological marker is a measurable indicator of some biological state or condition.";
					dcterms:modified "2020-09-14"^^xsd:date;
					dcterms:creator <https://www.tib.eu/en/research-development/scientific-data-management/staff/samaneh-jozashoori/>.

<http://research.tib.eu/clarify2020/vocab/Phenotype>	rdf:type	owl:Class;
					rdfs:label	"Phenotype";
					rdfs:subClassOf	<http://research.tib.eu/clarify2020/vocab/Concept>;
					rdfs:comment "The set of observable characteristics of an individual resulting from the interaction of its genotype with the environment. This class include side effects that result from different drugs.";
					dcterms:modified "2020-12-15"^^xsd:date;
					dcterms:creator <https://www.tib.eu/en/research-development/scientific-data-management/staff/samaneh-jozashoori/>.

<http://research.tib.eu/clarify2020/vocab/Target>	rdf:type	owl:Class;
				rdfs:label	"Target";
				rdfs:subClassOf	<http://research.tib.eu/clarify2020/vocab/Concept>;
				rdfs:comment "A drug target is a molecule in the body, usually a protein, that is intrinsically associated with a particular disease process and that could be addressed by a drug to produce a desired therapeutic effect.";
				dcterms:modified "2020-12-15"^^xsd:date;
				dcterms:creator <https://www.tib.eu/en/research-development/scientific-data-management/staff/samaneh-jozashoori/>.

<http://research.tib.eu/clarify2020/vocab/Protein>	rdf:type	owl:Class;
				rdfs:label	"Protein";
				rdfs:subClassOf	<http://research.tib.eu/clarify2020/vocab/Concept>;
				rdfs:comment "Large and complex molecules that play many critical roles in the body. They are required for the structure, function and regulation of the body's tissues and organs.";
				dcterms:modified "2020-12-15"^^xsd:date;
				dcterms:creator <https://www.tib.eu/en/research-development/scientific-data-management/staff/samaneh-jozashoori/>.

<http://research.tib.eu/clarify2020/vocab/Enzyme>	rdf:type	owl:Class;
				rdfs:label	"Enzyme";
				rdfs:subClassOf	<http://research.tib.eu/clarify2020/vocab/Concept>;
				rdfs:comment "Macromolecular biological catalyst that accelerate chemical reactions. Most enzymes are proteins.";
				dcterms:modified "2020-12-15"^^xsd:date;
				dcterms:creator <https://www.tib.eu/en/research-development/scientific-data-management/staff/samaneh-jozashoori/>.

<http://research.tib.eu/clarify2020/vocab/DrugDrugInteraction>	rdf:type	owl:Class;
				rdfs:label	"DrugDrugInteraction";
				rdfs:subClassOf	<http://research.tib.eu/clarify2020/vocab/Interaction>;
				rdfs:comment "The relation between two drugs that interact.";
				dcterms:modified "2020-12-15"^^xsd:date;
				dcterms:creator <https://www.tib.eu/en/research-development/scientific-data-management/staff/samaneh-jozashoori/>.

<http://research.tib.eu/clarify2020/vocab/Interaction>	rdf:type owl:Class;
			rdfs:label	"Interaction";
			rdfs:subClassOf	<http://research.tib.eu/clarify2020/vocab/INTERACTS_WITH>;
			rdfs:comment "Interaction between drugs and disorder, enzyme, target.";
			dcterms:modified "2021-01-07"^^xsd:date;
			dcterms:creator <https://www.tib.eu/en/research-development/scientific-data-management/staff/samaneh-jozashoori/>.

<http://research.tib.eu/clarify2020/vocab/DrugDisorderInteraction>	rdf:type	owl:Class;
								rdfs:label	"DrugDisorderInteraction";
								rdfs:subClassOf	<http://research.tib.eu/clarify2020/vocab/Interaction>;
								rdfs:comment "A drug-induced disorder.";
								dcterms:modified "2020-12-15"^^xsd:date;
								dcterms:creator <https://www.tib.eu/en/research-development/scientific-data-management/staff/maria-isabel-castellanos/>.

<http://research.tib.eu/clarify2020/vocab/DrugEnzymeInteraction>	rdf:type	owl:Class;
				rdfs:label	"DrugEnzymeInteraction";
				rdfs:subClassOf	<http://research.tib.eu/clarify2020/vocab/Interaction>;
				rdfs:comment "Interactions similar to drug receptor interactions where drugs resemble the natural substrates and bind enzymes.";
				dcterms:modified "2020-12-15"^^xsd:date;
				dcterms:creator <https://www.tib.eu/en/research-development/scientific-data-management/staff/samaneh-jozashoori/>.

<http://research.tib.eu/clarify2020/vocab/DrugSideEffectInteraction>	rdf:type	owl:Class;
						rdfs:label	"DrugSideEffectInteraction";
						rdfs:subClassOf	<http://research.tib.eu/clarify2020/vocab/Interaction>;
						rdfs:comment "Effects of drugs, whether therapeutic or adverse, that are secondary to the one intended.";
						dcterms:modified "2020-12-15"^^xsd:date;
						dcterms:creator <https://www.tib.eu/en/research-development/scientific-data-management/staff/samaneh-jozashoori/>.

<http://research.tib.eu/clarify2020/vocab/DrugTargetInteraction>	rdf:type	owl:Class;
				rdfs:label	"DrugTargetInteraction";
				rdfs:subClassOf	<http://research.tib.eu/clarify2020/vocab/Interaction>;
				rdfs:comment "Interactions between chemical compounds and the protein targets in the human body.";
				dcterms:modified "2020-12-15"^^xsd:date;
				dcterms:creator <https://www.tib.eu/en/research-development/scientific-data-management/staff/samaneh-jozashoori/>.

<http://research.tib.eu/clarify2020/vocab/SymmetricDrugDrugInteraction>	rdf:type	owl:Class;
				rdfs:label	"SymmetricDrugDrugInteraction";
				rdfs:subClassOf	<http://research.tib.eu/clarify2020/vocab/DrugDrugInteraction>;
				rdfs:comment "The interactions between two drugs that do not change the effectiveness of the drugs.";
				dcterms:modified "2020-12-15"^^xsd:date;
				dcterms:creator <https://www.tib.eu/en/research-development/scientific-data-management/staff/samaneh-jozashoori/>.

<http://research.tib.eu/clarify2020/vocab/NonSymmetricDrugDrugInteraction>	rdf:type	owl:Class;
				rdfs:label	"NonSymmetricDrugDrugInteraction";
				rdfs:subClassOf	<http://research.tib.eu/clarify2020/vocab/DrugDrugInteraction>;
				rdfs:comment "The interactions between two drugs that change the effectiveness of the drugs.";
				dcterms:modified "2021-07-01"^^xsd:date;
				dcterms:creator <https://www.tib.eu/en/research-development/scientific-data-management/staff/samaneh-jozashoori/>.

<http://research.tib.eu/clarify2020/vocab/CancerStage>	rdf:type	owl:Class;
					rdfs:label	"CancerStage";
					rdfs:comment "Represents the assessment of the stage of tumor in a particular date.";
					dcterms:modified "2020-09-14"^^xsd:date;
					dcterms:creator <https://www.tib.eu/en/research-development/scientific-data-management/staff/samaneh-jozashoori/>.



######################################################################################################################################
#################################################    Drug Predictions   ##############################################################
######################################################################################################################################

<http://research.tib.eu/clarify2020/vocab/DrugDrugPrediction>	rdf:type owl:Class;
						rdfs:label	"DrugDrugPrediction";
						rdfs:subClassOf	<http://research.tib.eu/clarify2020/vocab/Interaction>;
						rdfs:comment "Represents the predicted relation between drugs.";
						dcterms:modified "2021-01-07"^^xsd:date;
						dcterms:creator <https://www.tib.eu/en/research-development/scientific-data-management/staff/samaneh-jozashoori/>.

<http://research.tib.eu/clarify2020/vocab/DrugEnzymePrediction>	rdf:type owl:Class;
							rdfs:label	"DrugEnzymePrediction";
							rdfs:subClassOf	<http://research.tib.eu/clarify2020/vocab/Interaction>;
							rdfs:comment "Represents the predicted relation between drug and enzyme.";
							dcterms:modified "2021-01-07"^^xsd:date;
							dcterms:creator <https://www.tib.eu/en/research-development/scientific-data-management/staff/samaneh-jozashoori/>.

<http://research.tib.eu/clarify2020/vocab/DrugSideEffectPrediction>	rdf:type owl:Class;
								rdfs:label	"DrugSideEffectPrediction";
								rdfs:subClassOf	<http://research.tib.eu/clarify2020/vocab/Interaction>;
								rdfs:comment "Represents the predicted relation between drug and side effects.";
								dcterms:modified "2021-01-07"^^xsd:date;
								dcterms:creator <https://www.tib.eu/en/research-development/scientific-data-management/staff/samaneh-jozashoori/>.

<http://research.tib.eu/clarify2020/vocab/DrugTargetPrediction>	rdf:type owl:Class;
							rdfs:label	"DrugTargetPrediction";
							rdfs:subClassOf	<http://research.tib.eu/clarify2020/vocab/Interaction>;
							rdfs:comment "Represents the predicted relation between drug and target.";
							dcterms:modified "2021-01-07"^^xsd:date;
							dcterms:creator <https://www.tib.eu/en/research-development/scientific-data-management/staff/samaneh-jozashoori/>.

#################################################################################################################################################
#################################################################################################################################################
#################################################################################################################################################
######################################################## Properties - attributes ################################################################
#################################################################################################################################################
#################################################################################################################################################
#################################################################################################################################################


######################################################################################################################################
#########################################################    Clinical    #################################################################
######################################################################################################################################


<http://research.tib.eu/clarify2020/vocab/date>	rdf:type	owl:DatatypeProperty;
								rdfs:label	"date";
								rdfs:domain	<http://research.tib.eu/clarify2020/vocab/Concept>;
								rdfs:range	rdfs:Literal;
								rdfs:comment "Represents the date of occurrence.";
								dcterms:modified "2020-10-20"^^xsd:date;							
								dcterms:creator <https://www.tib.eu/en/research-development/scientific-data-management/staff/samaneh-jozashoori/>.

<http://research.tib.eu/clarify2020/vocab/treatementLineDate>	rdf:type	owl:DatatypeProperty;
								rdfs:label	"treatementLineDate";
								rdfs:subPropertyOf <http://research.tib.eu/clarify2020/vocab/date>;
								rdfs:domain	<http://research.tib.eu/clarify2020/vocab/Concept>;
								rdfs:range	rdfs:Literal;
								rdfs:comment "Represents the date of the occurrence of a treatment.";
								dcterms:modified "2022-09-12"^^xsd:date;							
								dcterms:creator <https://www.tib.eu/en/research-development/scientific-data-management/staff/samaneh-jozashoori/>.

<http://research.tib.eu/clarify2020/vocab/firstSurgeryDate>	rdf:type	owl:DatatypeProperty;
							rdfs:label	"firstSurgeryDate";
							rdfs:subPropertyOf <http://research.tib.eu/clarify2020/vocab/date>;
							rdfs:domain	<http://research.tib.eu/clarify2020/vocab/Concept>;
							rdfs:range	rdfs:Literal;
							rdfs:comment "Represents the date of the occurrence of the first oncological surgery.";
							dcterms:modified "2022-09-12"^^xsd:date;							
							dcterms:creator <https://www.tib.eu/en/research-development/scientific-data-management/staff/samaneh-jozashoori/>.

<http://research.tib.eu/clarify2020/vocab/previousCancerTypeDescription>	rdf:type	owl:DatatypeProperty;
										rdfs:label	"previousCancerTypeDescription";
										rdfs:domain	<http://research.tib.eu/clarify2020/vocab/Concept>;
										rdfs:range	rdfs:Literal;
										rdfs:comment "Provides extra texual descriptions about the concept.";
										dcterms:modified "2020-10-21"^^xsd:date;							
										dcterms:creator <https://www.tib.eu/en/research-development/scientific-data-management/staff/samaneh-jozashoori/>.

<http://research.tib.eu/clarify2020/vocab/birthDate>	rdf:type	owl:DatatypeProperty;
						rdfs:label	"birthDate";
						rdfs:domain	<http://research.tib.eu/clarify2020/vocab/LCPatient>;
						rdfs:range	rdfs:Literal;
						rdfs:comment "Represents the birth date of the patient.";
						dcterms:modified "2020-10-19"^^xsd:date;
						dcterms:creator <https://www.tib.eu/en/research-development/scientific-data-management/staff/samaneh-jozashoori/>.		

<http://research.tib.eu/clarify2020/vocab/biomarkerSpecification>	rdf:type	owl:DatatypeProperty;
								rdfs:label	"biomarkerSpecification";
								rdfs:domain	<http://research.tib.eu/clarify2020/vocab/Biomarker>;
								rdfs:range	rdfs:Literal;
								rdfs:comment "Textual description of a molecular marker.";
								dcterms:modified "2020-10-19"^^xsd:date;
								dcterms:creator <https://www.tib.eu/en/research-development/scientific-data-management/staff/samaneh-jozashoori/>.

<http://research.tib.eu/clarify2020/vocab/numberOfFamilyWithLC>	rdf:type	owl:DatatypeProperty;
									rdfs:label	"numberOfFamilyWithLC";
									rdfs:domain	<http://research.tib.eu/clarify2020/vocab/FamilyHistory>;
									rdfs:range	rdfs:Literal;
									rdfs:comment "Represents the number of family members with lung cancer.";
									dcterms:modified "2020-10-20"^^xsd:date;							
									dcterms:creator <https://www.tib.eu/en/research-development/scientific-data-management/staff/samaneh-jozashoori/>.

<http://research.tib.eu/clarify2020/vocab/numberOfFamilyWithOtherCancers>	rdf:type	owl:DatatypeProperty;
										rdfs:label	"numberOfFamilyWithOtherCancers";
										rdfs:domain	<http://research.tib.eu/clarify2020/vocab/FamilyHistory>;
										rdfs:range	rdfs:Literal;
										rdfs:comment "Represents the number of family members with cancers other than lung.";
										dcterms:modified "2020-10-20"^^xsd:date;							
										dcterms:creator <https://www.tib.eu/en/research-development/scientific-data-management/staff/samaneh-jozashoori/>.

<http://research.tib.eu/clarify2020/vocab/treatmentLineDosage>	rdf:type	owl:DatatypeProperty;
							rdfs:label	"treatmentLineDosage";
							rdfs:domain	<http://research.tib.eu/clarify2020/vocab/OncologicalTreatmentLine>;
							rdfs:range	rdfs:Literal;
							rdfs:comment "Represents the dosage that is prescribed to the patient.";
							dcterms:modified "2020-10-20"^^xsd:date;														
							dcterms:creator <https://www.tib.eu/en/research-development/scientific-data-management/staff/samaneh-jozashoori/>.

<http://research.tib.eu/clarify2020/vocab/treatmentLineFractioning>	rdf:type	owl:DatatypeProperty;
									rdfs:label	"treatmentLineFractioning";
									rdfs:domain	<http://research.tib.eu/clarify2020/vocab/OncologicalTreatmentLine>;
									rdfs:range	rdfs:Literal;
									rdfs:comment "Represents the radiotherapy fraction that is prescribed to the patient.";
									dcterms:modified "2020-11-19"^^xsd:date;														
									dcterms:creator <https://www.tib.eu/en/research-development/scientific-data-management/staff/samaneh-jozashoori/>.

<http://research.tib.eu/clarify2020/vocab/disorderLabel>	rdf:type owl:DatatypeProperty;
							rdfs:label "disorderLabel";
							rdfs:domain <http://research.tib.eu/clarify2020/vocab/Disorder>;
						  	rdfs:range rdfs:Literal;
							rdfs:comment "Disorder label.";
							dcterms:modified "2020-10-21"^^xsd:date;
							dcterms:creator <https://www.tib.eu/en/research-development/scientific-data-management/staff/samaneh-jozashoori/>.

<http://research.tib.eu/clarify2020/vocab/lastMonitoringDate>	rdf:type owl:DatatypeProperty;
							rdfs:label "lastMonitoringDate";
							rdfs:domain <http://research.tib.eu/clarify2020/vocab/StatusEvolution>;
						  	rdfs:range rdfs:Literal;
							rdfs:comment "Represents the date on which the patient was monitored for the last time.";
							dcterms:modified "2020-10-21"^^xsd:date;
							dcterms:creator <https://www.tib.eu/en/research-development/scientific-data-management/staff/samaneh-jozashoori/>.

<http://research.tib.eu/clarify2020/vocab/deathDate>	rdf:type	owl:DatatypeProperty;
					rdfs:label	"deathDate";
					rdfs:domain	<http://research.tib.eu/clarify2020/vocab/StatusEvolution>;
					rdfs:range	rdfs:Literal;
					rdfs:comment "Represents the lung cancer patient's date of death (structured information provided by HUPHM).";
					dcterms:modified "2020-10-21"^^xsd:date;
					dcterms:creator <https://www.tib.eu/en/research-development/scientific-data-management/staff/samaneh-jozashoori/>.

<http://research.tib.eu/clarify2020/vocab/numberOfCigarettesPerDay>	rdf:type	owl:DatatypeProperty;	
									rdfs:label	"numberOfCigarettesPerDay";
									rdfs:domain	<http://research.tib.eu/clarify2020/vocab/CPatient>;
									rdfs:range	rdfs:Literal;
									rdfs:comment	"The number of cigarettes per day that the patient smokes.";
									dcterms:modified "2020-10-21"^^xsd:date;
									dcterms:creator <https://www.tib.eu/en/research-development/scientific-data-management/staff/samaneh-jozashoori/>.

<http://research.tib.eu/clarify2020/vocab/numberOfCigarettesPerYear>	rdf:type	owl:DatatypeProperty;	
									rdfs:label	"numberOfCigarettesPerYear";
									rdfs:domain	<http://research.tib.eu/clarify2020/vocab/CPatient>;
									rdfs:range	rdfs:Literal;
									rdfs:comment	"The number of cigarettes per year that the patient smokes.";
									dcterms:modified "2020-11-19"^^xsd:date;
									dcterms:creator <https://www.tib.eu/en/research-development/scientific-data-management/staff/samaneh-jozashoori/>.

<http://research.tib.eu/clarify2020/vocab/numberOfYearsOfSmoking>	rdf:type        owl:DatatypeProperty;	
								rdfs:label	"numberOfYearsOfSmoking";
								rdfs:domain	<http://research.tib.eu/clarify2020/vocab/CPatient>;
								rdfs:range	rdfs:Literal;
								rdfs:comment "Represents for how many years the patient used to be an active smoker.";
								dcterms:modified "2020-10-21"^^xsd:date;
								dcterms:creator <https://www.tib.eu/en/research-development/scientific-data-management/staff/samaneh-jozashoori/>.

<http://research.tib.eu/clarify2020/vocab/treatementLineEndingDate>	rdf:type owl:DatatypeProperty;	
									rdfs:label	"treatementLineEndingDate";
									rdfs:domain	<http://research.tib.eu/clarify2020/vocab/OncologicalTreatmentLine>;
									rdfs:range	rdfs:Literal;
									rdfs:comment "Represents the ending date of the treatment line.";
									dcterms:modified "2021-02-25"^^xsd:date;
									dcterms:creator <https://www.tib.eu/en/research-development/scientific-data-management/staff/samaneh-jozashoori/>.

<http://research.tib.eu/clarify2020/vocab/treatementLineStartDate>	rdf:type owl:DatatypeProperty;	
								rdfs:label	"treatementLineStartDate";
								rdfs:domain	<http://research.tib.eu/clarify2020/vocab/OncologicalTreatmentLine>;
								rdfs:range	rdfs:Literal;
								rdfs:comment "Represents the starting date of the treatment line.";
								dcterms:modified "2021-02-25"^^xsd:date;
								dcterms:creator <https://www.tib.eu/en/research-development/scientific-data-management/staff/samaneh-jozashoori/>.

<http://research.tib.eu/clarify2020/vocab/hasOriginalValue>	rdf:type owl:DatatypeProperty;	
							rdfs:label	"hasOriginalValue";
							rdfs:domain	<http://research.tib.eu/clarify2020/vocab/Concept>;
							rdfs:range	rdfs:Literal;
							rdfs:comment "The original value of the instance in the RDB provided by UPM.";
							dcterms:modified "2021-05-17"^^xsd:date;
							dcterms:creator <https://www.tib.eu/en/research-development/scientific-data-management/staff/samaneh-jozashoori/>.


<http://research.tib.eu/clarify2020/vocab/hasProteinName>	rdf:type owl:DatatypeProperty;	
							rdfs:label	"hasProteinName";
							rdfs:domain	<http://research.tib.eu/clarify2020/vocab/Protein>;
							rdfs:range	rdfs:Literal;
							rdfs:comment "The name of Protein.";
							dcterms:modified "2023-04-25"^^xsd:date;
							dcterms:creator <https://www.tib.eu/en/research-development/scientific-data-management/staff/emetis-niazmand/>.

<http://research.tib.eu/clarify2020/vocab/biomarkerAnalysisDate>	rdf:type owl:DatatypeProperty;	
								rdfs:label	"biomarkerAnalysisDate";
								rdfs:domain	<http://research.tib.eu/clarify2020/vocab/CPatient>;
								rdfs:range	rdfs:Literal;
								rdfs:comment "The date on which a biomarker test of the patient is analysed.";
								dcterms:modified "2021-05-17"^^xsd:date;
								dcterms:creator <https://www.tib.eu/en/research-development/scientific-data-management/staff/samaneh-jozashoori/>.

<http://research.tib.eu/clarify2020/vocab/surgerySubTypeSpecification>	rdf:type owl:DatatypeProperty;	
									rdfs:label	"surgerySubTypeSpecification";
									rdfs:domain	<http://research.tib.eu/clarify2020/vocab/SurgerySubType>;
									rdfs:range	rdfs:Literal;
									rdfs:comment "Further specification of the surgery subtype.";
									dcterms:modified "2021-05-17"^^xsd:date;
									dcterms:creator <https://www.tib.eu/en/research-development/scientific-data-management/staff/samaneh-jozashoori/>.

<http://research.tib.eu/clarify2020/vocab/age>	rdf:type owl:DatatypeProperty;	
				rdfs:label	"age";
				rdfs:domain	<http://research.tib.eu/clarify2020/vocab/CPatient>;
				rdfs:range	rdfs:Literal;
				rdfs:comment "Indicates the calculated age of the patient.";
				dcterms:modified "2021-06-02"^^xsd:date;
				dcterms:creator <https://www.tib.eu/en/research-development/scientific-data-management/staff/samaneh-jozashoori/>.

<http://research.tib.eu/clarify2020/vocab/categoryDescription>	rdf:type owl:DatatypeProperty;	
							rdfs:label	"categoryDescription";
							rdfs:domain	<http://research.tib.eu/clarify2020/vocab/Concept>;
							rdfs:range	rdfs:Literal;
							rdfs:comment "Represents the desciption of the category to which the patient belong provided by HUPHM.";
							dcterms:modified "2021-11-03"^^xsd:date;
							dcterms:creator <https://www.tib.eu/en/research-development/scientific-data-management/staff/samaneh-jozashoori/>.

<http://research.tib.eu/clarify2020/vocab/hasDiagnosisDate>	rdf:type	owl:DatatypeProperty;
								rdfs:label	"hasDiagnosisDate";
								rdfs:domain	<http://research.tib.eu/clarify2020/vocab/Diagnosis>;
								rdfs:range	rdfs:Literal;
								rdfs:comment "Represents the information regarding the date of diagnosis provided by HUPHM.";
								dcterms:modified "2021-11-05"^^xsd:date;							
								dcterms:creator <https://www.tib.eu/en/research-development/scientific-data-management/staff/samaneh-jozashoori/>.

<http://research.tib.eu/clarify2020/vocab/primaryTumorSize>	rdf:type	owl:DatatypeProperty;
							rdfs:label	"primaryTumorSize";
							rdfs:domain	<http://research.tib.eu/clarify2020/vocab/TumorType>;
							rdfs:range	rdfs:Literal;
							rdfs:comment "Represents the primary size of the tumor.";
							dcterms:modified "2022-02-09"^^xsd:date;							
							dcterms:creator <https://www.tib.eu/en/research-development/scientific-data-management/staff/samaneh-jozashoori/>.

<http://research.tib.eu/clarify2020/vocab/subType>	rdf:type	owl:DatatypeProperty;
				rdfs:label	"subType";
				rdfs:domain	<http://research.tib.eu/clarify2020/vocab/TumorType>;
				rdfs:range	rdfs:Literal;
				rdfs:comment "Represents the subtype of the tumor.";
				dcterms:modified "2022-02-09"^^xsd:date;							
				dcterms:creator <https://www.tib.eu/en/research-development/scientific-data-management/staff/samaneh-jozashoori/>.

<http://research.tib.eu/clarify2020/vocab/percentage>	rdf:type	owl:DatatypeProperty;
					rdfs:label	"percentage";
					rdfs:domain	<http://research.tib.eu/clarify2020/vocab/BiomarkerObservation>;
					rdfs:range	rdfs:Literal;
					rdfs:comment "The percentage of the studied biomarker.";
					dcterms:modified "2022-02-09"^^xsd:date;							
					dcterms:creator <https://www.tib.eu/en/research-development/scientific-data-management/staff/samaneh-jozashoori/>.

<http://research.tib.eu/clarify2020/vocab/ki67>	rdf:type 	owl:DatatypeProperty;	
				rdfs:label	"ki67";
				rdfs:domain	<http://research.tib.eu/clarify2020/vocab/BCPatient>;
				rdfs:range	rdfs:Literal;
				rdfs:comment "The ki67 score calculated as the percentage of the positively malignated cells (percentage of the cells showing malignancy agian all the cells). The higher this score the worse the disease is.";
				dcterms:modified "2022-09-12"^^xsd:date;
				dcterms:creator <https://www.tib.eu/en/research-development/scientific-data-management/staff/samaneh-jozashoori/>.

<http://research.tib.eu/clarify2020/vocab/gravidity>	rdf:type 	owl:DatatypeProperty;	
					rdfs:label	"gravidity";
					rdfs:domain	<http://research.tib.eu/clarify2020/vocab/BCPatient>;
					rdfs:range	rdfs:Literal;
					rdfs:comment "Represents the total number of the pregnancies that the patient has had.";
					dcterms:modified "2022-09-12"^^xsd:date;
					dcterms:creator <https://www.tib.eu/en/research-development/scientific-data-management/staff/samaneh-jozashoori/>.

<http://research.tib.eu/clarify2020/vocab/abortion>	rdf:type 	owl:DatatypeProperty;	
				rdfs:label	"ki67";
				rdfs:domain	<http://research.tib.eu/clarify2020/vocab/BCPatient>;
				rdfs:range	rdfs:Literal;
				rdfs:comment "Represents the number of abortion that the patient has had.";
				dcterms:modified "2022-09-12"^^xsd:date;
				dcterms:creator <https://www.tib.eu/en/research-development/scientific-data-management/staff/samaneh-jozashoori/>.

<http://research.tib.eu/clarify2020/vocab/parity>	rdf:type 	owl:DatatypeProperty;	
				rdfs:label	"parity";
				rdfs:domain	<http://research.tib.eu/clarify2020/vocab/BCPatient>;
				rdfs:range	rdfs:Literal;
				rdfs:comment "Represents the number of the pregnancies that the patient has had which ended with giving birth.";
				dcterms:modified "2022-09-12"^^xsd:date;
				dcterms:creator <https://www.tib.eu/en/research-development/scientific-data-management/staff/samaneh-jozashoori/>.

<http://research.tib.eu/clarify2020/vocab/cSection>	rdf:type 	owl:DatatypeProperty;	
					rdfs:label	"cSection";
					rdfs:domain	<http://research.tib.eu/clarify2020/vocab/BCPatient>;
					rdfs:range	rdfs:Literal;
					rdfs:comment "The number of the C section that the patient has had.";
					dcterms:modified "2022-09-12"^^xsd:date;
					dcterms:creator <https://www.tib.eu/en/research-development/scientific-data-management/staff/samaneh-jozashoori/>.

<http://research.tib.eu/clarify2020/vocab/hasEarlyMenopause>	rdf:type 	owl:DatatypeProperty;	
							rdfs:label	"hasEarlyMenopause";
							rdfs:domain	<http://research.tib.eu/clarify2020/vocab/BCPatient>;
							rdfs:range	rdfs:Literal;
							rdfs:comment "Represents if the patient has had an early-age menopause.";
							dcterms:modified "2022-09-12"^^xsd:date;
							dcterms:creator <https://www.tib.eu/en/research-development/scientific-data-management/staff/samaneh-jozashoori/>.

<http://research.tib.eu/clarify2020/vocab/surgeryYear>	rdf:type 	owl:DatatypeProperty;	
					rdfs:label	"surgeryYear";
					rdfs:domain	<http://research.tib.eu/clarify2020/vocab/BCPatient>;
					rdfs:range	rdfs:Literal;
					rdfs:comment "Represents if the patient has had an early-age menopause.";
					dcterms:modified "2022-09-12"^^xsd:date;
					dcterms:creator <https://www.tib.eu/en/research-development/scientific-data-management/staff/samaneh-jozashoori/>.

<http://research.tib.eu/clarify2020/vocab/surgeryMonth>	rdf:type 	owl:DatatypeProperty;	
						rdfs:label	"surgeryMonth";
						rdfs:domain	<http://research.tib.eu/clarify2020/vocab/BCPatient>;
						rdfs:range	rdfs:Literal;
						rdfs:comment "Represents if the patient has had an early-age menopause.";
						dcterms:modified "2022-09-12"^^xsd:date;
						dcterms:creator <https://www.tib.eu/en/research-development/scientific-data-management/staff/samaneh-jozashoori/>.

<http://research.tib.eu/clarify2020/vocab/surgeryDay>	rdf:type 	owl:DatatypeProperty;	
					rdfs:label	"surgeryDay";
					rdfs:domain	<http://research.tib.eu/clarify2020/vocab/BCPatient>;
					rdfs:range	rdfs:Literal;
					rdfs:comment "Represents if the patient has had an early-age menopause.";
					dcterms:modified "2022-09-12"^^xsd:date;
					dcterms:creator <https://www.tib.eu/en/research-development/scientific-data-management/staff/samaneh-jozashoori/>.

<http://research.tib.eu/clarify2020/vocab/isAssessedDuring>	rdf:type 	owl:DatatypeProperty;	
							rdfs:label	"isAssessedDuring";
							rdfs:domain	<http://research.tib.eu/clarify2020/vocab/TNMstageAssessment>;
							rdfs:range	rdfs:Literal;
							rdfs:comment "Indicates when the TNM stage is assessed (for instance at the diagnosis time).";
							dcterms:modified "2022-09-12"^^xsd:date;
							dcterms:creator <https://www.tib.eu/en/research-development/scientific-data-management/staff/samaneh-jozashoori/>.

<http://research.tib.eu/clarify2020/vocab/hasStage>	rdf:type 	owl:DatatypeProperty;	
					rdfs:label	"hasStage";
					rdfs:domain	<http://research.tib.eu/clarify2020/vocab/TNMstageAssessment>;
					rdfs:range	rdfs:Literal;
					rdfs:comment "Represents the stage.";
					dcterms:modified "2022-09-12"^^xsd:date;
					dcterms:creator <https://www.tib.eu/en/research-development/scientific-data-management/staff/samaneh-jozashoori/>.

<http://research.tib.eu/clarify2020/vocab/tumorGrade>	rdf:type 	owl:DatatypeProperty;	
					rdfs:label	"tumorGrade";
					rdfs:domain	<http://research.tib.eu/clarify2020/vocab/CPatient>;
					rdfs:range	rdfs:Literal;
					rdfs:comment "Represents the tumor grade of the patient.";
					dcterms:modified "2022-09-12"^^xsd:date;
					dcterms:creator <https://www.tib.eu/en/research-development/scientific-data-management/staff/samaneh-jozashoori/>.

<http://research.tib.eu/clarify2020/vocab/diagnosisDate>	rdf:type 	owl:DatatypeProperty;	
						rdfs:label	"diagnosisDate";
						rdfs:domain	<http://research.tib.eu/clarify2020/vocab/CPatient>;
						rdfs:range	rdfs:Literal;
						rdfs:comment "Represents the date of the diagnosis.";
						dcterms:modified "2023-01-11"^^xsd:date;
						dcterms:creator <https://www.tib.eu/en/research-development/scientific-data-management/staff/samaneh-jozashoori/>.

<http://research.tib.eu/clarify2020/vocab/deathAge>	rdf:type 	owl:DatatypeProperty;	
					rdfs:label	"deathAge";
					rdfs:domain	<http://research.tib.eu/clarify2020/vocab/CPatient>;
					rdfs:range	rdfs:Literal;
					rdfs:comment "Represents the age at which the cancer patient was died.";
					dcterms:modified "2023-01-11"^^xsd:date;
					dcterms:creator <https://www.tib.eu/en/research-development/scientific-data-management/staff/samaneh-jozashoori/>.

<http://research.tib.eu/clarify2020/vocab/relapseYear>	rdf:type 	owl:DatatypeProperty;	
						rdfs:label	"relapseYear";
						rdfs:domain	<http://research.tib.eu/clarify2020/vocab/CPatient>;
						rdfs:range	rdfs:Literal;
						rdfs:comment "Represents the year at which the cancer patient had a relapse.";
						dcterms:modified "2023-01-11"^^xsd:date;
						dcterms:creator <https://www.tib.eu/en/research-development/scientific-data-management/staff/samaneh-jozashoori/>.

<http://research.tib.eu/clarify2020/vocab/isAssessedOn>	rdf:type 	owl:DatatypeProperty;	
						rdfs:label	"isAssessedOn";
						rdfs:domain	<http://research.tib.eu/clarify2020/vocab/Assessment>;
						rdfs:range	rdfs:Literal;
						rdfs:comment "Represents the date of the diagnosis.";
						dcterms:modified "2023-01-11"^^xsd:date;
						dcterms:creator <https://www.tib.eu/en/research-development/scientific-data-management/staff/samaneh-jozashoori/>.

<http://research.tib.eu/clarify2020/vocab/surgeryDate>	rdf:type 	owl:DatatypeProperty;	
					rdfs:label	"surgeryDate";
					rdfs:domain	<http://research.tib.eu/clarify2020/vocab/OncologicalSurgery>;
					rdfs:range	rdfs:Literal;
					rdfs:comment "Represents the date of the surgery.";
					dcterms:modified "2023-01-11"^^xsd:date;
					dcterms:creator <https://www.tib.eu/en/research-development/scientific-data-management/staff/samaneh-jozashoori/>.

<http://research.tib.eu/clarify2020/vocab/tumorSize_staging_method>	rdf:type 	owl:DatatypeProperty;	
									rdfs:label	"tumorSize_staging_method";
									rdfs:domain	<http://research.tib.eu/clarify2020/vocab/TumorSize>;
									rdfs:range	rdfs:Literal;
									rdfs:comment "Represents the staging method by which the tumor size is assessed.";
									dcterms:modified "2023-01-11"^^xsd:date;
									dcterms:creator <https://www.tib.eu/en/research-development/scientific-data-management/staff/samaneh-jozashoori/>.

<http://research.tib.eu/clarify2020/vocab/tumorSize_staging_category>	rdf:type 	owl:DatatypeProperty;	
									rdfs:label	"tumorSize_staging_category";
									rdfs:domain	<http://research.tib.eu/clarify2020/vocab/TumorSize>;
									rdfs:range	rdfs:Literal;
									rdfs:comment "Represents the staging category according to which the tumor size is assessed.";
									dcterms:modified "2023-01-11"^^xsd:date;
									dcterms:creator <https://www.tib.eu/en/research-development/scientific-data-management/staff/samaneh-jozashoori/>.

<http://research.tib.eu/clarify2020/vocab/lymphNodesInvolvement_staging_method>	rdf:type 	owl:DatatypeProperty;	
												rdfs:label	"lymphNodesInvolvement_staging_method";
												rdfs:domain	<http://research.tib.eu/clarify2020/vocab/LymphNodesInvolvement>;
												rdfs:range	rdfs:Literal;
												rdfs:comment "Represents the staging method by which the lymph involvement is assessed.";
												dcterms:modified "2023-01-11"^^xsd:date;
												dcterms:creator <https://www.tib.eu/en/research-development/scientific-data-management/staff/samaneh-jozashoori/>.

<http://research.tib.eu/clarify2020/vocab/lymphNodesInvolvement_staging_category>	rdf:type 	owl:DatatypeProperty;	
									rdfs:label	"lymphNodesInvolvement_staging_category";
									rdfs:domain	<http://research.tib.eu/clarify2020/vocab/LymphNodesInvolvement>;
									rdfs:range	rdfs:Literal;
									rdfs:comment "Represents the staging category according to which the lymph involvement is assessed.";
									dcterms:modified "2023-01-11"^^xsd:date;
									dcterms:creator <https://www.tib.eu/en/research-development/scientific-data-management/staff/samaneh-jozashoori/>.

<http://research.tib.eu/clarify2020/vocab/metastatisStage_staging_category>	rdf:type 	owl:DatatypeProperty;	
											rdfs:label	"metastatisStage_staging_category";
											rdfs:domain	<http://research.tib.eu/clarify2020/vocab/MetastatisStage>;
											rdfs:range	rdfs:Literal;
											rdfs:comment "Represents the staging category according to which the metastatis stage is assessed.";
											dcterms:modified "2023-01-11"^^xsd:date;
											dcterms:creator <https://www.tib.eu/en/research-development/scientific-data-management/staff/samaneh-jozashoori/>.

######################################################################################################################################
#####################################################    Annotation    ##############################################################
######################################################################################################################################

<http://research.tib.eu/clarify2020/vocab/annID>	rdf:type	owl:DatatypeProperty;
				rdfs:label	"annID";
				rdfs:domain <http://research.tib.eu/clarify2020/vocab/Annotation>;
				rdfs:range	rdfs:Literal;
				rdfs:comment	"Identification of instances of Annotation class";	
				dcterms:modified "2020-11-19"^^xsd:date;
				dcterms:creator <https://www.tib.eu/en/research-development/scientific-data-management/staff/samaneh-jozashoori/>.

<http://research.tib.eu/clarify2020/vocab/definition>	rdf:type	owl:DatatypeProperty;
						rdfs:label	"definition";
						rdfs:domain <http://research.tib.eu/clarify2020/vocab/Concept>;
						rdfs:range	rdfs:Literal;
						rdfs:comment	"Definition that is provided by UMLS";	
						dcterms:modified "2021-12-16"^^xsd:date;
						dcterms:creator <https://www.tib.eu/en/research-development/scientific-data-management/staff/samaneh-jozashoori/>.

<http://research.tib.eu/clarify2020/vocab/semanticTypeLabel>	rdf:type	owl:DatatypeProperty;
							rdfs:label	"semanticTypeLabel";
							rdfs:domain <http://research.tib.eu/clarify2020/vocab/SemanticType>;
							rdfs:range	rdfs:Literal;
							rdfs:comment	"The label of the UMLS semantic type.";	
							dcterms:modified "2021-12-16"^^xsd:date;
							dcterms:creator <https://www.tib.eu/en/research-development/scientific-data-management/staff/samaneh-jozashoori/>.

<http://research.tib.eu/clarify2020/vocab/typeGroup>	rdf:type	owl:DatatypeProperty;
							rdfs:label	"typeGroup";
							rdfs:domain <http://research.tib.eu/clarify2020/vocab/SemanticTypeGroup>;
							rdfs:range	rdfs:Literal;
							rdfs:comment	"The group of the UMLS CUI type.";	
							dcterms:modified "2021-12-16"^^xsd:date;
							dcterms:creator <https://www.tib.eu/en/research-development/scientific-data-management/staff/samaneh-jozashoori/>.

<http://research.tib.eu/clarify2020/vocab/annotationFrequency>	rdf:type	owl:DatatypeProperty;
							rdfs:label	"annotationFrequency";
							rdfs:domain <http://research.tib.eu/clarify2020/vocab/Annotation>;
							rdfs:range	rdfs:Literal;
							rdfs:comment	"The frequency of the UMLS CUI.";	
							dcterms:modified "2021-12-16"^^xsd:date;
							dcterms:creator <https://www.tib.eu/en/research-development/scientific-data-management/staff/samaneh-jozashoori/>.

######################################################################################################################################
#####################################################    Publication    ##############################################################
######################################################################################################################################

<http://research.tib.eu/clarify2020/vocab/pubmedID>	rdf:type owl:DatatypeProperty;
					rdfs:label "PubMed ID";
					rdfs:domain <http://research.tib.eu/clarify2020/vocab/Publication>;
				  	rdfs:range rdfs:Literal;
					rdfs:comment "PubMed ID.";
					dcterms:modified "2020-12-15"^^xsd:date;
					dcterms:creator <https://www.tib.eu/en/research-development/scientific-data-management/staff/samaneh-jozashoori/>.

<http://research.tib.eu/clarify2020/vocab/confidence>    rdf:type     owl:DatatypeProperty;
					rdfs:label	"confidence";
					rdfs:domain	<http://research.tib.eu/clarify2020/vocab/Concept>;
					rdfs:range	rdfs:Literal;
					rdfs:comment "Confidence score of the concept";
					dcterms:modified "2020-12-15"^^xsd:date;
					dcterms:creator <https://www.tib.eu/en/research-development/scientific-data-management/staff/samaneh-jozashoori/>.

<http://research.tib.eu/clarify2020/vocab/semanticType>	rdf:type	owl:DatatypeProperty;
					rdfs:label	"semanticType";
					rdfs:domain	<http://research.tib.eu/clarify2020/vocab/Annotation>;
					rdfs:range	rdfs:Literal;
					rdfs:comment	"A list with the allowed semantic_types for this Annotation in the UMLS.";
					dcterms:modified "2020-12-15"^^xsd:date;
					dcterms:creator <https://www.tib.eu/en/research-development/scientific-data-management/staff/samaneh-jozashoori/>.

<http://research.tib.eu/clarify2020/vocab/year>	rdf:type owl:DatatypeProperty;
				rdfs:label "year";
				rdfs:domain <http://research.tib.eu/clarify2020/vocab/Publication>;
			  	rdfs:range rdfs:Literal;
				rdfs:comment "Year of Publication.";
				dcterms:modified "2021-05-17"^^xsd:date;
				dcterms:creator <https://www.tib.eu/en/research-development/scientific-data-management/staff/samaneh-jozashoori/>.

<http://research.tib.eu/clarify2020/vocab/authorName>	rdf:type owl:DatatypeProperty;
					rdfs:label "authorName";
					rdfs:domain <http://research.tib.eu/clarify2020/vocab/Author>;
				  	rdfs:range rdfs:Literal;
					rdfs:comment "Name of author.";
					dcterms:modified "2021-05-17"^^xsd:date;
					dcterms:creator <https://www.tib.eu/en/research-development/scientific-data-management/staff/samaneh-jozashoori/>.

<http://research.tib.eu/clarify2020/vocab/rankingScore_SJR>	rdf:type owl:DatatypeProperty;
							rdfs:label "rankingScore_SJR";
							rdfs:domain <http://research.tib.eu/clarify2020/vocab/Publication>;
						  	rdfs:range rdfs:Literal;
							rdfs:comment "ranking Score_SJR Journal of publication.";
							dcterms:modified "2021-05-17"^^xsd:date;
							dcterms:creator <https://www.tib.eu/en/research-development/scientific-data-management/staff/samaneh-jozashoori/>.

<http://research.tib.eu/clarify2020/vocab/rankingScore_hIndex>	rdf:type owl:DatatypeProperty;
							rdfs:label "rankingScore_hIndex";
							rdfs:domain <http://research.tib.eu/clarify2020/vocab/Publication>;
						  	rdfs:range rdfs:Literal;
							rdfs:comment "ranking Score_hIndex of Journal of publication.";
							dcterms:modified "2021-05-17"^^xsd:date;
							dcterms:creator <https://www.tib.eu/en/research-development/scientific-data-management/staff/samaneh-jozashoori/>.

<http://research.tib.eu/clarify2020/vocab/publicationTypeName>	rdf:type owl:DatatypeProperty;
							rdfs:label "publicationTypeName";
							rdfs:domain <http://research.tib.eu/clarify2020/vocab/PublicationType>;
						  	rdfs:range rdfs:Literal;
							rdfs:comment "Represents the name of the publication type.";
							dcterms:modified "2021-11-17"^^xsd:date;
							dcterms:creator <https://www.tib.eu/en/research-development/scientific-data-management/staff/samaneh-jozashoori/>.

<http://research.tib.eu/clarify2020/vocab/title>	rdf:type owl:DatatypeProperty;
				rdfs:label "title";
				rdfs:domain <http://research.tib.eu/clarify2020/vocab/Publication>;
			  	rdfs:range rdfs:Literal;
				rdfs:comment "Represents the title of the publication.";
				dcterms:modified "2021-11-17"^^xsd:date;
				dcterms:creator <https://www.tib.eu/en/research-development/scientific-data-management/staff/samaneh-jozashoori/>.

<http://research.tib.eu/clarify2020/vocab/citedBy>	rdf:type owl:DatatypeProperty;
							rdfs:label "citedBy";
							rdfs:domain <http://research.tib.eu/clarify2020/vocab/PublicationType>;
						  	rdfs:range rdfs:Literal;
							rdfs:comment "Represents the citation of the publication type.";
							dcterms:modified "2021-11-17"^^xsd:date;
							dcterms:creator <https://www.tib.eu/en/research-development/scientific-data-management/staff/samaneh-jozashoori/>.

<http://research.tib.eu/clarify2020/vocab/citedByLink>	rdf:type owl:DatatypeProperty;
					rdfs:label "citedByLink";
					rdfs:domain <http://research.tib.eu/clarify2020/vocab/PublicationType>;
				  	rdfs:range rdfs:Literal;
					rdfs:comment "Represents the citation link of the publication type.";
					dcterms:modified "2021-11-17"^^xsd:date;
					dcterms:creator <https://www.tib.eu/en/research-development/scientific-data-management/staff/samaneh-jozashoori/>.


######################################################################################################################################
#########################################################    Drug    #################################################################
######################################################################################################################################

<http://research.tib.eu/clarify2020/vocab/annLabel>	rdf:type	owl:DatatypeProperty;
					rdfs:label	"annLabel";
					rdfs:domain	<http://research.tib.eu/clarify2020/vocab/Annotation>;
					rdfs:range	rdfs:Literal;
					rdfs:comment	"Label of instances of Annotation class";
					dcterms:modified "2020-12-15"^^xsd:date;
					dcterms:creator <https://www.tib.eu/en/research-development/scientific-data-management/staff/samaneh-jozashoori/>.

<http://research.tib.eu/clarify2020/vocab/annLabel_SPA>	rdf:type	owl:DatatypeProperty;
						rdfs:label	"annLabel_SPA";
						rdfs:domain	<http://research.tib.eu/clarify2020/vocab/Annotation>;
						rdfs:range	rdfs:Literal;
						rdfs:comment "Spanish label of instances of Annotation class";
						dcterms:modified "2022-02-09"^^xsd:date;
						dcterms:creator <https://www.tib.eu/en/research-development/scientific-data-management/staff/samaneh-jozashoori/>.

<http://research.tib.eu/clarify2020/vocab/drugLabel>	rdf:type owl:DatatypeProperty;
					rdfs:label "DrugLabel";
					rdfs:domain <http://research.tib.eu/clarify2020/vocab/Drug>;
				  	rdfs:range rdfs:Literal;
					rdfs:comment "Drug label.";
					dcterms:modified "2020-12-15"^^xsd:date;
					dcterms:creator <https://www.tib.eu/en/research-development/scientific-data-management/staff/samaneh-jozashoori/>.

<http://research.tib.eu/clarify2020/vocab/drugBankID>	rdf:type	owl:DatatypeProperty;
					rdfs:label "DrugBankID";
					rdfs:domain <http://research.tib.eu/clarify2020/vocab/Drug>;
				  	rdfs:range rdfs:Literal;
					rdfs:comment "Drug Bank ID.";
					dcterms:modified "2020-12-15"^^xsd:date;
					dcterms:creator <https://www.tib.eu/en/research-development/scientific-data-management/staff/samaneh-jozashoori/>.

<http://research.tib.eu/clarify2020/vocab/biomarkerLabel>	rdf:type	owl:DatatypeProperty;
				rdfs:label	"biomarkerLabel";
				rdfs:domain	<http://research.tib.eu/clarify2020/vocab/Biomarker>;
				rdfs:range	rdfs:Literal;
				rdfs:comment	"The name of biomarker.";
				dcterms:modified "2020-12-15"^^xsd:date;
				dcterms:creator <https://www.tib.eu/en/research-development/scientific-data-management/staff/samaneh-jozashoori/>.

<http://research.tib.eu/clarify2020/vocab/targetID>	rdf:type	owl:DatatypeProperty;
					rdfs:label "targetID";
					rdfs:domain <http://research.tib.eu/clarify2020/vocab/Target>;
				  	rdfs:range rdfs:Literal;
					rdfs:comment "Target ID.";
					dcterms:modified "2020-12-15"^^xsd:date;
					dcterms:creator <https://www.tib.eu/en/research-development/scientific-data-management/staff/samaneh-jozashoori/>.

<http://research.tib.eu/clarify2020/vocab/targetLabel>	rdf:type	owl:DatatypeProperty;
				rdfs:label	"targetLabel";
				rdfs:domain	<http://research.tib.eu/clarify2020/vocab/Target>;
				rdfs:range	rdfs:Literal;
				rdfs:comment	"Target Label";
				dcterms:modified "2020-12-15"^^xsd:date;
				dcterms:creator <https://www.tib.eu/en/research-development/scientific-data-management/staff/samaneh-jozashoori/>.

<http://research.tib.eu/clarify2020/vocab/proteinID>	rdf:type owl:DatatypeProperty;
					rdfs:label	"proteinID";
					rdfs:domain <http://research.tib.eu/clarify2020/vocab/Protein>;
					rdfs:range rdfs:Literal;
					rdfs:comment	"Uniprot Accession key for protein.";
					dcterms:modified "2020-12-15"^^xsd:date;
					dcterms:creator <https://www.tib.eu/en/research-development/scientific-data-management/staff/samaneh-jozashoori/>.

<http://research.tib.eu/clarify2020/vocab/proteinLabel>	rdf:type owl:DatatypeProperty;
					rdfs:label	"proteinLabel";
					rdfs:domain <http://research.tib.eu/clarify2020/vocab/Protein>;
					rdfs:range rdfs:Literal;
					rdfs:comment "Represents the name of protein.";
					dcterms:modified "2020-12-15"^^xsd:date;
					dcterms:creator <https://www.tib.eu/en/research-development/scientific-data-management/staff/samaneh-jozashoori/>.

<http://research.tib.eu/clarify2020/vocab/enzymeID>	rdf:type owl:DatatypeProperty;
					rdfs:label "EnzymeID";
					rdfs:domain <http://research.tib.eu/clarify2020/vocab/Enzyme>;
				  	rdfs:range rdfs:Literal;
					rdfs:comment "Enzyme ID.";
					dcterms:modified "2020-12-15"^^xsd:date;
					dcterms:creator <https://www.tib.eu/en/research-development/scientific-data-management/staff/samaneh-jozashoori/>.

<http://research.tib.eu/clarify2020/vocab/enzymeLabel>	rdf:type owl:DatatypeProperty;
					rdfs:label "EnzymeLabel";
					rdfs:domain <http://research.tib.eu/clarify2020/vocab/Enzyme>;
				  	rdfs:range rdfs:Literal;
					rdfs:comment "Enzyme Label.";
					dcterms:modified "2020-12-15"^^xsd:date;
					dcterms:creator <https://www.tib.eu/en/research-development/scientific-data-management/staff/samaneh-jozashoori/>.

<http://research.tib.eu/clarify2020/vocab/disorderLabel>	rdf:type	owl:DatatypeProperty;
					rdfs:label "DisorderLabel";
					rdfs:domain <http://research.tib.eu/clarify2020/vocab/Disorder>;
				  	rdfs:range rdfs:Literal;
					rdfs:comment "Disorder Label.";
					dcterms:modified "2020-09-14"^^xsd:date;
					dcterms:creator <https://www.tib.eu/en/research-development/scientific-data-management/staff/samaneh-jozashoori/>.

<http://research.tib.eu/clarify2020/vocab/targetID>	rdf:type	owl:DatatypeProperty;
					rdfs:label "targetID";
					rdfs:domain <http://research.tib.eu/clarify2020/vocab/Target>;
				  	rdfs:range rdfs:Literal;
					rdfs:comment "Target ID.";
					dcterms:modified "2020-09-14"^^xsd:date;
					dcterms:creator <https://www.tib.eu/en/research-development/scientific-data-management/staff/samaneh-jozashoori/>.
					
<http://research.tib.eu/clarify2020/vocab/targetLabel>	rdf:type	owl:DatatypeProperty;
				rdfs:label	"targetLabel";
				rdfs:domain	<http://research.tib.eu/clarify2020/vocab/Target>;
				rdfs:range	rdfs:Literal;
				rdfs:comment	"Target Label";
				dcterms:modified "2020-09-14"^^xsd:date;
				dcterms:creator <https://www.tib.eu/en/research-development/scientific-data-management/staff/samaneh-jozashoori/>.

<http://research.tib.eu/clarify2020/vocab/phenotypeLabel>	rdf:type owl:DatatypeProperty;
					rdfs:label "PhenotypeLabel";
					rdfs:domain <http://research.tib.eu/clarify2020/vocab/Phenotype>;
				  	rdfs:range rdfs:Literal;
					rdfs:comment "Phenotype Label.";
					dcterms:modified "2020-12-15"^^xsd:date;
					dcterms:creator <https://www.tib.eu/en/research-development/scientific-data-management/staff/samaneh-jozashoori/>.

<http://research.tib.eu/clarify2020/vocab/toxicityType>	rdf:type owl:DatatypeProperty;
					rdfs:label "toxicityType";
					rdfs:domain <http://research.tib.eu/clarify2020/vocab/Phenotype>;
				  	rdfs:range rdfs:Literal;
					rdfs:comment "Toxicity Label.";
					dcterms:modified "2020-12-15"^^xsd:date;
					dcterms:creator <https://www.tib.eu/en/research-development/scientific-data-management/staff/samaneh-jozashoori/>.

<http://research.tib.eu/clarify2020/vocab/externalLink>	rdf:type owl:DatatypeProperty;
					rdfs:label "externalLink";
					rdfs:domain <http://research.tib.eu/clarify2020/vocab/Concept>;
				  	rdfs:range xsd:anyURI;
					rdfs:comment "Link to external resources.";
					dcterms:modified "2020-12-15"^^xsd:date;
					dcterms:creator <https://www.tib.eu/en/research-development/scientific-data-management/staff/samaneh-jozashoori/>.

<http://research.tib.eu/clarify2020/vocab/uniprotID>	rdf:type	owl:DatatypeProperty;
					rdfs:label "uniprotID";
					rdfs:domain <http://research.tib.eu/clarify2020/vocab/Concept>;
				  	rdfs:range rdfs:Literal;
					rdfs:comment "External relationship to accession ID in uniprot.";
					dcterms:modified "2020-12-15"^^xsd:date;
					dcterms:creator <https://www.tib.eu/en/research-development/scientific-data-management/staff/samaneh-jozashoori/>.

<http://research.tib.eu/clarify2020/vocab/dse_AvgFrequency>	rdf:type	owl:DatatypeProperty;
							rdfs:label	"dse_AvgFrequency";
							rdfs:domain	<http://research.tib.eu/clarify2020/vocab/DrugSideEffectInteraction>;
							rdfs:range	rdfs:Literal;
							rdfs:comment	"Represents the average frequecy of particular drug having specific side effect.";
							dcterms:modified "2020-12-15"^^xsd:date;
							dcterms:creator <https://www.tib.eu/en/research-development/scientific-data-management/staff/samaneh-jozashoori/>.

<http://research.tib.eu/clarify2020/vocab/ddi_description>	rdf:type	owl:DatatypeProperty;
						rdfs:label	"ddi_description";
						rdfs:domain	<http://research.tib.eu/clarify2020/vocab/DrugDrugInteraction>;
						rdfs:range	rdfs:Literal;
						rdfs:comment "The texual description of the drug drug interacion.";
						dcterms:modified "2021-06-29"^^xsd:date;
						dcterms:creator <https://www.tib.eu/en/research-development/scientific-data-management/staff/samaneh-jozashoori/>.	

<http://research.tib.eu/clarify2020/vocab/drugAbsorption>	rdf:type	owl:DatatypeProperty;
						rdfs:label	"drugAbsorption";
						rdfs:domain	<http://research.tib.eu/clarify2020/vocab/Drug>;
						rdfs:range	rdfs:Literal;
						rdfs:comment "The texual explanation about the drug absorption.";
						dcterms:modified "2021-06-29"^^xsd:date;
						dcterms:creator <https://www.tib.eu/en/research-development/scientific-data-management/staff/samaneh-jozashoori/>.	

<http://research.tib.eu/clarify2020/vocab/drugsMechanismOfAction>	rdf:type	owl:DatatypeProperty;
								rdfs:label	"drugsMechanismOfAction";
								rdfs:domain	<http://research.tib.eu/clarify2020/vocab/Drug>;
								rdfs:range	rdfs:Literal;
								rdfs:comment "The texual explanation about the mechanism of action of the drug.";
								dcterms:modified "2021-06-29"^^xsd:date;
								dcterms:creator <https://www.tib.eu/en/research-development/scientific-data-management/staff/samaneh-jozashoori/>.	




######################################################################################################################################
#################################################    Drug Predictions   ##############################################################
######################################################################################################################################

<http://research.tib.eu/clarify2020/vocab/predictionMethod>	rdf:type	owl:DatatypeProperty;
							rdfs:label	"predictionMethod";
							rdfs:domain	<http://research.tib.eu/clarify2020/vocab/Interaction>;
							rdfs:range	rdfs:Literal;
							rdfs:comment "Represents the prediction method that is used in order to extract DDI predictions from literature or databases.";
							dcterms:modified "2021-01-07"^^xsd:date;
							dcterms:creator <https://www.tib.eu/en/research-development/scientific-data-management/staff/samaneh-jozashoori/>.	

<http://research.tib.eu/clarify2020/vocab/methodAbbreviation>	rdf:type	owl:DatatypeProperty;
							rdfs:label	"methodAbbreviation";
							rdfs:domain	<http://research.tib.eu/clarify2020/vocab/Interaction>;
							rdfs:range	rdfs:Literal;
							rdfs:comment "Represents the abbreviation of the prediction method that is used.";
							dcterms:modified "2021-01-07"^^xsd:date;
							dcterms:creator <https://www.tib.eu/en/research-development/scientific-data-management/staff/samaneh-jozashoori/>.

<http://research.tib.eu/clarify2020/vocab/total_number_of_metastasis>	rdf:type	owl:DatatypeProperty;
									rdfs:label	"total_number_of_metastasis";
									rdfs:domain	<http://research.tib.eu/clarify2020/vocab/LCPatient>;
									rdfs:range	rdfs:Literal;
									rdfs:comment "Indicates the total number of metastasis of the patient.";
									dcterms:modified "2021-04-29"^^xsd:date;
									dcterms:creator <https://www.tib.eu/en/research-development/scientific-data-management/staff/samaneh-jozashoori/>.


#################################################################################################################################################																																			
#################################################################################################################################################
#################################################################################################################################################
#################################################### Properties - relationships #################################################################
#################################################################################################################################################
#################################################################################################################################################
#################################################################################################################################################


######################################################################################################################################
##########################################################    Clinical    ################################################################
######################################################################################################################################

<http://research.tib.eu/clarify2020/vocab/sex>	rdf:type	owl:ObjectProperty;
			rdfs:label	"sex";
			rdfs:domain	<http://research.tib.eu/clarify2020/vocab/CPatient>;
			rdfs:range	<http://research.tib.eu/clarify2020/vocab/Sex>;
			rdfs:comment	"Association of the patient to one of the two main biological categories of female or male.";
			dcterms:modified "2020-10-19"^^xsd:date;
			dcterms:creator <https://www.tib.eu/en/research-development/scientific-data-management/staff/samaneh-jozashoori/>.	

<http://research.tib.eu/clarify2020/vocab/hasRace>	rdf:type	owl:ObjectProperty;
				rdfs:label	"hasRace";
				rdfs:domain	<http://research.tib.eu/clarify2020/vocab/CPatient>;
				rdfs:range	<http://research.tib.eu/clarify2020/vocab/Race>;
				rdfs:comment	"Association of the patient with one of the categories of humankind that shares certain distinctive physical traits.";
				dcterms:modified "2020-11-16"^^xsd:date;
				dcterms:creator <https://www.tib.eu/en/research-development/scientific-data-management/staff/samaneh-jozashoori/>.		

<http://research.tib.eu/clarify2020/vocab/hasBiomarker>	rdf:type	owl:ObjectProperty;
						rdfs:label	"hasBiomarker";
						rdfs:domain	<http://research.tib.eu/clarify2020/vocab/Concept>;
						rdfs:range	<http://research.tib.eu/clarify2020/vocab/Biomarker>;
						rdfs:comment "Associates a cancer patient with an observed biomarker.";
						dcterms:modified "2020-10-19"^^xsd:date;						
						dcterms:creator <https://www.tib.eu/en/research-development/scientific-data-management/staff/samaneh-jozashoori/>.						

<http://research.tib.eu/clarify2020/vocab/hasBio>	rdf:type	owl:ObjectProperty;
						rdfs:label	"hasBio";
						rdfs:domain	<http://research.tib.eu/clarify2020/vocab/CancerPatient>;
						rdfs:range	<http://research.tib.eu/clarify2020/vocab/Biomarker>;
						rdfs:comment "Associates a cancer patient with an observed biomarker.";
						dcterms:modified "2020-10-19"^^xsd:date;						
						dcterms:creator <https://www.tib.eu/en/research-development/scientific-data-management/staff/samaneh-jozashoori/>.						

<http://research.tib.eu/clarify2020/vocab/involved_in>	rdf:type	owl:ObjectProperty;
								rdfs:label	"involved_in";
								rdfs:domain	<http://research.tib.eu/clarify2020/vocab/CPatient>;
								rdfs:range	<http://research.tib.eu/clarify2020/vocab/ClinicalTrial>;
								rdfs:comment "Relation between the cancer patient and the clinical trial.";
								dcterms:modified "2020-10-20"^^xsd:date;								
								dcterms:creator <https://www.tib.eu/en/research-development/scientific-data-management/staff/samaneh-jozashoori/>.	

<http://research.tib.eu/clarify2020/vocab/hasDiagnosisStage>	rdf:type	owl:ObjectProperty;
								rdfs:label	"hasDiagnosisStage";
								rdfs:domain	<http://research.tib.eu/clarify2020/vocab/Diagnosis>;
								rdfs:range	<http://research.tib.eu/clarify2020/vocab/CancerStage>;
								rdfs:comment "Relation between the diagnosis observation and the coded cancer stage (at the diagnosis time).";
								dcterms:modified "2020-12-10"^^xsd:date;							
								dcterms:creator <https://www.tib.eu/en/research-development/scientific-data-management/staff/samaneh-jozashoori/>.

<http://research.tib.eu/clarify2020/vocab/hasDiagnosis>	rdf:type     owl:ObjectProperty;
						rdfs:label	"hasDiagnosis";
						rdfs:domain	<http://research.tib.eu/clarify2020/vocab/CPatient>;
						rdfs:range	<http://research.tib.eu/clarify2020/vocab/Diagnosis>;
						rdfs:comment "Patient's initial diagnosis.";
						dcterms:modified "2020-10-20"^^xsd:date;
						dcterms:creator <https://www.tib.eu/en/research-development/scientific-data-management/staff/samaneh-jozashoori/>.			

<http://research.tib.eu/clarify2020/vocab/hasOncologicalTreatmentLine>      rdf:type     owl:ObjectProperty;
										rdfs:label	"hasOncologicalTreatmentLine";
										rdfs:domain	<http://research.tib.eu/clarify2020/vocab/LCPatient>;
										rdfs:range	<http://research.tib.eu/clarify2020/vocab/OncologicalTreatmentLine>;
										rdfs:comment "Relation between the patient and the oncological treatment line that is received by the patient.";
										dcterms:modified "2020-10-20"^^xsd:date;
										dcterms:creator <https://www.tib.eu/en/research-development/scientific-data-management/staff/samaneh-jozashoori/>.

<http://research.tib.eu/clarify2020/vocab/hasFamilyHistory>	rdf:type        owl:ObjectProperty;	
							rdfs:label	"hasFamilyHistory";
							rdfs:domain	<http://research.tib.eu/clarify2020/vocab/CPatient>;
							rdfs:range	<http://research.tib.eu/clarify2020/vocab/FamilyHistory>;
							rdfs:comment "Connection between patient and her/his family history.";
							dcterms:modified "2020-11-16"^^xsd:date;
							dcterms:creator <https://www.tib.eu/en/research-development/scientific-data-management/staff/samaneh-jozashoori/>.

<http://research.tib.eu/clarify2020/vocab/hasDrug>	rdf:type        owl:ObjectProperty;	
				rdfs:label	"hasDrug";
				rdfs:domain	<http://research.tib.eu/clarify2020/vocab/DrugSchema>;
				rdfs:range	<http://research.tib.eu/clarify2020/vocab/Drug>;
				rdfs:comment "A relation between the oncological treatment line and the prescribed drug.";
				dcterms:modified "2020-10-20"^^xsd:date;
				dcterms:creator <https://www.tib.eu/en/research-development/scientific-data-management/staff/samaneh-jozashoori/>.													

<http://research.tib.eu/clarify2020/vocab/hasDrug1>	rdf:type        owl:ObjectProperty;	
					rdfs:label	"hasDrug";
					rdfs:subPropertyOf <http://research.tib.eu/clarify2020/vocab/hasDrug>;
					rdfs:domain	<http://research.tib.eu/clarify2020/vocab/DrugSchema>;
					rdfs:range	<http://research.tib.eu/clarify2020/vocab/Drug>;
					rdfs:comment "A relation between the oncological treatment line and the prescribed drug.";
					dcterms:modified "2020-10-20"^^xsd:date;
					dcterms:creator <https://www.tib.eu/en/research-development/scientific-data-management/staff/samaneh-jozashoori/>.													

<http://research.tib.eu/clarify2020/vocab/hasDrug2>	rdf:type        owl:ObjectProperty;	
					rdfs:label	"hasDrug";
					rdfs:subPropertyOf <http://research.tib.eu/clarify2020/vocab/hasDrug>;
					rdfs:domain	<http://research.tib.eu/clarify2020/vocab/DrugSchema>;
					rdfs:range	<http://research.tib.eu/clarify2020/vocab/Drug>;
					rdfs:comment "A relation between the oncological treatment line and the prescribed drug.";
					dcterms:modified "2020-10-20"^^xsd:date;
					dcterms:creator <https://www.tib.eu/en/research-development/scientific-data-management/staff/samaneh-jozashoori/>.													

<http://research.tib.eu/clarify2020/vocab/hasDrug3>	rdf:type        owl:ObjectProperty;	
					rdfs:label	"hasDrug";
					rdfs:subPropertyOf <http://research.tib.eu/clarify2020/vocab/hasDrug>;
					rdfs:domain	<http://research.tib.eu/clarify2020/vocab/DrugSchema>;
					rdfs:range	<http://research.tib.eu/clarify2020/vocab/Drug>;
					rdfs:comment "A relation between the oncological treatment line and the prescribed drug.";
					dcterms:modified "2020-10-20"^^xsd:date;
					dcterms:creator <https://www.tib.eu/en/research-development/scientific-data-management/staff/samaneh-jozashoori/>.													

<http://research.tib.eu/clarify2020/vocab/hasDrug4>	rdf:type        owl:ObjectProperty;	
					rdfs:label	"hasDrug";
					rdfs:subPropertyOf <http://research.tib.eu/clarify2020/vocab/hasDrug>;
					rdfs:domain	<http://research.tib.eu/clarify2020/vocab/DrugSchema>;
					rdfs:range	<http://research.tib.eu/clarify2020/vocab/Drug>;
					rdfs:comment "A relation between the oncological treatment line and the prescribed drug.";
					dcterms:modified "2020-10-20"^^xsd:date;
					dcterms:creator <https://www.tib.eu/en/research-development/scientific-data-management/staff/samaneh-jozashoori/>.													

<http://research.tib.eu/clarify2020/vocab/hasDrugSchema>	rdf:type owl:ObjectProperty;	
							rdfs:label	"hasDrugSchema";
							rdfs:domain	<http://research.tib.eu/clarify2020/vocab/CPatient>;
							rdfs:range	<http://research.tib.eu/clarify2020/vocab/DrugSchema>;
							rdfs:comment "A relation between the patient and the combination of the prescribed drugs.";
							dcterms:modified "2022-09-12"^^xsd:date;
							dcterms:creator <https://www.tib.eu/en/research-development/scientific-data-management/staff/samaneh-jozashoori/>.													

<http://research.tib.eu/clarify2020/vocab/hasComorbidity>	rdf:type        owl:ObjectProperty;	
						rdfs:label	"hasComorbidity";
						rdfs:domain	<http://research.tib.eu/clarify2020/vocab/CPatient>;
						rdfs:range	<http://research.tib.eu/clarify2020/vocab/Disorder>;
						rdfs:comment	"Connection between patient and her/his Comorbidities.";
						dcterms:modified "2020-10-21"^^xsd:date;
						dcterms:creator <https://www.tib.eu/en/research-development/scientific-data-management/staff/samaneh-jozashoori/>.

<http://research.tib.eu/clarify2020/vocab/hasTreatmentLineSymptom>	rdf:type        owl:ObjectProperty;	
								rdfs:label	"hasTreatmentLineSymptom";
								rdfs:domain	<http://research.tib.eu/clarify2020/vocab/ComorbidityTreatmentLine>;
								rdfs:range	<http://research.tib.eu/clarify2020/vocab/Disorder>;
								rdfs:comment	"Connection between the ComorbidityTreatmentLine and the observed Comorbidities.";
								dcterms:modified "2021-06-22"^^xsd:date;
								dcterms:creator <https://www.tib.eu/en/research-development/scientific-data-management/staff/samaneh-jozashoori/>.

<http://research.tib.eu/clarify2020/vocab/hasNonOncologicalConsultation>	rdf:type        owl:ObjectProperty;	
						rdfs:label	"hasNonOncologicalConsultation";
						rdfs:domain	<http://research.tib.eu/clarify2020/vocab/CPatient>;
						rdfs:range	<http://research.tib.eu/clarify2020/vocab/NonOncologicalConsultation>;
						rdfs:comment	"Connection between patient and her/his non-oncological consultation that have had.";
						dcterms:modified "2020-11-17"^^xsd:date;
						dcterms:creator <https://www.tib.eu/en/research-development/scientific-data-management/staff/samaneh-jozashoori/>.

<http://research.tib.eu/clarify2020/vocab/hasMontoring>	rdf:type        owl:ObjectProperty;	
						rdfs:label	"hasMontoring";
						rdfs:domain	<http://research.tib.eu/clarify2020/vocab/CPatient>;
						rdfs:range	<http://research.tib.eu/clarify2020/vocab/StatusEvolution>;
						rdfs:comment	"Connection between patient and srvival observation.";
						dcterms:modified "2020-10-21"^^xsd:date;
						dcterms:creator <https://www.tib.eu/en/research-development/scientific-data-management/staff/samaneh-jozashoori/>.		

<http://research.tib.eu/clarify2020/vocab/hasTreatmentLineCycle>	rdf:type	owl:ObjectProperty;
							rdfs:label	"treatmentLineCycle";
							rdfs:domain	<http://research.tib.eu/clarify2020/vocab/Episode>;
							rdfs:range	<http://research.tib.eu/clarify2020/vocab/TreatmentLineCycle>;
							rdfs:comment "Represents the number of cycles through which the corresponding drugs have been applied.";
							dcterms:modified "2022-09-12"^^xsd:date;														
							dcterms:creator <https://www.tib.eu/en/research-development/scientific-data-management/staff/samaneh-jozashoori/>.

<http://research.tib.eu/clarify2020/vocab/familyType>	rdf:type	owl:ObjectProperty;
					rdfs:label	"familyType";
					rdfs:domain	<http://research.tib.eu/clarify2020/vocab/FamilyHistory>;
					rdfs:range	<http://research.tib.eu/clarify2020/vocab/FamilyType>;
					rdfs:comment "Represents the type of family kinship with the patient.";
					dcterms:modified "2021-02-25"^^xsd:date;							
					dcterms:creator <https://www.tib.eu/en/research-development/scientific-data-management/staff/samaneh-jozashoori/>.

<http://research.tib.eu/clarify2020/vocab/familyRelationDegree>	rdf:type	owl:ObjectProperty;
								rdfs:label	"familyRelationDegree";
								rdfs:domain	<http://research.tib.eu/clarify2020/vocab/FamilyHistory>;
								rdfs:range	<http://research.tib.eu/clarify2020/vocab/FamilyRelationDegree>;
								rdfs:comment "Represents the relative degree of the family member with the patient.";
								dcterms:modified "2021-07-26"^^xsd:date;							
								dcterms:creator <https://www.tib.eu/en/research-development/scientific-data-management/staff/samaneh-jozashoori/>.

<http://research.tib.eu/clarify2020/vocab/hasTestResult>	rdf:type owl:ObjectProperty;	
							rdfs:label	"hasTestResult";
							rdfs:domain	<http://research.tib.eu/clarify2020/vocab/Concept>;
							rdfs:range	<http://research.tib.eu/clarify2020/vocab/BiomarkerTestResult>;
							rdfs:comment "Indicates a positive test result.";
							dcterms:modified "2021-02-25"^^xsd:date;
							dcterms:creator <https://www.tib.eu/en/research-development/scientific-data-management/staff/samaneh-jozashoori/>.

<http://research.tib.eu/clarify2020/vocab/hasTestIHQResult>	rdf:type owl:ObjectProperty;	
							rdfs:label	"hasTestIHQResult";
							rdfs:domain	<http://research.tib.eu/clarify2020/vocab/Biomarker>;
							rdfs:range	<http://research.tib.eu/clarify2020/vocab/BiomarkerTestResult>;
							rdfs:comment	"Indicates a positive results of the Test IHQ.";
							dcterms:modified "2021-03-02"^^xsd:date;
							dcterms:creator <https://www.tib.eu/en/research-development/scientific-data-management/staff/samaneh-jozashoori/>.

<http://research.tib.eu/clarify2020/vocab/hasTestFISHResult>	rdf:type owl:ObjectProperty;	
							rdfs:label	"hasTestFISHResult";
							rdfs:domain	<http://research.tib.eu/clarify2020/vocab/Biomarker>;
							rdfs:range	<http://research.tib.eu/clarify2020/vocab/BiomarkerTestResult>;
							rdfs:comment	"Indicates a positive results of the Test FISH.";
							dcterms:modified "2021-03-02"^^xsd:date;
							dcterms:creator <https://www.tib.eu/en/research-development/scientific-data-management/staff/samaneh-jozashoori/>.

<http://research.tib.eu/clarify2020/vocab/hasTestRNAResult>	rdf:type owl:ObjectProperty;	
							rdfs:label	"hasTestRNAResult";
							rdfs:domain	<http://research.tib.eu/clarify2020/vocab/Biomarker>;
							rdfs:range	<http://research.tib.eu/clarify2020/vocab/BiomarkerTestResult>;
							rdfs:comment	"Indicates a positive results of the Test RNA.";
							dcterms:modified "2021-03-02"^^xsd:date;
							dcterms:creator <https://www.tib.eu/en/research-development/scientific-data-management/staff/samaneh-jozashoori/>.

<http://research.tib.eu/clarify2020/vocab/hasBestResponse>	rdf:type owl:ObjectProperty;	
						rdfs:label	"hasBestResponse";
						rdfs:domain	<http://research.tib.eu/clarify2020/vocab/OncologicalTreatmentLine>;
						rdfs:range	<http://research.tib.eu/clarify2020/vocab/TreatementLineBestResponse>;
						rdfs:comment	"Indicates the best response in the treatment line of a oncological.";
						dcterms:modified "2021-02-25"^^xsd:date;
						dcterms:creator <https://www.tib.eu/en/research-development/scientific-data-management/staff/samaneh-jozashoori/>.

<http://research.tib.eu/clarify2020/vocab/hasType>	rdf:type owl:ObjectProperty;	
				rdfs:label	"hasType";
				rdfs:domain	<http://research.tib.eu/clarify2020/vocab/Concept>;
				rdfs:range	<http://research.tib.eu/clarify2020/vocab/Concept>;
				rdfs:comment	"Indicates the type of the oncological treatment.";
				dcterms:modified "2021-02-25"^^xsd:date;
				dcterms:creator <https://www.tib.eu/en/research-development/scientific-data-management/staff/samaneh-jozashoori/>.

<http://research.tib.eu/clarify2020/vocab/is_directed_OrNot>	rdf:type owl:ObjectProperty;	
							rdfs:label	"is_directed_OrNot";
							rdfs:domain	<http://research.tib.eu/clarify2020/vocab/ClinicalTrial>;
							rdfs:range	<http://research.tib.eu/clarify2020/vocab/TrialType>;
							rdfs:comment	"Indicates if the trial is direct or not.";
							dcterms:modified "2021-02-25"^^xsd:date;
							dcterms:creator <https://www.tib.eu/en/research-development/scientific-data-management/staff/samaneh-jozashoori/>.

<http://research.tib.eu/clarify2020/vocab/biomarker>	rdf:type owl:ObjectProperty;	
							rdfs:label	"biomarker";
							rdfs:domain	<http://research.tib.eu/clarify2020/vocab/BiomarkerObservation>;
							rdfs:range	<http://research.tib.eu/clarify2020/vocab/Biomarker>;
							rdfs:comment	"Indicates the connection between the observation and the relevant studied biomarker.";
							dcterms:modified "2022-09-12"^^xsd:date;
							dcterms:creator <https://www.tib.eu/en/research-development/scientific-data-management/staff/samaneh-jozashoori/>.

<http://research.tib.eu/clarify2020/vocab/hasPhase>	rdf:type owl:ObjectProperty;	
					rdfs:label	"hasPhase";
					rdfs:domain	<http://research.tib.eu/clarify2020/vocab/ClinicalTrial>;
					rdfs:range	<http://research.tib.eu/clarify2020/vocab/TrialPhase>;
					rdfs:comment	"Indicates the phase of a clinical trial.";
					dcterms:modified "2021-02-25"^^xsd:date;
					dcterms:creator <https://www.tib.eu/en/research-development/scientific-data-management/staff/samaneh-jozashoori/>.

<http://research.tib.eu/clarify2020/vocab/has_mutation_T790M_positive_result>	rdf:type owl:ObjectProperty;	
											rdfs:label	"has_mutation_T790M_positive_result";
											rdfs:domain	<http://research.tib.eu/clarify2020/vocab/Biomarker>;
											rdfs:range	<http://research.tib.eu/clarify2020/vocab/BiomarkerTestResult>;
											rdfs:comment	"Indicates a positive result of the mutation EGFR T790M.";
											dcterms:modified "2021-03-02"^^xsd:date;
											dcterms:creator <https://www.tib.eu/en/research-development/scientific-data-management/staff/samaneh-jozashoori/>.

<http://research.tib.eu/clarify2020/vocab/has_mutation_T790M_negative_result>	rdf:type owl:ObjectProperty;	
											rdfs:label	"has_mutation_T790M_negative_result";
											rdfs:domain	<http://research.tib.eu/clarify2020/vocab/Biomarker>;
											rdfs:range	<http://research.tib.eu/clarify2020/vocab/BiomarkerTestResult>;
											rdfs:comment	"Indicates a negative result of the mutation EGFR T790M.";
											dcterms:modified "2021-03-02"^^xsd:date;
											dcterms:creator <https://www.tib.eu/en/research-development/scientific-data-management/staff/samaneh-jozashoori/>.

<http://research.tib.eu/clarify2020/vocab/has_mutation_exon19_result>	rdf:type owl:ObjectProperty;	
									rdfs:label	"has_mutation_exon19_result";
									rdfs:domain	<http://research.tib.eu/clarify2020/vocab/Biomarker>;
									rdfs:range	<http://research.tib.eu/clarify2020/vocab/BiomarkerTestResult>;
									rdfs:comment	"Indicates a positive result of the mutation EGFR in exon19.";
									dcterms:modified "2021-03-02"^^xsd:date;
									dcterms:creator <https://www.tib.eu/en/research-development/scientific-data-management/staff/samaneh-jozashoori/>.

<http://research.tib.eu/clarify2020/vocab/has_mutation_exon21_result>	rdf:type owl:ObjectProperty;	
									rdfs:label	"has_mutation_exon21_result";
									rdfs:domain	<http://research.tib.eu/clarify2020/vocab/Biomarker>;
									rdfs:range	<http://research.tib.eu/clarify2020/vocab/BiomarkerTestResult>;
									rdfs:comment	"Indicates a positive result of the mutation EGFR in exon21.";
									dcterms:modified "2021-03-02"^^xsd:date;
									dcterms:creator <https://www.tib.eu/en/research-development/scientific-data-management/staff/samaneh-jozashoori/>.

<http://research.tib.eu/clarify2020/vocab/has_performed_study>	rdf:type owl:ObjectProperty;	
							rdfs:label	"has_performed_study";
							rdfs:domain	<http://research.tib.eu/clarify2020/vocab/Biomarker>;
							rdfs:range	<http://research.tib.eu/clarify2020/vocab/PerformedStudyStatus>;
							rdfs:comment	"Connect the biomarker to the indication of performed study.";
							dcterms:modified "2021-04-07"^^xsd:date;
							dcterms:creator <https://www.tib.eu/en/research-development/scientific-data-management/staff/samaneh-jozashoori/>.


<http://research.tib.eu/clarify2020/vocab/hasNegativeTestResult>	rdf:type owl:ObjectProperty;	
								rdfs:label	"hasNegativeTestResult";
								rdfs:domain	<http://research.tib.eu/clarify2020/vocab/Biomarker>;
								rdfs:range	<http://research.tib.eu/clarify2020/vocab/BiomarkerTestResult>;
								rdfs:comment	"Indicates a negative result.";
								dcterms:modified "2021-03-02"^^xsd:date;
								dcterms:creator <https://www.tib.eu/en/research-development/scientific-data-management/staff/samaneh-jozashoori/>.

<http://research.tib.eu/clarify2020/vocab/has_familyWithCancer_OrNot>	rdf:type owl:ObjectProperty;	
									rdfs:label	"has_familyWithCancer_OrNot";
									rdfs:domain	<http://research.tib.eu/clarify2020/vocab/CPatient>;
									rdfs:range	<http://research.tib.eu/clarify2020/vocab/FamilyWithCancer>;
									rdfs:comment "Indicates if the patient has a family with cancer or not.";
									dcterms:modified "2021-02-25"^^xsd:date;
									dcterms:creator <https://www.tib.eu/en/research-development/scientific-data-management/staff/samaneh-jozashoori/>.

<http://research.tib.eu/clarify2020/vocab/hasFamilyCancerType>	rdf:type owl:ObjectProperty;	
							rdfs:label	"hasFamilyCancerType";
							rdfs:domain	<http://research.tib.eu/clarify2020/vocab/CPatient>;
							rdfs:range	<http://research.tib.eu/clarify2020/vocab/CancerType>;
							rdfs:comment "Indicates the type of cancer of the relatives.";
							dcterms:modified "2021-02-25"^^xsd:date;
							dcterms:creator <https://www.tib.eu/en/research-development/scientific-data-management/staff/samaneh-jozashoori/>.

<http://research.tib.eu/clarify2020/vocab/hasSymptom>	rdf:type owl:ObjectProperty;	
					rdfs:label	"hasSymptom";
					rdfs:domain	<http://research.tib.eu/clarify2020/vocab/Concept>;
					rdfs:range	<http://research.tib.eu/clarify2020/vocab/Phenotype>;
					rdfs:comment	"Indicates the symptoms that a person had.";
					dcterms:modified "2021-02-25"^^xsd:date;
					dcterms:creator <https://www.tib.eu/en/research-development/scientific-data-management/staff/samaneh-jozashoori/>.

<http://research.tib.eu/clarify2020/vocab/patient_is_asymptomatic>	rdf:type owl:ObjectProperty;	
								rdfs:label	"patient_is_asymptomatic";
								rdfs:domain	<http://research.tib.eu/clarify2020/vocab/Observation>;
								rdfs:range	<http://research.tib.eu/clarify2020/vocab/Phenotype>;
								rdfs:comment	"Indicates if the patient had no symptom before the first consultation in Oncology.";
								dcterms:modified "2021-02-25"^^xsd:date;
								dcterms:creator <https://www.tib.eu/en/research-development/scientific-data-management/staff/samaneh-jozashoori/>.

<http://research.tib.eu/clarify2020/vocab/has_cancer_metastasized_to_extrathoracic_lymphadenopaties>	rdf:type owl:ObjectProperty;	
																	rdfs:label	"has_cancer_metastasized_to_extrathoracic_lymphadenopaties";
																	rdfs:domain	<http://research.tib.eu/clarify2020/vocab/CPatient>;
																	rdfs:range	<http://research.tib.eu/clarify2020/vocab/MetastasisLocation>;
																	rdfs:comment	"Associates the patient with the location (extrathoracic lymphadenopaties) to where the cancer is metastasized.";
																	dcterms:modified "2022-02-09"^^xsd:date;
																	dcterms:creator <https://www.tib.eu/en/research-development/scientific-data-management/staff/samaneh-jozashoori/>.

<http://research.tib.eu/clarify2020/vocab/has_cancer_metastasized_to_thoracic_lymphadenopaties>	rdf:type owl:ObjectProperty;	
																	rdfs:label	"has_cancer_metastasized_to_thoracic_lymphadenopaties";
																	rdfs:domain	<http://research.tib.eu/clarify2020/vocab/CPatient>;
																	rdfs:range	<http://research.tib.eu/clarify2020/vocab/MetastasisLocation>;
																	rdfs:comment	"Associates the patient with the location (thoracic lymphadenopaties) to where the cancer is metastasized.";
																	dcterms:modified "2022-02-09"^^xsd:date;
																	dcterms:creator <https://www.tib.eu/en/research-development/scientific-data-management/staff/samaneh-jozashoori/>.

<http://research.tib.eu/clarify2020/vocab/has_cancer_metastasized_to_meningeal_carcinomatosis>	rdf:type owl:ObjectProperty;	
															rdfs:label	"has_cancer_metastasized_to_meningeal_carcinomatosis";
															rdfs:domain	<http://research.tib.eu/clarify2020/vocab/CPatient>;
															rdfs:range	<http://research.tib.eu/clarify2020/vocab/MetastasisLocation>;
															rdfs:comment	"Associates the patient with the location (meningeal carcinomatosis) to where the cancer is metastasized.";
															dcterms:modified "2022-02-09"^^xsd:date;
															dcterms:creator <https://www.tib.eu/en/research-development/scientific-data-management/staff/samaneh-jozashoori/>.

<http://research.tib.eu/clarify2020/vocab/has_cancer_metastasized_to_pericardial_effusion>	rdf:type owl:ObjectProperty;	
														rdfs:label	"has_cancer_metastasized_to_pericardial_effusion";
														rdfs:domain	<http://research.tib.eu/clarify2020/vocab/CPatient>;
														rdfs:range	<http://research.tib.eu/clarify2020/vocab/MetastasisLocation>;
														rdfs:comment	"Associates the patient with the location (pericardial effusion) to where the cancer is metastasized.";
														dcterms:modified "2022-02-09"^^xsd:date;
														dcterms:creator <https://www.tib.eu/en/research-development/scientific-data-management/staff/samaneh-jozashoori/>.

<http://research.tib.eu/clarify2020/vocab/has_cancer_metastasized_to_pleural_effusion>	rdf:type owl:ObjectProperty;	
													rdfs:label	"has_cancer_metastasized_to_pleural_effusion";
													rdfs:domain	<http://research.tib.eu/clarify2020/vocab/CPatient>;
													rdfs:range	<http://research.tib.eu/clarify2020/vocab/MetastasisLocation>;
													rdfs:comment	"Associates the patient with the location (pleural effusion) to where the cancer is metastasized.";
													dcterms:modified "2022-02-09"^^xsd:date;
													dcterms:creator <https://www.tib.eu/en/research-development/scientific-data-management/staff/samaneh-jozashoori/>.

<http://research.tib.eu/clarify2020/vocab/has_cancer_metastasized_to_liver>	rdf:type owl:ObjectProperty;	
											rdfs:label	"has_cancer_metastasized_to_liver";
											rdfs:domain	<http://research.tib.eu/clarify2020/vocab/CPatient>;
											rdfs:range	<http://research.tib.eu/clarify2020/vocab/MetastasisLocation>;
											rdfs:comment	"Associates the patient with the location (liver) to where the cancer is metastasized.";
											dcterms:modified "2022-02-09"^^xsd:date;
											dcterms:creator <https://www.tib.eu/en/research-development/scientific-data-management/staff/samaneh-jozashoori/>.

<http://research.tib.eu/clarify2020/vocab/has_cancer_metastasized_to_bone>	rdf:type owl:ObjectProperty;	
										rdfs:label	"has_cancer_metastasized_to_bone";
										rdfs:domain	<http://research.tib.eu/clarify2020/vocab/CPatient>;
										rdfs:range	<http://research.tib.eu/clarify2020/vocab/MetastasisLocation>;
										rdfs:comment	"Associates the patient with the location (bone) to where the cancer is metastasized.";
										dcterms:modified "2022-02-09"^^xsd:date;
										dcterms:creator <https://www.tib.eu/en/research-development/scientific-data-management/staff/samaneh-jozashoori/>.

<http://research.tib.eu/clarify2020/vocab/has_cancer_metastasized_to_bilateral>	rdf:type owl:ObjectProperty;	
												rdfs:label	"has_cancer_metastasized_to_bilateral";
												rdfs:domain	<http://research.tib.eu/clarify2020/vocab/CPatient>;
												rdfs:range	<http://research.tib.eu/clarify2020/vocab/MetastasisLocation>;
												rdfs:comment	"Associates the patient with the location (bilateral) to where the cancer is metastasized.";
												dcterms:modified "2022-02-09"^^xsd:date;
												dcterms:creator <https://www.tib.eu/en/research-development/scientific-data-management/staff/samaneh-jozashoori/>.

<http://research.tib.eu/clarify2020/vocab/has_cancer_metastasized_to_pleural_nodules>	rdf:type owl:ObjectProperty;	
													rdfs:label	"has_cancer_metastasized_to_pleural_nodules";
													rdfs:domain	<http://research.tib.eu/clarify2020/vocab/CPatient>;
													rdfs:range	<http://research.tib.eu/clarify2020/vocab/MetastasisLocation>;
													rdfs:comment	"Associates the patient with the location (pleural nodules) to where the cancer is metastasized.";
													dcterms:modified "2022-02-09"^^xsd:date;
													dcterms:creator <https://www.tib.eu/en/research-development/scientific-data-management/staff/samaneh-jozashoori/>.

<http://research.tib.eu/clarify2020/vocab/has_cancer_metastasized_to_pancreatic>	rdf:type owl:ObjectProperty;	
												rdfs:label	"has_cancer_metastasized_to_pancreatic";
												rdfs:domain	<http://research.tib.eu/clarify2020/vocab/CPatient>;
												rdfs:range	<http://research.tib.eu/clarify2020/vocab/MetastasisLocation>;
												rdfs:comment	"Associates the patient with the location (pancreatic) to where the cancer is metastasized.";
												dcterms:modified "2022-02-09"^^xsd:date;
												dcterms:creator <https://www.tib.eu/en/research-development/scientific-data-management/staff/samaneh-jozashoori/>.

<http://research.tib.eu/clarify2020/vocab/has_cancer_metastasized_to_peritoneal>	rdf:type owl:ObjectProperty;	
												rdfs:label	"has_cancer_metastasized_to_peritoneal";
												rdfs:domain	<http://research.tib.eu/clarify2020/vocab/CPatient>;
												rdfs:range	<http://research.tib.eu/clarify2020/vocab/MetastasisLocation>;
												rdfs:comment	"Associates the patient with the location (peritoneal) to where the cancer is metastasized.";
												dcterms:modified "2022-02-09"^^xsd:date;
												dcterms:creator <https://www.tib.eu/en/research-development/scientific-data-management/staff/samaneh-jozashoori/>.

<http://research.tib.eu/clarify2020/vocab/has_cancer_metastasized_to_lung>	rdf:type owl:ObjectProperty;	
										rdfs:label	"has_cancer_metastasized_to_lung";
										rdfs:domain	<http://research.tib.eu/clarify2020/vocab/CPatient>;
										rdfs:range	<http://research.tib.eu/clarify2020/vocab/MetastasisLocation>;
										rdfs:comment	"Associates the patient with the location (lung) to where the cancer is metastasized.";
										dcterms:modified "2022-02-09"^^xsd:date;
										dcterms:creator <https://www.tib.eu/en/research-development/scientific-data-management/staff/samaneh-jozashoori/>.

<http://research.tib.eu/clarify2020/vocab/has_cancer_metastasized_to_central_nervous_system>	rdf:type owl:ObjectProperty;	
															rdfs:label	"has_cancer_metastasized_to_central_nervous_system";
															rdfs:domain	<http://research.tib.eu/clarify2020/vocab/CPatient>;
															rdfs:range	<http://research.tib.eu/clarify2020/vocab/MetastasisLocation>;
															rdfs:comment	"Associates the patient with the location (central nervous system) to where the cancer is metastasized.";
															dcterms:modified "2022-02-09"^^xsd:date;
															dcterms:creator <https://www.tib.eu/en/research-development/scientific-data-management/staff/samaneh-jozashoori/>.

<http://research.tib.eu/clarify2020/vocab/has_cancer_metastasized_to_subcutaneous>	rdf:type owl:ObjectProperty;	
												rdfs:label	"has_cancer_metastasized_to_subcutaneous";
												rdfs:domain	<http://research.tib.eu/clarify2020/vocab/CPatient>;
												rdfs:range	<http://research.tib.eu/clarify2020/vocab/MetastasisLocation>;
												rdfs:comment	"Associates the patient with the location (subcutaneous) to where the cancer is metastasized.";
												dcterms:modified "2022-02-09"^^xsd:date;
												dcterms:creator <https://www.tib.eu/en/research-development/scientific-data-management/staff/samaneh-jozashoori/>.

<http://research.tib.eu/clarify2020/vocab/has_cancer_metastasized_to_adrenal>	rdf:type owl:ObjectProperty;	
											rdfs:label	"has_cancer_metastasized_to_adrenal";
											rdfs:domain	<http://research.tib.eu/clarify2020/vocab/CPatient>;
											rdfs:range	<http://research.tib.eu/clarify2020/vocab/MetastasisLocation>;
											rdfs:comment	"Associates the patient with the location (adrenal) to where the cancer is metastasized.";
											dcterms:modified "2022-02-09"^^xsd:date;
											dcterms:creator <https://www.tib.eu/en/research-development/scientific-data-management/staff/samaneh-jozashoori/>.

<http://research.tib.eu/clarify2020/vocab/has_cancer_metastasized_to_soft_tissues>	rdf:type owl:ObjectProperty;	
												rdfs:label	"has_cancer_metastasized_to_soft_tissues";
												rdfs:domain	<http://research.tib.eu/clarify2020/vocab/CPatient>;
												rdfs:range	<http://research.tib.eu/clarify2020/vocab/MetastasisLocation>;
												rdfs:comment	"Associates the patient with the location (soft tissues) to where the cancer is metastasized.";
												dcterms:modified "2022-02-09"^^xsd:date;
												dcterms:creator <https://www.tib.eu/en/research-development/scientific-data-management/staff/samaneh-jozashoori/>.

<http://research.tib.eu/clarify2020/vocab/has_cancer_metastasized_to_other_locations>	rdf:type owl:ObjectProperty;	
													rdfs:label	"has_cancer_metastasized_to_other_locations";
													rdfs:domain	<http://research.tib.eu/clarify2020/vocab/CPatient>;
													rdfs:range	<http://research.tib.eu/clarify2020/vocab/MetastasisLocation>;
													rdfs:comment	"Associates the patient with the locations to where the cancer is metastasized.";
													dcterms:modified "2022-02-09"^^xsd:date;
													dcterms:creator <https://www.tib.eu/en/research-development/scientific-data-management/staff/samaneh-jozashoori/>.

<http://research.tib.eu/clarify2020/vocab/hasReasonOfDeath>	rdf:type owl:ObjectProperty;	
							rdfs:label	"hasReasonOfDeath";
							rdfs:domain	<http://research.tib.eu/clarify2020/vocab/StatusEvolution>;
							rdfs:range	<http://research.tib.eu/clarify2020/vocab/ReasonOfDeath>;
							rdfs:comment  "Indicates the reason of the death.";
							dcterms:modified "2021-02-25"^^xsd:date;
							dcterms:creator <https://www.tib.eu/en/research-development/scientific-data-management/staff/samaneh-jozashoori/>.

<http://research.tib.eu/clarify2020/vocab/hasCurrentStatus>	rdf:type owl:ObjectProperty;	
							rdfs:label	"hasCurrentStatus";
							rdfs:domain	<http://research.tib.eu/clarify2020/vocab/StatusEvolution>;
							rdfs:range	<http://research.tib.eu/clarify2020/vocab/CurrentStatus>;
							rdfs:comment	"Indicates the current status of Lung Cancer patient.";
							dcterms:modified "2021-02-25"^^xsd:date;
							dcterms:creator <https://www.tib.eu/en/research-development/scientific-data-management/staff/samaneh-jozashoori/>.

<http://research.tib.eu/clarify2020/vocab/hasCauseOfDeath>	rdf:type owl:ObjectProperty;	
						rdfs:label	"hasCauseOfDeath";
						rdfs:domain	<http://research.tib.eu/clarify2020/vocab/StatusEvolution>;
						rdfs:range	<http://research.tib.eu/clarify2020/vocab/CauseOfDeath>;
						rdfs:comment	"Indicates the cause of death, lung cancer or others.";
						dcterms:modified "2021-02-25"^^xsd:date;
						dcterms:creator <https://www.tib.eu/en/research-development/scientific-data-management/staff/samaneh-jozashoori/>.

<http://research.tib.eu/clarify2020/vocab/has_previousCancerHistory_OrNot>	rdf:type owl:ObjectProperty;	
										rdfs:label	"has_previousCancerHistory_OrNot";
										rdfs:domain	<http://research.tib.eu/clarify2020/vocab/CPatient>;
										rdfs:range	<http://research.tib.eu/clarify2020/vocab/PatientCancerHistory>;
										rdfs:comment "Indicates if the patient has previous cancer history or not.";
										dcterms:modified "2021-02-25"^^xsd:date;
										dcterms:creator <https://www.tib.eu/en/research-development/scientific-data-management/staff/samaneh-jozashoori/>.

<http://research.tib.eu/clarify2020/vocab/hasPreviousCancerType>	rdf:type owl:ObjectProperty;	
								rdfs:label	"hasPreviousCancerType";
								rdfs:domain	<http://research.tib.eu/clarify2020/vocab/CPatient>;
								rdfs:range	<http://research.tib.eu/clarify2020/vocab/CancerType>;
								rdfs:comment "Indicates whicht type of previous cancer.";
								dcterms:modified "2021-02-25"^^xsd:date;
								dcterms:creator <https://www.tib.eu/en/research-development/scientific-data-management/staff/samaneh-jozashoori/>.

<http://research.tib.eu/clarify2020/vocab/hasCurrentCancerType>	rdf:type	owl:ObjectProperty;
								rdfs:label	"hasCurrentCancerType";
								rdfs:domain	<http://research.tib.eu/clarify2020/vocab/CPatient>;
								rdfs:range	<http://research.tib.eu/clarify2020/vocab/CancerType>;
								rdfs:comment	"Indicates the cancer type of the patient.";
								dcterms:modified "2021-02-25"^^xsd:date;								
								dcterms:creator <https://www.tib.eu/en/research-development/scientific-data-management/staff/samaneh-jozashoori/>.

<http://research.tib.eu/clarify2020/vocab/locatedInHospital>	rdf:type	owl:ObjectProperty;
							rdfs:label	"locatedInHospital";
							rdfs:domain	<http://research.tib.eu/clarify2020/vocab/CPatient>;
							rdfs:range	<http://research.tib.eu/clarify2020/vocab/Hospital>;
							rdfs:comment	"Represents the hospital where the patient is assigned.";
							dcterms:modified "2021-02-25"^^xsd:date;							
							dcterms:creator <https://www.tib.eu/en/research-development/scientific-data-management/staff/samaneh-jozashoori/>.

<http://research.tib.eu/clarify2020/vocab/locatedInCity>	rdf:type	owl:ObjectProperty;
						rdfs:label	"locatedInCity";
						rdfs:domain	<http://research.tib.eu/clarify2020/vocab/CPatient>;
						rdfs:range	<http://research.tib.eu/clarify2020/vocab/City>;
						rdfs:comment	"Represents the city where the patient is assigned.";
						dcterms:modified "2021-02-25"^^xsd:date;							
						dcterms:creator <https://www.tib.eu/en/research-development/scientific-data-management/staff/samaneh-jozashoori/>.

<http://research.tib.eu/clarify2020/vocab/is_located_in>	rdf:type	owl:ObjectProperty;
						rdfs:label	"is_located_in";
						rdfs:domain	<http://research.tib.eu/clarify2020/vocab/RadiotherapyTreatmentLine>;
						rdfs:range	<http://research.tib.eu/clarify2020/vocab/RadiotherapyLocation>;
						rdfs:comment	"indicates the irradiated area during radiotherapy.";
						dcterms:modified "2021-02-25"^^xsd:date;							
						dcterms:creator <https://www.tib.eu/en/research-development/scientific-data-management/staff/samaneh-jozashoori/>.

<http://research.tib.eu/clarify2020/vocab/hasIntention>	rdf:type	owl:ObjectProperty;
						rdfs:label	"hasIntention";
						rdfs:domain	<http://research.tib.eu/clarify2020/vocab/RadiotherapyTreatmentLine>;
						rdfs:range	<http://research.tib.eu/clarify2020/vocab/RadiotherapyIntention>;
						rdfs:comment	"Indicates the intention of the radiotherapy.";
						dcterms:modified "2021-02-25"^^xsd:date;							
						dcterms:creator <https://www.tib.eu/en/research-development/scientific-data-management/staff/samaneh-jozashoori/>.

<http://research.tib.eu/clarify2020/vocab/hasProgressionOrRelapse>	rdf:type	owl:ObjectProperty;
								rdfs:label	"hasProgressionOrRelapse";
								rdfs:domain	<http://research.tib.eu/clarify2020/vocab/CPatient>;
								rdfs:range	<http://research.tib.eu/clarify2020/vocab/ProgressionRelapse>;
								rdfs:comment	"Specifies that either of progression or relapse exists.";
								dcterms:modified "2021-05-17"^^xsd:date;							
								dcterms:creator <https://www.tib.eu/en/research-development/scientific-data-management/staff/samaneh-jozashoori/>.

<http://research.tib.eu/clarify2020/vocab/hasTherapyType>	rdf:type	owl:ObjectProperty;
						rdfs:label	"hasTherapyType";
						rdfs:domain	<http://research.tib.eu/clarify2020/vocab/CPatient>;
						rdfs:range	<http://research.tib.eu/clarify2020/vocab/TherapyType>;
						rdfs:comment	"Type of therapy.";
						dcterms:modified "2021-02-25"^^xsd:date;							
						dcterms:creator <https://www.tib.eu/en/research-development/scientific-data-management/staff/samaneh-jozashoori/>.

<http://research.tib.eu/clarify2020/vocab/hasProgressionType>	rdf:type	owl:ObjectProperty;
							rdfs:label	"hasProgressionType";
							rdfs:domain	<http://research.tib.eu/clarify2020/vocab/CPatient>;
							rdfs:range	<http://research.tib.eu/clarify2020/vocab/ProgressionType>;
							rdfs:comment	"Indicates the type of therapy at progression .";
							dcterms:modified "2021-02-25"^^xsd:date;							
							dcterms:creator <https://www.tib.eu/en/research-development/scientific-data-management/staff/samaneh-jozashoori/>.

<http://research.tib.eu/clarify2020/vocab/hasTreatmentLineNumber>	rdf:type	owl:ObjectProperty;
							rdfs:label	"hasProgressionType";
							rdfs:domain	<http://research.tib.eu/clarify2020/vocab/Concept>;
							rdfs:range	<http://research.tib.eu/clarify2020/vocab/TreatmentLineNumber>;
							rdfs:comment	"Indicates the type of patient.";
							dcterms:modified "2021-02-25"^^xsd:date;							
							dcterms:creator <https://www.tib.eu/en/research-development/scientific-data-management/staff/samaneh-jozashoori/>.

<http://research.tib.eu/clarify2020/vocab/hasSmokingHabit>	rdf:type	owl:ObjectProperty;
						rdfs:label	"hasSmokingHabit";
						rdfs:domain	<http://research.tib.eu/clarify2020/vocab/CPatient>;
						rdfs:range	<http://research.tib.eu/clarify2020/vocab/SmokingHabit>;
						rdfs:comment	"Indicates the smoking habit of the patient and people whoe are living/ lived with the patient.";
						dcterms:modified "2021-12-06"^^xsd:date;								
						dcterms:creator <https://www.tib.eu/en/research-development/scientific-data-management/staff/samaneh-jozashoori/>.

<http://research.tib.eu/clarify2020/vocab/hasSmokeEnvironment>	rdf:type	owl:ObjectProperty;
							rdfs:label	"hasSmokeEnvironment";
							rdfs:domain	<http://research.tib.eu/clarify2020/vocab/CPatient>;
							rdfs:range	<http://research.tib.eu/clarify2020/vocab/SmokeEnvironment>;
							rdfs:comment	"Indicates the connection of the patient with exposure to the smoking environment.";
							dcterms:modified "2022-02-16"^^xsd:date;								
							dcterms:creator <https://www.tib.eu/en/research-development/scientific-data-management/staff/samaneh-jozashoori/>.

<http://research.tib.eu/clarify2020/vocab/performedMonitoring_OrNot>	rdf:type	owl:ObjectProperty;
									rdfs:label	"performedMonitoring_OrNot";
									rdfs:domain	<http://research.tib.eu/clarify2020/vocab/StatusEvolution>;
									rdfs:range	<http://research.tib.eu/clarify2020/vocab/PerformedMonitoring>;
									rdfs:comment	"Indicates if the monitoring has been performed on the patient.";
									dcterms:modified "2021-04-29"^^xsd:date;								
									dcterms:creator <https://www.tib.eu/en/research-development/scientific-data-management/staff/samaneh-jozashoori/>.

<http://research.tib.eu/clarify2020/vocab/hasPathologicalResponse>	rdf:type	owl:ObjectProperty;
								rdfs:label	"hasPathologicalResponse";
								rdfs:domain	<http://research.tib.eu/clarify2020/vocab/OncologicalSurgery>;
								rdfs:range	<http://research.tib.eu/clarify2020/vocab/SurgeryPathologicalResponse>;
								rdfs:comment	"Indicates the pathologic response of the patient.";
								dcterms:modified "2021-02-25"^^xsd:date;							
								dcterms:creator <https://www.tib.eu/en/research-development/scientific-data-management/staff/samaneh-jozashoori/>.

<http://research.tib.eu/clarify2020/vocab/hasClass>	rdf:type	owl:ObjectProperty;
					rdfs:label	"hasClass";
					rdfs:domain	<http://research.tib.eu/clarify2020/vocab/OncologicalSurgery>;
					rdfs:range	<http://research.tib.eu/clarify2020/vocab/SurgeryClass>;
					rdfs:comment	"Indicates the class of the surgery.";
					dcterms:modified "2021-02-25"^^xsd:date;							
					dcterms:creator <https://www.tib.eu/en/research-development/scientific-data-management/staff/samaneh-jozashoori/>.

<http://research.tib.eu/clarify2020/vocab/hasSubType>	rdf:type	owl:ObjectProperty;
					rdfs:label	"hasSubType";
					rdfs:domain	<http://research.tib.eu/clarify2020/vocab/OncologicalSurgery>;
					rdfs:range	<http://research.tib.eu/clarify2020/vocab/SurgerySubType>;
					rdfs:comment	"Is the subtype of procedure follow in in a surgery.";
					dcterms:modified "2021-02-25"^^xsd:date;							
					dcterms:creator <https://www.tib.eu/en/research-development/scientific-data-management/staff/samaneh-jozashoori/>.

<http://research.tib.eu/clarify2020/vocab/has_PerioperativeDeath_orNot>	rdf:type	owl:ObjectProperty;
										rdfs:label	"has_PerioperativeDeath_orNot";
										rdfs:domain	<http://research.tib.eu/clarify2020/vocab/OncologicalSurgery>;
										rdfs:range	<http://research.tib.eu/clarify2020/vocab/PerioperativeDeath>;
										rdfs:comment "Indicates if the perioperative death was the cause of death (30 days after surgery).";
										dcterms:modified "2021-02-25"^^xsd:date;							
										dcterms:creator <https://www.tib.eu/en/research-development/scientific-data-management/staff/samaneh-jozashoori/>.

<http://research.tib.eu/clarify2020/vocab/cancerStageTNM_TumorSize>	rdf:type	owl:ObjectProperty;
									rdfs:label	"cancerStageTNM_TumorSize";
									rdfs:domain	<http://research.tib.eu/clarify2020/vocab/CPatient>;
									rdfs:range	<http://research.tib.eu/clarify2020/vocab/TumorSize>;
									rdfs:comment "Associates the cancer stage (based on on TNM system) of the patient with the size of the primary tumor, based on which the cancer stage is evaluated.";
									dcterms:modified "2021-05-11"^^xsd:date;							
									dcterms:creator <https://www.tib.eu/en/research-development/scientific-data-management/staff/samaneh-jozashoori/>.

<http://research.tib.eu/clarify2020/vocab/cancerStageTNM_LymphNodesInvolvement>	rdf:type	owl:ObjectProperty;
												rdfs:label	"cancerStageTNM_LymphNodesInvolvement";
												rdfs:domain	<http://research.tib.eu/clarify2020/vocab/CPatient>;
												rdfs:range	<http://research.tib.eu/clarify2020/vocab/LymphNodesInvolvement>;
												rdfs:comment "Associates the cancer stage (based on on TNM system) of the patient with the involvement of lymph nodes, based on which the cancer stage is evaluated.";
												dcterms:modified "2021-05-11"^^xsd:date;							
												dcterms:creator <https://www.tib.eu/en/research-development/scientific-data-management/staff/samaneh-jozashoori/>.

<http://research.tib.eu/clarify2020/vocab/cancerStageTNM_MetastatisStage>	rdf:type	owl:ObjectProperty;
										rdfs:label	"cancerStageTNM_MetastatisStage";
										rdfs:domain	<http://research.tib.eu/clarify2020/vocab/CPatient>;
										rdfs:range	<http://research.tib.eu/clarify2020/vocab/MetastatisStage>;
										rdfs:comment "Associates the cancer stage (based on on TNM system) of the patient with the metasta stage, based on which the cancer stage is evaluated.";
										dcterms:modified "2021-05-11"^^xsd:date;								
										dcterms:creator <https://www.tib.eu/en/research-development/scientific-data-management/staff/samaneh-jozashoori/>.

<http://research.tib.eu/clarify2020/vocab/cancerStageTNM_Version>	rdf:type	owl:ObjectProperty;
								rdfs:label	"cancerStageTNM_Version";
								rdfs:domain	<http://research.tib.eu/clarify2020/vocab/Concept>;
								rdfs:range	<http://research.tib.eu/clarify2020/vocab/Version>;
								rdfs:comment "Associates the concept with the version, based on which the concept value is provided.";
								dcterms:modified "2021-04-26"^^xsd:date;								
								dcterms:creator <https://www.tib.eu/en/research-development/scientific-data-management/staff/samaneh-jozashoori/>.

<http://research.tib.eu/clarify2020/vocab/basedOn_Scale>	rdf:type	owl:ObjectProperty;
						rdfs:label	"basedOn_Scale";
						rdfs:domain	<http://research.tib.eu/clarify2020/vocab/PerformanceStatusObservation>;
						rdfs:range	<http://research.tib.eu/clarify2020/vocab/Scale>;
						rdfs:comment "Associates the performance status observation with the scale that is considered for the assessment.";
						dcterms:modified "2021-03-03"^^xsd:date;								
						dcterms:creator <https://www.tib.eu/en/research-development/scientific-data-management/staff/samaneh-jozashoori/>.

<http://research.tib.eu/clarify2020/vocab/has_SynchronousTumor_OrNot>	rdf:type	owl:ObjectProperty;
									rdfs:label	"has_SynchronousTumor_OrNot";
									rdfs:domain	<http://research.tib.eu/clarify2020/vocab/CPatient>;
									rdfs:range	<http://research.tib.eu/clarify2020/vocab/SynchronousTumor>;
									rdfs:comment "indicates if a second primary cancer is diagnosed within 6 months of the primary cancer or not.";
									dcterms:modified "2021-02-25"^^xsd:date;								
									dcterms:creator <https://www.tib.eu/en/research-development/scientific-data-management/staff/samaneh-jozashoori/>.

<http://research.tib.eu/clarify2020/vocab/hasMesotheliomaType>	rdf:type	owl:ObjectProperty;
							rdfs:label	"hasMesotheliomaType";
							rdfs:domain	<http://research.tib.eu/clarify2020/vocab/TumorType>;
							rdfs:range	<http://research.tib.eu/clarify2020/vocab/MesotheliomaType>;
							rdfs:comment	"Associates the tumor type with the related subtype mesothelyoma.";
							dcterms:modified "2021-02-25"^^xsd:date;								
							dcterms:creator <https://www.tib.eu/en/research-development/scientific-data-management/staff/samaneh-jozashoori/>.

<http://research.tib.eu/clarify2020/vocab/hasAdenocarcinomaHistology>	rdf:type	owl:ObjectProperty;
									rdfs:label	"hasAdenocarcinomaHistology";
									rdfs:domain	<http://research.tib.eu/clarify2020/vocab/TumorType>;
									rdfs:range	<http://research.tib.eu/clarify2020/vocab/AdenocarcinomaHistology>;
									rdfs:comment	"Associates the tumor type with the related subtype adenocarcinoma.";
									dcterms:modified "2021-02-25"^^xsd:date;								
									dcterms:creator <https://www.tib.eu/en/research-development/scientific-data-management/staff/samaneh-jozashoori/>.

<http://research.tib.eu/clarify2020/vocab/hasCarcinomaType>	rdf:type	owl:ObjectProperty;
							rdfs:label	"hasCarcinomaType";
							rdfs:domain	<http://research.tib.eu/clarify2020/vocab/TumorType>;
							rdfs:range	<http://research.tib.eu/clarify2020/vocab/CarcinomaType>;
							rdfs:comment	"Associates the tumor type with the details of the type of carcinoma.";
							dcterms:modified "2021-02-25"^^xsd:date;							
							dcterms:creator <https://www.tib.eu/en/research-development/scientific-data-management/staff/samaneh-jozashoori/>.

<http://research.tib.eu/clarify2020/vocab/hasHistologyDegree>	rdf:type	owl:ObjectProperty;
							rdfs:label	"hasHistologyDegree";
							rdfs:domain	<http://research.tib.eu/clarify2020/vocab/TumorType>;
							rdfs:range	<http://research.tib.eu/clarify2020/vocab/HistologyDegree>;
							rdfs:comment	"Associates the tumor type with the related degree of the histology.";
							dcterms:modified "2021-02-25"^^xsd:date;							
							dcterms:creator <https://www.tib.eu/en/research-development/scientific-data-management/staff/samaneh-jozashoori/>.

<http://research.tib.eu/clarify2020/vocab/hasSmallCellCarcinomaType>	rdf:type	owl:ObjectProperty;
									rdfs:label	"hasSmallCellCarcinomaType";
									rdfs:domain	<http://research.tib.eu/clarify2020/vocab/TumorType>;
									rdfs:range	<http://research.tib.eu/clarify2020/vocab/SmallCellCarcinomaType>;
									rdfs:comment	"Associates the tumor type with the subtype small cell lung cancer (microcytic).";
									dcterms:modified "2021-02-25"^^xsd:date;							
									dcterms:creator <https://www.tib.eu/en/research-development/scientific-data-management/staff/samaneh-jozashoori/>.

<http://research.tib.eu/clarify2020/vocab/hasSecondNeoplasm>	rdf:type 	owl:ObjectProperty;	
							rdfs:label	"hasSecondNeoplasm";
							rdfs:domain	<http://research.tib.eu/clarify2020/vocab/StatusEvolution>;
							rdfs:range	<http://research.tib.eu/clarify2020/vocab/SecondNeoplasm>;
							rdfs:comment "Associates the status evolution with the information on secondary malignant neoplasm.";
							dcterms:modified "2021-03-18"^^xsd:date;
							dcterms:creator <https://www.tib.eu/en/research-development/scientific-data-management/staff/samaneh-jozashoori/>.

<http://research.tib.eu/clarify2020/vocab/has_other_result>	rdf:type owl:ObjectProperty;	
							rdfs:label	"has_other_result";
							rdfs:domain	<http://research.tib.eu/clarify2020/vocab/Biomarker>;
							rdfs:range	<http://research.tib.eu/clarify2020/vocab/BiomarkerTestResult>;
							rdfs:comment "Assocaites the Biomarker with the other test results.";
							dcterms:modified "2021-03-18"^^xsd:date;
							dcterms:creator <https://www.tib.eu/en/research-development/scientific-data-management/staff/samaneh-jozashoori/>.

<http://research.tib.eu/clarify2020/vocab/has_NOS_result>	rdf:type owl:ObjectProperty;	
						rdfs:label	"has_NOS_result";
						rdfs:domain	<http://research.tib.eu/clarify2020/vocab/Biomarker>;
						rdfs:range	<http://research.tib.eu/clarify2020/vocab/BiomarkerTestResult>;
						rdfs:comment "Associates the Biomarker with NOS(!) test results.";
						dcterms:modified "2021-03-18"^^xsd:date;
						dcterms:creator <https://www.tib.eu/en/research-development/scientific-data-management/staff/samaneh-jozashoori/>.

<http://research.tib.eu/clarify2020/vocab/hasClinicalTrialTreatmentLine>	rdf:type 	owl:ObjectProperty;	
							rdfs:label	"hasClinicalTrialTreatmentLine";
							rdfs:domain	<http://research.tib.eu/clarify2020/vocab/CPatient>;
							rdfs:range	<http://research.tib.eu/clarify2020/vocab/ClinicalTrialTreatmentLine>;
							rdfs:comment "Associates Patient with treatment line of the clinical trial .";
							dcterms:modified "2021-05-17"^^xsd:date;
							dcterms:creator <https://www.tib.eu/en/research-development/scientific-data-management/staff/samaneh-jozashoori/>.

<http://research.tib.eu/clarify2020/vocab/hasComorbidityStatus>	rdf:type 	owl:ObjectProperty;	
								rdfs:label	"hasComorbidityStatus";
								rdfs:domain	<http://research.tib.eu/clarify2020/vocab/CPatient>;
								rdfs:range	<http://research.tib.eu/clarify2020/vocab/ComorbidityStatus>;
								rdfs:comment "Associates Patient with the comorbidity status.";
								dcterms:modified "2021-05-17"^^xsd:date;
								dcterms:creator <https://www.tib.eu/en/research-development/scientific-data-management/staff/samaneh-jozashoori/>.

<http://research.tib.eu/clarify2020/vocab/hasSecondNeoplasmType>	rdf:type 	owl:ObjectProperty;	
								rdfs:label	"hasSecondNeoplasmType";
								rdfs:domain	<http://research.tib.eu/clarify2020/vocab/StatusEvolution>;
								rdfs:range	<http://research.tib.eu/clarify2020/vocab/SecondNeoplasmType>;
								rdfs:comment "Associates Patient with second neoplasm type.";
								dcterms:modified "2021-05-17"^^xsd:date;
								dcterms:creator <https://www.tib.eu/en/research-development/scientific-data-management/staff/samaneh-jozashoori/>.

<http://research.tib.eu/clarify2020/vocab/hasPerformanceStatus>	rdf:type 	owl:ObjectProperty;	
								rdfs:label	"hasPerformanceStatus";
								rdfs:domain	<http://research.tib.eu/clarify2020/vocab/CPatient>;
								rdfs:range	<http://research.tib.eu/clarify2020/vocab/PerformanceStatus>;
								rdfs:comment "Associates Patient with her/his performance status.";
								dcterms:modified "2021-05-17"^^xsd:date;
								dcterms:creator <https://www.tib.eu/en/research-development/scientific-data-management/staff/samaneh-jozashoori/>.

<http://research.tib.eu/clarify2020/vocab/hasStudiedBiomarker>	rdf:type 	owl:ObjectProperty;	
							rdfs:label	"hasStudiedBiomarker";
							rdfs:domain	<http://research.tib.eu/clarify2020/vocab/CPatient>;
							rdfs:range	<http://research.tib.eu/clarify2020/vocab/Biomarker>;
							rdfs:comment "Associates Patient with the studied biomarkers.";
							dcterms:modified "2021-05-17"^^xsd:date;
							dcterms:creator <https://www.tib.eu/en/research-development/scientific-data-management/staff/samaneh-jozashoori/>.

<http://research.tib.eu/clarify2020/vocab/hasBiomarkerTestResult>	rdf:type 	owl:ObjectProperty;	
								rdfs:label	"hasBiomarkerTestResult";
								rdfs:domain	<http://research.tib.eu/clarify2020/vocab/CPatient>;
								rdfs:range	<http://research.tib.eu/clarify2020/vocab/BiomarkerTestResult>;
								rdfs:comment "Associates Patient with the result of the studied biomarkers.";
								dcterms:modified "2021-05-17"^^xsd:date;
								dcterms:creator <https://www.tib.eu/en/research-development/scientific-data-management/staff/samaneh-jozashoori/>.

<http://research.tib.eu/clarify2020/vocab/hasSurgeryIteration>	rdf:type 	owl:ObjectProperty;	
							rdfs:label	"hasSurgeryIteration";
							rdfs:domain	<http://research.tib.eu/clarify2020/vocab/SurgerySubType>;
							rdfs:range	<http://research.tib.eu/clarify2020/vocab/SurgeryIteration>;
							rdfs:comment "Associates the surgery sub type with the surgery iteration.";
							dcterms:modified "2021-05-17"^^xsd:date;
							dcterms:creator <https://www.tib.eu/en/research-development/scientific-data-management/staff/samaneh-jozashoori/>.

<http://research.tib.eu/clarify2020/vocab/hasResectionGrade>	rdf:type 	owl:ObjectProperty;	
							rdfs:label	"hasResectionGrade";
							rdfs:domain	<http://research.tib.eu/clarify2020/vocab/OncologicalSurgery>;
							rdfs:range	<http://research.tib.eu/clarify2020/vocab/SurgeryResectionDegree>;
							rdfs:comment "Associates the oncological surgery with the surgery resection degree.";
							dcterms:modified "2021-05-17"^^xsd:date;
							dcterms:creator <https://www.tib.eu/en/research-development/scientific-data-management/staff/samaneh-jozashoori/>.

<http://research.tib.eu/clarify2020/vocab/hasTreatment>	rdf:type	owl:ObjectProperty;
						rdfs:label	"hasTreatment";
						rdfs:domain	<http://research.tib.eu/clarify2020/vocab/CPatient>;
						rdfs:range	<http://research.tib.eu/clarify2020/vocab/OncologicalTreatmentLine>;
						rdfs:comment "Represents the type of treatment.";
						dcterms:modified "2021-11-05"^^xsd:date;														
						dcterms:creator <https://www.tib.eu/en/research-development/scientific-data-management/staff/samaneh-jozashoori/>.

<http://research.tib.eu/clarify2020/vocab/has_LC_SLCG_ID>	rdf:type 	owl:ObjectProperty;	
						rdfs:label	"has_LC_SLCG_ID";
						rdfs:domain	<http://research.tib.eu/clarify2020/vocab/CancerPatient>;
						rdfs:range	<http://research.tib.eu/clarify2020/vocab/PatientIdentifier>;
						rdfs:comment "Associates LC patients with their SLCG identifiers.";
						dcterms:modified "2021-11-17"^^xsd:date;
						dcterms:creator <https://www.tib.eu/en/research-development/scientific-data-management/staff/samaneh-jozashoori/>.

<http://research.tib.eu/clarify2020/vocab/has_LC_HUPHM_ID>	rdf:type 	owl:ObjectProperty;	
						rdfs:label	"has_LC_HUPHM_ID";
						rdfs:domain	<http://research.tib.eu/clarify2020/vocab/CancerPatient>;
						rdfs:range	<http://research.tib.eu/clarify2020/vocab/PatientIdentifier>;
						rdfs:comment "Associates LC patients with their HUPHM identifiers.";
						dcterms:modified "2021-11-17"^^xsd:date;
						dcterms:creator <https://www.tib.eu/en/research-development/scientific-data-management/staff/samaneh-jozashoori/>.

<http://research.tib.eu/clarify2020/vocab/has_LC_KH_ID>	rdf:type 	owl:ObjectProperty;	
						rdfs:label	"has_LC_KH_ID";
						rdfs:domain	<http://research.tib.eu/clarify2020/vocab/CancerPatient>;
						rdfs:range	<http://research.tib.eu/clarify2020/vocab/PatientIdentifier>;
						rdfs:comment "Associates LC patients with their KH identifiers.";
						dcterms:modified "2021-11-17"^^xsd:date;
						dcterms:creator <https://www.tib.eu/en/research-development/scientific-data-management/staff/samaneh-jozashoori/>.

<http://research.tib.eu/clarify2020/vocab/has_BC_HUPHM_ID>	rdf:type 	owl:ObjectProperty;	
						rdfs:label	"has_BC_HUPHM_ID";
						rdfs:domain	<http://research.tib.eu/clarify2020/vocab/CancerPatient>;
						rdfs:range	<http://research.tib.eu/clarify2020/vocab/PatientIdentifier>;
						rdfs:comment "Associates BC patients with their HUPHM identifiers.";
						dcterms:modified "2021-11-17"^^xsd:date;
						dcterms:creator <https://www.tib.eu/en/research-development/scientific-data-management/staff/samaneh-jozashoori/>.

<http://research.tib.eu/clarify2020/vocab/has_BC_KH_ID>	rdf:type 	owl:ObjectProperty;	
						rdfs:label	"has_BC_KH_ID";
						rdfs:domain	<http://research.tib.eu/clarify2020/vocab/CancerPatient>;
						rdfs:range	<http://research.tib.eu/clarify2020/vocab/PatientIdentifier>;
						rdfs:comment "Associates BC patients with their KH identifiers.";
						dcterms:modified "2021-11-17"^^xsd:date;
						dcterms:creator <https://www.tib.eu/en/research-development/scientific-data-management/staff/samaneh-jozashoori/>.

<http://research.tib.eu/clarify2020/vocab/belongsTo>	rdf:type 	owl:ObjectProperty;	
						rdfs:label	"belongsTo";
						rdfs:domain	<http://research.tib.eu/clarify2020/vocab/CancerPatient>;
						rdfs:range	<http://research.tib.eu/clarify2020/vocab/PatientCategory>;
						rdfs:comment "Representsthe associations of the patients to specific category.";
						dcterms:modified "2021-11-17"^^xsd:date;
						dcterms:creator <https://www.tib.eu/en/research-development/scientific-data-management/staff/samaneh-jozashoori/>.

<http://research.tib.eu/clarify2020/vocab/treatmentLineNumber>	rdf:type 	owl:ObjectProperty;	
						rdfs:label	"treatmentLineNumber";
						rdfs:domain	<http://research.tib.eu/clarify2020/vocab/ClinicalTrialTreatmentLine>;
						rdfs:range	<http://research.tib.eu/clarify2020/vocab/TreatmentLineNumber>;
						rdfs:comment "Associates the clinical trial treatment line to the treatment line.";
						dcterms:modified "2021-11-17"^^xsd:date;
						dcterms:creator <https://www.tib.eu/en/research-development/scientific-data-management/staff/samaneh-jozashoori/>.

<http://research.tib.eu/clarify2020/vocab/hasComorbidityTreatmentLine>	rdf:type 	owl:ObjectProperty;	
									rdfs:label	"hasComorbidityTreatmentLine";
									rdfs:domain	<http://research.tib.eu/clarify2020/vocab/CancerPatient>;
									rdfs:range	<http://research.tib.eu/clarify2020/vocab/ComorbidityTreatmentLine>;
									rdfs:comment "Associates the patient with the comorbidity treatment line observation.";
									dcterms:modified "2021-11-17"^^xsd:date;
									dcterms:creator <https://www.tib.eu/en/research-development/scientific-data-management/staff/samaneh-jozashoori/>.

<http://research.tib.eu/clarify2020/vocab/has_parentWithCancer_OrNot>	rdf:type 	owl:ObjectProperty;	
									rdfs:label	"has_parentWithCancer_OrNot";
									rdfs:domain	<http://research.tib.eu/clarify2020/vocab/CancerPatient>;
									rdfs:range	<http://research.tib.eu/clarify2020/vocab/ParentWithCancer>;
									rdfs:comment "Associates the patient with the comorbidity treatment line observation.";
									dcterms:modified "2021-11-17"^^xsd:date;
									dcterms:creator <https://www.tib.eu/en/research-development/scientific-data-management/staff/samaneh-jozashoori/>.

<http://research.tib.eu/clarify2020/vocab/hasMenopauseAge>	rdf:type 	owl:ObjectProperty;	
						rdfs:label	"hasMenopauseAge";
						rdfs:domain	<http://research.tib.eu/clarify2020/vocab/CancerPatient>;
						rdfs:range	<http://research.tib.eu/clarify2020/vocab/MenopauseAge>;
						rdfs:comment "The association between the patient and the menopause age.";
						dcterms:modified "2021-11-17"^^xsd:date;
						dcterms:creator <https://www.tib.eu/en/research-development/scientific-data-management/staff/samaneh-jozashoori/>.

<http://research.tib.eu/clarify2020/vocab/hasMenarcheAge>	rdf:type 	owl:ObjectProperty;	
						rdfs:label	"hasMenarcheAge";
						rdfs:domain	<http://research.tib.eu/clarify2020/vocab/CancerPatient>;
						rdfs:range	<http://research.tib.eu/clarify2020/vocab/MenarcheAge>;
						rdfs:comment "The association between the patient and the menarche age.";
						dcterms:modified "2021-11-17"^^xsd:date;
						dcterms:creator <https://www.tib.eu/en/research-development/scientific-data-management/staff/samaneh-jozashoori/>.

<http://research.tib.eu/clarify2020/vocab/hasTreatmentEpisode>	rdf:type 	owl:ObjectProperty;	
						rdfs:label	"hasTreatmentEpisode";
						rdfs:domain	<http://research.tib.eu/clarify2020/vocab/CancerPatient>;
						rdfs:range	<http://research.tib.eu/clarify2020/vocab/TreatmentEpisode>;
						rdfs:comment "The association between the patient and the treatment episode.";
						dcterms:modified "2022-09-12"^^xsd:date;
						dcterms:creator <https://www.tib.eu/en/research-development/scientific-data-management/staff/samaneh-jozashoori/>.

<http://research.tib.eu/clarify2020/vocab/hasTreatmentType>	rdf:type 	owl:ObjectProperty;	
							rdfs:label	"hasTreatmentType";
							rdfs:domain	<http://research.tib.eu/clarify2020/vocab/TreatmentEpisode>;
							rdfs:range	<http://research.tib.eu/clarify2020/vocab/Treatment>;
							rdfs:comment "The association between the treatment episode and the specific treatement type.";
							dcterms:modified "2022-09-12"^^xsd:date;
							dcterms:creator <https://www.tib.eu/en/research-development/scientific-data-management/staff/samaneh-jozashoori/>.

<http://research.tib.eu/clarify2020/vocab/hasEpisode>	rdf:type 	owl:ObjectProperty;	
					rdfs:label	"hasEpisode";
					rdfs:domain	<http://research.tib.eu/clarify2020/vocab/OncologicalProcedure>;
					rdfs:range	<http://research.tib.eu/clarify2020/vocab/Episode>;
					rdfs:comment "The association between any oncological procedure and the corresponding episodes .";
					dcterms:modified "2022-09-12"^^xsd:date;
					dcterms:creator <https://www.tib.eu/en/research-development/scientific-data-management/staff/samaneh-jozashoori/>.

<http://research.tib.eu/clarify2020/vocab/hasEpisodeType>	rdf:type 	owl:ObjectProperty;	
						rdfs:label	"hasEpisodeType";
						rdfs:domain	<http://research.tib.eu/clarify2020/vocab/TreatmentEpisode>;
						rdfs:range	<http://research.tib.eu/clarify2020/vocab/EpisodeType>;
						rdfs:comment "The association between treatment episodes and corresponding types .";
						dcterms:modified "2022-09-12"^^xsd:date;
						dcterms:creator <https://www.tib.eu/en/research-development/scientific-data-management/staff/samaneh-jozashoori/>.

<http://research.tib.eu/clarify2020/vocab/hasTreatmentMaintenance>	rdf:type 	owl:ObjectProperty;	
								rdfs:label	"hasTreatmentMaintenance";
								rdfs:domain	<http://research.tib.eu/clarify2020/vocab/Chemotherapy>;
								rdfs:range	<http://research.tib.eu/clarify2020/vocab/Drug>;
								rdfs:comment "The association between the maintenance chemotherapy treatment and the prescribed drug.";
								dcterms:modified "2022-09-12"^^xsd:date;
								dcterms:creator <https://www.tib.eu/en/research-development/scientific-data-management/staff/samaneh-jozashoori/>.

<http://research.tib.eu/clarify2020/vocab/hasMaintenanceCycles>	rdf:type 	owl:ObjectProperty;	
								rdfs:label	"hasMaintenanceCycles";
								rdfs:domain	<http://research.tib.eu/clarify2020/vocab/Chemotherapy>;
								rdfs:range	<http://research.tib.eu/clarify2020/vocab/TreatmentLineCycle>;
								rdfs:comment "The association between the maintenance chemotherapy treatment nad the cycles of the treatment.";
								dcterms:modified "2022-09-12"^^xsd:date;
								dcterms:creator <https://www.tib.eu/en/research-development/scientific-data-management/staff/samaneh-jozashoori/>.

<http://research.tib.eu/clarify2020/vocab/hasOralDrug>	rdf:type 	owl:ObjectProperty;	
					rdfs:label	"hasOralDrug";
					rdfs:domain	<http://research.tib.eu/clarify2020/vocab/BCPatient>;
					rdfs:range	<http://research.tib.eu/clarify2020/vocab/Drug>;
					rdfs:comment "The association between the cycles of the treatment.";
					dcterms:modified "2022-09-12"^^xsd:date;
					dcterms:creator <https://www.tib.eu/en/research-development/scientific-data-management/staff/samaneh-jozashoori/>.

<http://research.tib.eu/clarify2020/vocab/hasOralDrugType>	rdf:type 	owl:ObjectProperty;	
						rdfs:label	"hasOralDrugType";
						rdfs:domain	<http://research.tib.eu/clarify2020/vocab/BCPatient>;
						rdfs:range	<http://research.tib.eu/clarify2020/vocab/Concept>;
						rdfs:comment "The association between the patient and the prescribed oral drugs.";
						dcterms:modified "2022-09-12"^^xsd:date;
						dcterms:creator <https://www.tib.eu/en/research-development/scientific-data-management/staff/samaneh-jozashoori/>.

<http://research.tib.eu/clarify2020/vocab/estrogenPositive>	rdf:type 	owl:ObjectProperty;	
							rdfs:label	"estrogenPositive";
							rdfs:domain	<http://research.tib.eu/clarify2020/vocab/BCPatient>;
							rdfs:range	<http://research.tib.eu/clarify2020/vocab/Concept>;
							rdfs:comment "The association between the patient and information about the receptor for the hormone estrogen.";
							dcterms:modified "2022-09-12"^^xsd:date;
							dcterms:creator <https://www.tib.eu/en/research-development/scientific-data-management/staff/samaneh-jozashoori/>.

<http://research.tib.eu/clarify2020/vocab/progesteronePositive>	rdf:type 	owl:ObjectProperty;	
								rdfs:label	"progesteronePositive";
								rdfs:domain	<http://research.tib.eu/clarify2020/vocab/BCPatient>;
								rdfs:range	<http://research.tib.eu/clarify2020/vocab/Concept>;
								rdfs:comment "The association between the patient and information about the receptor for the hormone progesterone.";
								dcterms:modified "2022-09-12"^^xsd:date;
								dcterms:creator <https://www.tib.eu/en/research-development/scientific-data-management/staff/samaneh-jozashoori/>.

<http://research.tib.eu/clarify2020/vocab/her2Positive>	rdf:type 	owl:ObjectProperty;	
						rdfs:label	"her2Positive";
						rdfs:domain	<http://research.tib.eu/clarify2020/vocab/BCPatient>;
						rdfs:range	<http://research.tib.eu/clarify2020/vocab/Concept>;
						rdfs:comment "The association between the patient and information about the protein HER2.";
						dcterms:modified "2022-09-12"^^xsd:date;
						dcterms:creator <https://www.tib.eu/en/research-development/scientific-data-management/staff/samaneh-jozashoori/>.

<http://research.tib.eu/clarify2020/vocab/hasTNMstageAssessment>	rdf:type 	owl:ObjectProperty;	
								rdfs:label	"hasTNMstageAssessment";
								rdfs:domain	<http://research.tib.eu/clarify2020/vocab/CPatient>;
								rdfs:range	<http://research.tib.eu/clarify2020/vocab/TNMstageAssessment>;
								rdfs:comment "The association between the patient and the TNM stage assessment event.";
								dcterms:modified "2022-09-12"^^xsd:date;
								dcterms:creator <https://www.tib.eu/en/research-development/scientific-data-management/staff/samaneh-jozashoori/>.

<http://research.tib.eu/clarify2020/vocab/hasTNMstage>	rdf:type 	owl:ObjectProperty;	
					rdfs:label	"hasTNMstage";
					rdfs:domain	<http://research.tib.eu/clarify2020/vocab/TNMstageAssessment>;
					rdfs:range	<http://research.tib.eu/clarify2020/vocab/TNMstage>;
					rdfs:comment "The association between the TNM stage assessment event and the TNM stage assessment result.";
					dcterms:modified "2022-09-12"^^xsd:date;
					dcterms:creator <https://www.tib.eu/en/research-development/scientific-data-management/staff/samaneh-jozashoori/>.

<http://research.tib.eu/clarify2020/vocab/hasTumorHistologyAssessment>	rdf:type 	owl:ObjectProperty;	
									rdfs:label	"hasTumorHistologyAssessment";
									rdfs:domain	<http://research.tib.eu/clarify2020/vocab/CPatient>;
									rdfs:range	<http://research.tib.eu/clarify2020/vocab/TumorHistologyAssessment>;
									rdfs:comment "The association between the patient and the tumor histology assessment event.";
									dcterms:modified "2022-09-12"^^xsd:date;
									dcterms:creator <https://www.tib.eu/en/research-development/scientific-data-management/staff/samaneh-jozashoori/>.

<http://research.tib.eu/clarify2020/vocab/hasHistology>	rdf:type 	owl:ObjectProperty;	
						rdfs:label	"hasHistology";
						rdfs:domain	<http://research.tib.eu/clarify2020/vocab/TumorHistologyAssessment>;
						rdfs:range	<http://research.tib.eu/clarify2020/vocab/TumorType>;
						rdfs:comment "The association between the tumor histology assessment event and the tumor type.";
						dcterms:modified "2022-09-12"^^xsd:date;
						dcterms:creator <https://www.tib.eu/en/research-development/scientific-data-management/staff/samaneh-jozashoori/>.

<http://research.tib.eu/clarify2020/vocab/hasMonitoring>	rdf:type 	owl:ObjectProperty;	
						rdfs:label	"hasMonitoring";
						rdfs:domain	<http://research.tib.eu/clarify2020/vocab/CPatient>;
						rdfs:range	<http://research.tib.eu/clarify2020/vocab/StatusEvolution>;
						rdfs:comment "The association between the cancer patient and the evolution assessment result.";
						dcterms:modified "2023-01-11"^^xsd:date;
						dcterms:creator <https://www.tib.eu/en/research-development/scientific-data-management/staff/samaneh-jozashoori/>.

<http://research.tib.eu/clarify2020/vocab/hasNeoadjuvantTherapy>	rdf:type 	owl:ObjectProperty;	
								rdfs:label	"hasNeoadjuvantTherapy";
								rdfs:domain	<http://research.tib.eu/clarify2020/vocab/CPatient>;
								rdfs:range	<http://research.tib.eu/clarify2020/vocab/NeoadjuvantTherapy>;
								rdfs:comment "The association between the cancer patient and the neoadjuvant therapy.";
								dcterms:modified "2023-01-11"^^xsd:date;
								dcterms:creator <https://www.tib.eu/en/research-development/scientific-data-management/staff/samaneh-jozashoori/>.

<http://research.tib.eu/clarify2020/vocab/hasObservation>	rdf:type 	owl:ObjectProperty;	
						rdfs:label	"hasObservation";
						rdfs:domain	<http://research.tib.eu/clarify2020/vocab/CPatient>;
						rdfs:range	<http://research.tib.eu/clarify2020/vocab/Observation>;
						rdfs:comment "The association between the cancer patient and the performed observations.";
						dcterms:modified "2023-01-11"^^xsd:date;
						dcterms:creator <https://www.tib.eu/en/research-development/scientific-data-management/staff/samaneh-jozashoori/>.

<http://research.tib.eu/clarify2020/vocab/hasRadiotherapyRound>	rdf:type 	owl:ObjectProperty;	
								rdfs:label	"hasRadiotherapyRound";
								rdfs:domain	<http://research.tib.eu/clarify2020/vocab/Radiotherapy>;
								rdfs:range	<http://research.tib.eu/clarify2020/vocab/RadiotherapyRound>;
								rdfs:comment "The association between a radiotherapy of a cancer patient and its corresponding information.";
								dcterms:modified "2023-01-11"^^xsd:date;
								dcterms:creator <https://www.tib.eu/en/research-development/scientific-data-management/staff/samaneh-jozashoori/>.

<http://research.tib.eu/clarify2020/vocab/hasProgressionRelapseAssessment>	rdf:type 	owl:ObjectProperty;	
										rdfs:label	"hasProgressionRelapseAssessment";
										rdfs:domain	<http://research.tib.eu/clarify2020/vocab/CPatient>;
										rdfs:range	<http://research.tib.eu/clarify2020/vocab/ProgressionRelapseAssessment>;
										rdfs:comment "The association between the cancer patient and the assessment of the progression and the relapse.";
										dcterms:modified "2023-01-11"^^xsd:date;
										dcterms:creator <https://www.tib.eu/en/research-development/scientific-data-management/staff/samaneh-jozashoori/>.

<http://research.tib.eu/clarify2020/vocab/smokerType>	rdf:type 	owl:ObjectProperty;	
					rdfs:label	"smokerType";
					rdfs:domain	<http://research.tib.eu/clarify2020/vocab/CPatient>;
					rdfs:range	<http://research.tib.eu/clarify2020/vocab/SmokerType>;
					rdfs:comment "The association between the smoker cancer patient and the smoker types categorized based on the frequency of the consumption.";
					dcterms:modified "2023-01-11"^^xsd:date;
					dcterms:creator <https://www.tib.eu/en/research-development/scientific-data-management/staff/samaneh-jozashoori/>.


######################################################################################################################################
#####################################################    annotation    ##############################################################
######################################################################################################################################

<http://www.w3.org/ns/prov#has_provenance>	rdf:type	owl:ObjectProperty;
					rdfs:label	"has_provenance";
					rdfs:domain <http://research.tib.eu/clarify2020/vocab/Concept>;
					rdfs:range	<http://research.tib.eu/clarify2020/vocab/Source>;
					rdfs:comment	"Indicates a provenance-URI for a resource; the resource identified by this property presents a provenance record about its subject or anchor resource.";	
					dcterms:modified "2021-12-29"^^xsd:date;
					dcterms:creator <https://www.tib.eu/en/research-development/scientific-data-management/staff/samaneh-jozashoori/>.

<http://research.tib.eu/clarify2020/vocab/hasCUIAnnotation>	rdf:type owl:ObjectProperty;
							rdfs:label	"hasCUIAnnotation";
							rdfs:domain <http://research.tib.eu/clarify2020/vocab/Concept>;
			  				rdfs:range <http://research.tib.eu/clarify2020/vocab/Annotation>;
							rdfs:comment	"CUI annotation of the concept.";
							dcterms:modified "2020-10-19"^^xsd:date;
							dcterms:creator <https://www.tib.eu/en/research-development/scientific-data-management/staff/samaneh-jozashoori/>.

<http://research.tib.eu/clarify2020/vocab/hasCUI>	rdf:type owl:ObjectProperty;
				rdfs:label	"hasCUI";
				rdfs:domain <http://research.tib.eu/clarify2020/vocab/Concept>;
  				rdfs:range <http://research.tib.eu/clarify2020/vocab/Annotation>;
				rdfs:comment	"Connection between a concept and corresponding CUI.";
				dcterms:modified "2021-12-16"^^xsd:date;
				dcterms:creator <https://www.tib.eu/en/research-development/scientific-data-management/staff/samaneh-jozashoori/>.

######################################################################################################################################
#####################################################    Publication    ##############################################################
######################################################################################################################################

<http://research.tib.eu/clarify2020/vocab/hasAnnotation>	rdf:type owl:ObjectProperty;
						rdfs:label	"hasAnnotation";
						rdfs:domain <http://research.tib.eu/clarify2020/vocab/Relation>;
		  				rdfs:range <http://research.tib.eu/clarify2020/vocab/Annotation>;
						rdfs:comment	"Connection between the annotation and the relation between annotation and publication";
						dcterms:modified "2020-12-15"^^xsd:date;
						dcterms:creator <https://www.tib.eu/en/research-development/scientific-data-management/staff/samaneh-jozashoori/>.

<http://research.tib.eu/clarify2020/vocab/annotates>	rdf:type	owl:ObjectProperty;
					rdfs:label	"annotates";
					rdfs:domain	<http://research.tib.eu/clarify2020/vocab/Relation>;
					rdfs:range	<http://research.tib.eu/clarify2020/vocab/Publication>;
					rdfs:comment	"Connection between mentionedIn or HasTopic relation with CUI.";
					dcterms:modified "2020-12-15"^^xsd:date;
					dcterms:creator <https://www.tib.eu/en/research-development/scientific-data-management/staff/samaneh-jozashoori/>.

<http://research.tib.eu/clarify2020/vocab/relation_isRelatedTo_publication>	rdf:type        owl:ObjectProperty;	
											rdfs:label	"relation_isRelatedTo_publication";
											rdfs:domain	<http://research.tib.eu/clarify2020/vocab/Relation>;
											rdfs:range	<http://research.tib.eu/clarify2020/vocab/Publication>;
											rdfs:comment "The relationship between the relation and the publication.";
											dcterms:modified "2020-12-15"^^xsd:date;
											dcterms:creator <https://www.tib.eu/en/research-development/scientific-data-management/staff/samaneh-jozashoori/>.				

<http://research.tib.eu/clarify2020/vocab/relation_isRelatedTo_subject_annotation>	rdf:type        owl:ObjectProperty;	
												rdfs:label	"relation_isRelatedTo_subject_annotation";
												rdfs:domain	<http://research.tib.eu/clarify2020/vocab/Relation>;
												rdfs:range	<http://research.tib.eu/clarify2020/vocab/Annotation>;
												rdfs:comment "The relationship between the relation and the CUI annotation.";
												dcterms:modified "2023-01-11"^^xsd:date;
												dcterms:creator <https://www.tib.eu/en/research-development/scientific-data-management/staff/samaneh-jozashoori/>.				

<http://research.tib.eu/clarify2020/vocab/relation_isRelatedTo_object_annotation>	rdf:type        owl:ObjectProperty;	
												rdfs:label	"relation_isRelatedTo_object_annotation";
												rdfs:domain	<http://research.tib.eu/clarify2020/vocab/Relation>;
												rdfs:range	<http://research.tib.eu/clarify2020/vocab/Annotation>;
												rdfs:comment "The relationship between the relation and the CUI annotation.";
												dcterms:modified "2023-01-11"^^xsd:date;
												dcterms:creator <https://www.tib.eu/en/research-development/scientific-data-management/staff/samaneh-jozashoori/>.				

<http://research.tib.eu/clarify2020/vocab/relation_isRelatedTo_id>		rdf:type        owl:ObjectProperty;	
									rdfs:label	"relation_isRelatedTo_id";
									rdfs:domain	<http://research.tib.eu/clarify2020/vocab/Relation>;
									rdfs:range	<http://research.tib.eu/clarify2020/vocab/RelationIdentifier>;
									rdfs:comment "The relationship between the relation and its identifier.";
									dcterms:modified "2023-01-11"^^xsd:date;
									dcterms:creator <https://www.tib.eu/en/research-development/scientific-data-management/staff/samaneh-jozashoori/>.				

<http://research.tib.eu/clarify2020/vocab/relation_isRelatedTo_source>		rdf:type        owl:ObjectProperty;	
										rdfs:label	"relation_isRelatedTo_source";
										rdfs:domain	<http://research.tib.eu/clarify2020/vocab/Relation>;
										rdfs:range	<http://research.tib.eu/clarify2020/vocab/Source>;
										rdfs:comment "The relationship between the relation and the source.";
										dcterms:modified "2023-01-11"^^xsd:date;
										dcterms:creator <https://www.tib.eu/en/research-development/scientific-data-management/staff/samaneh-jozashoori/>.				

<http://research.tib.eu/clarify2020/vocab/hasAuthor>	rdf:type owl:ObjectProperty;
					rdfs:label "hasAuthor";
					rdfs:domain <http://research.tib.eu/clarify2020/vocab/Publication>;
				  	rdfs:range <http://research.tib.eu/clarify2020/vocab/Author>;
					rdfs:comment "Author of Publication.";
					dcterms:modified "2021-05-17"^^xsd:date;
					dcterms:creator <https://www.tib.eu/en/research-development/scientific-data-management/staff/samaneh-jozashoori/>.

<http://research.tib.eu/clarify2020/vocab/hasPublicationType>	rdf:type owl:ObjectProperty;
					rdfs:label "hasPublicationType";
					rdfs:domain <http://research.tib.eu/clarify2020/vocab/Publication>;
				  	rdfs:range <http://research.tib.eu/clarify2020/vocab/PublicationType>;
					rdfs:comment "The publication type.";
					dcterms:modified "2021-06-08"^^xsd:date;
					dcterms:creator <https://www.tib.eu/en/research-development/scientific-data-management/staff/samaneh-jozashoori/>.

<http://research.tib.eu/clarify2020/vocab/publication_isRelatedTo_Disease>	rdf:type owl:ObjectProperty;
					rdfs:label "publication_isRelatedTo_Disease";
					rdfs:domain <http://research.tib.eu/clarify2020/vocab/Publication>;
				  	rdfs:range <http://research.tib.eu/clarify2020/vocab/Disorder>;
					rdfs:comment "Represents the disorder to which the publicaiton correspondes.";
					dcterms:modified "2021-11-17"^^xsd:date;
					dcterms:creator <https://www.tib.eu/en/research-development/scientific-data-management/staff/samaneh-jozashoori/>.

######################################################################################################################################
#########################################################    Drug    #################################################################
######################################################################################################################################


<http://research.tib.eu/clarify2020/vocab/biomarker_has_indication>	rdf:type	owl:ObjectProperty;
								rdfs:label	"biomarker_has_indication";
								rdfs:domain	<http://research.tib.eu/clarify2020/vocab/Biomarker>;
								rdfs:range	<http://research.tib.eu/clarify2020/vocab/Drug>;
								rdfs:comment	"A biomarker has indication Drug";
								dcterms:modified "2020-12-15"^^xsd:date;
								dcterms:creator <https://www.tib.eu/en/research-development/scientific-data-management/staff/samaneh-jozashoori/>.

<http://research.tib.eu/clarify2020/vocab/interactor1>	rdf:type owl:ObjectProperty;
					rdfs:label "interactor1";
					rdfs:domain <http://research.tib.eu/clarify2020/vocab/Interaction>;
				  	rdfs:range <http://research.tib.eu/clarify2020/vocab/Concept>;
					rdfs:comment "Interactor 1";
					dcterms:modified "2020-12-15"^^xsd:date;
					dcterms:creator <https://www.tib.eu/en/research-development/scientific-data-management/staff/samaneh-jozashoori/>.

<http://research.tib.eu/clarify2020/vocab/interactor2>	rdf:type owl:ObjectProperty;
					rdfs:label "interactor2";
					rdfs:domain <http://research.tib.eu/clarify2020/vocab/Interaction>;
				  	rdfs:range <http://research.tib.eu/clarify2020/vocab/Concept>;
					rdfs:comment "Interactor 2";
					dcterms:modified "2021-11-16"^^xsd:date;
					dcterms:creator <https://www.tib.eu/en/research-development/scientific-data-management/staff/samaneh-jozashoori/>.

<http://research.tib.eu/clarify2020/vocab/drug_isRelatedTo_dse>	rdf:type	owl:ObjectProperty;
							rdfs:label	"drug_isRelatedTo_dse";
							rdfs:domain	<http://research.tib.eu/clarify2020/vocab/Drug>;
							rdfs:range	<http://research.tib.eu/clarify2020/vocab/DrugSideEffect>;
							rdfs:comment	"relationship between drug and drug-sideEffect relation.";
							dcterms:modified "2020-12-15"^^xsd:date;
							dcterms:creator <https://www.tib.eu/en/research-development/scientific-data-management/staff/samaneh-jozashoori/>.

<http://research.tib.eu/clarify2020/vocab/sideEffect_isRelatedTo_dse>	rdf:type	owl:ObjectProperty;
									rdfs:label	"sideEffect_isRelatedTo_dse";
									rdfs:domain	<http://research.tib.eu/clarify2020/vocab/Phenotype>;
									rdfs:range	<http://research.tib.eu/clarify2020/vocab/DrugSideEffect>;
									rdfs:comment	"relationship between sideEffect and drug-sideEffect relation.";
									dcterms:modified "2020-12-15"^^xsd:date;
									dcterms:creator <https://www.tib.eu/en/research-development/scientific-data-management/staff/samaneh-jozashoori/>.

<http://research.tib.eu/clarify2020/vocab/enzyme_isRelatedTo_gene>	rdf:type	owl:ObjectProperty;
									rdfs:label	"enzyme_isRelatedTo_gene";
									rdfs:domain	<http://research.tib.eu/clarify2020/vocab/Enzyme>;
									rdfs:range	<http://research.tib.eu/clarify2020/vocab/Gene>;
									rdfs:comment	"The relationship between the enzyme and the gene from which it is produced.";
									dcterms:modified "2020-09-14"^^xsd:date;
									dcterms:creator <https://www.tib.eu/en/research-development/scientific-data-management/staff/samaneh-jozashoori/>.

<http://research.tib.eu/clarify2020/vocab/affects>	rdf:type	owl:ObjectProperty;
								rdfs:label	"affects";
								rdfs:domain	<http://research.tib.eu/clarify2020/vocab/DrugDrugInteraction>;
								rdfs:range	<http://research.tib.eu/clarify2020/vocab/Drug>;
								rdfs:comment	"The conncetion between drug that affects by the other one through their interaction and the interaction node.";
								dcterms:modified "2020-12-15"^^xsd:date;
								dcterms:creator <https://www.tib.eu/en/research-development/scientific-data-management/staff/samaneh-jozashoori/>.

<http://research.tib.eu/clarify2020/vocab/isAffected>	rdf:type	owl:ObjectProperty;
								rdfs:label	"isAffected";
								rdfs:domain	<http://research.tib.eu/clarify2020/vocab/DrugDrugInteraction>;
								rdfs:range	<http://research.tib.eu/clarify2020/vocab/Drug>;
								rdfs:comment	"The conncetion between drug that is affected by the other one through their interaction and the interaction node.";
								dcterms:modified "2020-12-15"^^xsd:date;
								dcterms:creator <https://www.tib.eu/en/research-development/scientific-data-management/staff/samaneh-jozashoori/>.

<http://research.tib.eu/clarify2020/vocab/precipitant_drug>	rdf:type	owl:ObjectProperty;
								rdfs:label	"precipitant_drug";
								rdfs:domain	<http://research.tib.eu/clarify2020/vocab/DrugDrugInteraction>;
								rdfs:range	<http://research.tib.eu/clarify2020/vocab/Drug>;
								rdfs:comment	"The relationship between the drug drug interaction and corresponding precipitant drug.";
								dcterms:modified "2020-12-15"^^xsd:date;
								dcterms:creator <https://www.tib.eu/en/research-development/scientific-data-management/staff/samaneh-jozashoori/>.

<http://research.tib.eu/clarify2020/vocab/precipitant_drug_cui>	rdf:type	owl:ObjectProperty;
								rdfs:label	"precipitant_drug_cui";
								rdfs:domain	<http://research.tib.eu/clarify2020/vocab/DrugDrugInteraction>;
								rdfs:range	<http://research.tib.eu/clarify2020/vocab/Annotation>;
								rdfs:comment	"The relationship between the drug drug interaction and corresponding precipitant drug annotated by CUI IDs.";
								dcterms:modified "2021-06-30"^^xsd:date;
								dcterms:creator <https://www.tib.eu/en/research-development/scientific-data-management/staff/samaneh-jozashoori/>.

<http://research.tib.eu/clarify2020/vocab/object_drug>	rdf:type	owl:ObjectProperty;
								rdfs:label	"object_drug";
								rdfs:domain	<http://research.tib.eu/clarify2020/vocab/DrugDrugInteraction>;
								rdfs:range	<http://research.tib.eu/clarify2020/vocab/Drug>;
								rdfs:comment	"The relationship between the drug drug interaction and corresponding object drug .";
								dcterms:modified "2020-12-15"^^xsd:date;
								dcterms:creator <https://www.tib.eu/en/research-development/scientific-data-management/staff/samaneh-jozashoori/>.

<http://research.tib.eu/clarify2020/vocab/object_drug_cui>	rdf:type	owl:ObjectProperty;
								rdfs:label	"object_drug_cui";
								rdfs:domain	<http://research.tib.eu/clarify2020/vocab/DrugDrugInteraction>;
								rdfs:range	<http://research.tib.eu/clarify2020/vocab/Annotation>;
								rdfs:comment	"The relationship between the drug drug interaction and corresponding object drug annotated by CUI IDs.";
								dcterms:modified "2021-06-30"^^xsd:date;
								dcterms:creator <https://www.tib.eu/en/research-development/scientific-data-management/staff/samaneh-jozashoori/>.

<http://research.tib.eu/clarify2020/vocab/effect>	rdf:type	owl:ObjectProperty;
				rdfs:label	"effect";
				rdfs:domain	<http://research.tib.eu/clarify2020/vocab/DrugDrugInteraction>;
				rdfs:range	<http://research.tib.eu/clarify2020/vocab/AdverseEvent>;
				rdfs:comment	"The relationship between the drug drug interaction and corresponding adverse event.";
				dcterms:modified "2020-12-15"^^xsd:date;
				dcterms:creator <https://www.tib.eu/en/research-development/scientific-data-management/staff/samaneh-jozashoori/>.

<http://research.tib.eu/clarify2020/vocab/impact>	rdf:type	owl:ObjectProperty;
				rdfs:label	"impact";
				rdfs:domain	<http://research.tib.eu/clarify2020/vocab/DrugDrugInteraction>;
				rdfs:range	<http://research.tib.eu/clarify2020/vocab/Impact>;
				rdfs:comment	"The relationship between the drug drug interaction and corresponding impact.";
				dcterms:modified "2021-06-30"^^xsd:date;
				dcterms:creator <https://www.tib.eu/en/research-development/scientific-data-management/staff/samaneh-jozashoori/>.

<http://research.tib.eu/clarify2020/vocab/effect_cui>	rdf:type	owl:ObjectProperty;
					rdfs:label	"effect_cui";
					rdfs:domain	<http://research.tib.eu/clarify2020/vocab/DrugDrugInteraction>;
					rdfs:range	<http://research.tib.eu/clarify2020/vocab/Annotation>;
					rdfs:comment	"The relationship between the drug drug interaction and corresponding adverse event annotated by CUI IDs.";
					dcterms:modified "2021-06-30"^^xsd:date;
					dcterms:creator <https://www.tib.eu/en/research-development/scientific-data-management/staff/samaneh-jozashoori/>.

<http://research.tib.eu/clarify2020/vocab/target_isRelatedTo_gene>	rdf:type	owl:ObjectProperty;
									rdfs:label	"target_isRelatedTo_gene";
									rdfs:domain	<http://research.tib.eu/clarify2020/vocab/Target>;
									rdfs:range	<http://research.tib.eu/clarify2020/vocab/Gene>;
									rdfs:comment	"The relationship between the target and the gene from which it is produced.";
									dcterms:modified "2020-12-15"^^xsd:date;
									dcterms:creator <https://www.tib.eu/en/research-development/scientific-data-management/staff/samaneh-jozashoori/>.

<http://research.tib.eu/clarify2020/vocab/cancerStage_has_indication>	rdf:type	owl:ObjectProperty;
									rdfs:label	"cancerStage_has_indication";
									rdfs:domain	<http://research.tib.eu/clarify2020/vocab/CancerStage>;
									rdfs:range	<http://research.tib.eu/clarify2020/vocab/Drug>;
									rdfs:comment	"Tumor stage has indication drug";
									dcterms:modified "2020-09-14"^^xsd:date;
									dcterms:creator <https://www.tib.eu/en/research-development/scientific-data-management/staff/samaneh-jozashoori/>.

<http://research.tib.eu/clarify2020/vocab/hasHPOAnnotation>	rdf:type owl:ObjectProperty;
							rdfs:label	"hasHPOAnnotation";
							rdfs:domain <http://research.tib.eu/clarify2020/vocab/Phenotype>;
			  				rdfs:range <http://research.tib.eu/clarify2020/vocab/Annotation>;
							rdfs:comment	"HPO annotation of the phenotype.";
							dcterms:modified "2020-12-15"^^xsd:date;
							dcterms:creator <https://www.tib.eu/en/research-development/scientific-data-management/staff/samaneh-jozashoori/>.
